@prefix owl: <http://www.w3.org/2002/07/owl#> .
@prefix rdf: <http://www.w3.org/1999/02/22-rdf-syntax-ns#> .
@prefix xml: <http://www.w3.org/XML/1998/namespace> .
@prefix xsd: <http://www.w3.org/2001/XMLSchema#> .
@prefix RBBO: <https://purl.org/turbbo/RBBO_> .
@prefix rdfs: <http://www.w3.org/2000/01/rdf-schema#> .

<https://purl.org/turbbo/RBBO_Behaviour.ttl> rdf:type owl:Ontology ;
                                              owl:versionIRI <https://purl.org/turbbo/2023-07-21/RBBO_Behaviour.ttl> ;
                                              <http://purl.obolibrary.org/obo/IAO_0000232> "We could not find URIs for the classes in the IC-Behavior taxonomy therefore we created them for this project. In this ontology, we have two formats of URI which is to differentiate between the classes from the taxonomy and the extended classes for RBBO. All classes in RBBO have URIs in this format https://purl.org/turbbo/RBBO_0000000  while the classes from IC-Behavior have the URI format https://purl.org/turbbo/RBBO_R9HlY0i7brkkaamN0VMCVmw." ;
                                              <http://purl.org/dc/elements/1.1/title> "RBBO_Behaviour" ;
                                              rdfs:comment "The RBBO_Behaviour module of RBBO provides a classification of different kinds of behaviours. This module of the ontology has reused and extended the behaviour taxonomy from IC-Behavior, which is currently, the broadest of behavioural taxonomies. Larsen et al.classified 250 behaviours into nine domains: learning and applying knowledge; communicating; moving/exercising; self-care behaviour; domestic life activities; interpersonal interactions and relationships; behaviour related to major life areas; behaviour related to community, social, and civic life; and mood/state changing activities and behaviour. Behaviors considered important enough to serve as the dependent variable in articles accepted for publication in top journals were extracted from a large sample of journals in nine different behavioral and social disciplines." ;
                                              owl:versionInfo "2023-07-21" .

#################################################################
#    Annotation properties
#################################################################

###  http://purl.obolibrary.org/obo/IAO_0000232
<http://purl.obolibrary.org/obo/IAO_0000232> rdf:type owl:AnnotationProperty ;
                                             rdfs:label "curator note" .


###  http://purl.org/dc/elements/1.1/title
<http://purl.org/dc/elements/1.1/title> rdf:type owl:AnnotationProperty .


###  http://www.geneontology.org/formats/oboInOwl#created_by
<http://www.geneontology.org/formats/oboInOwl#created_by> rdf:type owl:AnnotationProperty .


###  http://www.geneontology.org/formats/oboInOwl#creation_date
<http://www.geneontology.org/formats/oboInOwl#creation_date> rdf:type owl:AnnotationProperty .


###  http://www.w3.org/2004/02/skos/core#definition
<http://www.w3.org/2004/02/skos/core#definition> rdf:type owl:AnnotationProperty .


###  https://purl.org/turbbo/RBBO_0000093
<https://purl.org/turbbo/RBBO_0000093> rdf:type owl:AnnotationProperty ;
                                       <http://www.geneontology.org/formats/oboInOwl#created_by> "Fatima Maikore" ;
                                       <http://www.geneontology.org/formats/oboInOwl#creation_date> "2022-03-27T15:12:26.622064Z" ;
                                       rdfs:label "original_IRI" .


#################################################################
#    Classes
#################################################################

###  https://purl.org/turbbo/RBBO_0000001
<https://purl.org/turbbo/RBBO_0000001> rdf:type owl:Class ;
                                       rdfs:subClassOf RBBO:RCgGDn1vqlfJSIRaFveJ3LD ;
                                       <http://www.geneontology.org/formats/oboInOwl#created_by> "PaulN" ;
                                       <http://www.geneontology.org/formats/oboInOwl#creation_date> "2022-01-26T13:54:32.612842Z" ;
                                       rdfs:label "Taking contraceptive pill" .


###  https://purl.org/turbbo/RBBO_0000002
<https://purl.org/turbbo/RBBO_0000002> rdf:type owl:Class ;
                                       rdfs:subClassOf RBBO:RCgGDn1vqlfJSIRaFveJ3LD ;
                                       <http://www.geneontology.org/formats/oboInOwl#created_by> "PaulN" ;
                                       <http://www.geneontology.org/formats/oboInOwl#creation_date> "2022-01-26T13:55:09.32696Z" ;
                                       rdfs:label "Taking 'morning after' pill" .


###  https://purl.org/turbbo/RBBO_0000003
<https://purl.org/turbbo/RBBO_0000003> rdf:type owl:Class ;
                                       rdfs:subClassOf RBBO:RmsFbX68kZa0rYXa7PeIG7 ;
                                       <http://www.geneontology.org/formats/oboInOwl#created_by> "PaulN" ;
                                       <http://www.geneontology.org/formats/oboInOwl#creation_date> "2022-01-26T14:01:52.332179Z" ;
                                       rdfs:label "Cleaning/disinfecting surfaces" .


###  https://purl.org/turbbo/RBBO_0000004
<https://purl.org/turbbo/RBBO_0000004> rdf:type owl:Class ;
                                       rdfs:subClassOf RBBO:RmsFbX68kZa0rYXa7PeIG7 ;
                                       <http://www.geneontology.org/formats/oboInOwl#created_by> "PaulN" ;
                                       <http://www.geneontology.org/formats/oboInOwl#creation_date> "2022-01-26T14:02:38.36258Z" ;
                                       rdfs:label "Vacuuming" .


###  https://purl.org/turbbo/RBBO_0000005
<https://purl.org/turbbo/RBBO_0000005> rdf:type owl:Class ;
                                       rdfs:subClassOf RBBO:RmsFbX68kZa0rYXa7PeIG7 ;
                                       <http://www.geneontology.org/formats/oboInOwl#created_by> "PaulN" ;
                                       <http://www.geneontology.org/formats/oboInOwl#creation_date> "2022-01-26T14:02:57.303567Z" ;
                                       rdfs:label "Dusting" .


###  https://purl.org/turbbo/RBBO_0000006
<https://purl.org/turbbo/RBBO_0000006> rdf:type owl:Class ;
                                       rdfs:subClassOf RBBO:RmsFbX68kZa0rYXa7PeIG7 ;
                                       <http://www.geneontology.org/formats/oboInOwl#created_by> "PaulN" ;
                                       <http://www.geneontology.org/formats/oboInOwl#creation_date> "2022-01-26T14:03:26.313224Z" ;
                                       rdfs:label "Cleaning windows" .


###  https://purl.org/turbbo/RBBO_0000007
<https://purl.org/turbbo/RBBO_0000007> rdf:type owl:Class ;
                                       rdfs:subClassOf RBBO:R8cCVugnbr4KoPFPOy98Qt2 ;
                                       <http://www.geneontology.org/formats/oboInOwl#created_by> "PaulN" ;
                                       <http://www.geneontology.org/formats/oboInOwl#creation_date> "2022-01-26T14:09:59.948087Z" ;
                                       rdfs:label "Working from home" .


###  https://purl.org/turbbo/RBBO_0000008
<https://purl.org/turbbo/RBBO_0000008> rdf:type owl:Class ;
                                       rdfs:subClassOf RBBO:R8cCVugnbr4KoPFPOy98Qt2 ;
                                       <http://www.geneontology.org/formats/oboInOwl#created_by> "PaulN" ;
                                       <http://www.geneontology.org/formats/oboInOwl#creation_date> "2022-01-26T14:10:47.040096Z" ;
                                       rdfs:label "Departing late" .


###  https://purl.org/turbbo/RBBO_0000009
<https://purl.org/turbbo/RBBO_0000009> rdf:type owl:Class ;
                                       rdfs:subClassOf RBBO:R8cCVugnbr4KoPFPOy98Qt2 ;
                                       <http://www.geneontology.org/formats/oboInOwl#created_by> "PaulN" ;
                                       <http://www.geneontology.org/formats/oboInOwl#creation_date> "2022-01-26T14:11:42.149733Z" ;
                                       rdfs:label "Working overtime" .


###  https://purl.org/turbbo/RBBO_0000010
<https://purl.org/turbbo/RBBO_0000010> rdf:type owl:Class ;
                                       rdfs:subClassOf RBBO:R74Nph6Q96RGCllk8UMt94p ;
                                       <http://www.geneontology.org/formats/oboInOwl#created_by> "PaulN" ;
                                       <http://www.geneontology.org/formats/oboInOwl#creation_date> "2022-01-26T14:17:54.346094Z" ;
                                       rdfs:label "Hand washing" .


###  https://purl.org/turbbo/RBBO_0000011
<https://purl.org/turbbo/RBBO_0000011> rdf:type owl:Class ;
                                       rdfs:subClassOf RBBO:R74Nph6Q96RGCllk8UMt94p ;
                                       <http://www.geneontology.org/formats/oboInOwl#created_by> "PaulN" ;
                                       <http://www.geneontology.org/formats/oboInOwl#creation_date> "2022-01-26T14:19:07.670831Z" ;
                                       rdfs:label "Sneeze/coughing etiquette" .


###  https://purl.org/turbbo/RBBO_0000012
<https://purl.org/turbbo/RBBO_0000012> rdf:type owl:Class ;
                                       rdfs:subClassOf RBBO:R74Nph6Q96RGCllk8UMt94p ;
                                       <http://www.geneontology.org/formats/oboInOwl#created_by> "PaulN" ;
                                       <http://www.geneontology.org/formats/oboInOwl#creation_date> "2022-01-26T14:19:58.803199Z" ;
                                       rdfs:label "Use of mouthwash" .


###  https://purl.org/turbbo/RBBO_0000013
<https://purl.org/turbbo/RBBO_0000013> rdf:type owl:Class ;
                                       rdfs:subClassOf RBBO:R74Nph6Q96RGCllk8UMt94p ;
                                       <http://www.geneontology.org/formats/oboInOwl#created_by> "PaulN" ;
                                       <http://www.geneontology.org/formats/oboInOwl#creation_date> "2022-01-26T14:21:29.640325Z" ;
                                       rdfs:label "Ear waxing" .


###  https://purl.org/turbbo/RBBO_0000014
<https://purl.org/turbbo/RBBO_0000014> rdf:type owl:Class ;
                                       rdfs:subClassOf RBBO:R74Nph6Q96RGCllk8UMt94p ;
                                       <http://www.geneontology.org/formats/oboInOwl#created_by> "PaulN" ;
                                       <http://www.geneontology.org/formats/oboInOwl#creation_date> "2022-01-26T14:22:14.300615Z" ;
                                       rdfs:label "Body hair removal/waxing" .


###  https://purl.org/turbbo/RBBO_0000015
<https://purl.org/turbbo/RBBO_0000015> rdf:type owl:Class ;
                                       rdfs:subClassOf RBBO:RINOST75D6djkBWwq9c5bA ;
                                       <http://www.geneontology.org/formats/oboInOwl#created_by> "PaulN" ;
                                       <http://www.geneontology.org/formats/oboInOwl#creation_date> "2022-01-26T14:35:45.963639Z" ;
                                       rdfs:label "Sadomaschism" .


###  https://purl.org/turbbo/RBBO_0000016
<https://purl.org/turbbo/RBBO_0000016> rdf:type owl:Class ;
                                       rdfs:subClassOf RBBO:R9SZhlXBAdyrsI5ItrSRZDG ;
                                       <http://www.geneontology.org/formats/oboInOwl#created_by> "PaulN" ;
                                       <http://www.geneontology.org/formats/oboInOwl#creation_date> "2022-01-26T14:38:59.154819Z" ;
                                       rdfs:label "Wearing face masks" .


###  https://purl.org/turbbo/RBBO_0000017
<https://purl.org/turbbo/RBBO_0000017> rdf:type owl:Class ;
                                       rdfs:subClassOf RBBO:R9SZhlXBAdyrsI5ItrSRZDG ;
                                       <http://www.geneontology.org/formats/oboInOwl#created_by> "PaulN" ;
                                       <http://www.geneontology.org/formats/oboInOwl#creation_date> "2022-01-26T14:28:59.646652Z" ;
                                       rdfs:label "Social distancing" .


###  https://purl.org/turbbo/RBBO_0000018
<https://purl.org/turbbo/RBBO_0000018> rdf:type owl:Class ;
                                       rdfs:subClassOf RBBO:R9SZhlXBAdyrsI5ItrSRZDG ;
                                       <http://www.geneontology.org/formats/oboInOwl#created_by> "PaulN" ;
                                       <http://www.geneontology.org/formats/oboInOwl#creation_date> "2022-01-26T14:29:25.50612Z" ;
                                       rdfs:label "Avoiding crowded places" .


###  https://purl.org/turbbo/RBBO_0000019
<https://purl.org/turbbo/RBBO_0000019> rdf:type owl:Class ;
                                       rdfs:subClassOf RBBO:R9SZhlXBAdyrsI5ItrSRZDG ;
                                       <http://www.geneontology.org/formats/oboInOwl#created_by> "PaulN" ;
                                       <http://www.geneontology.org/formats/oboInOwl#creation_date> "2022-01-26T14:30:09.98683Z" ;
                                       rdfs:label "Ventilation/opening windows" .


###  https://purl.org/turbbo/RBBO_0000020
<https://purl.org/turbbo/RBBO_0000020> rdf:type owl:Class ;
                                       rdfs:subClassOf RBBO:R9p5Yej3AOqhbZTK2kCgSWX ;
                                       <http://www.geneontology.org/formats/oboInOwl#created_by> "PaulN" ;
                                       <http://www.geneontology.org/formats/oboInOwl#creation_date> "2022-01-26T14:41:54.711375Z" ;
                                       rdfs:label "Football" .


###  https://purl.org/turbbo/RBBO_0000021
<https://purl.org/turbbo/RBBO_0000021> rdf:type owl:Class ;
                                       rdfs:subClassOf RBBO:R9p5Yej3AOqhbZTK2kCgSWX ;
                                       <http://www.geneontology.org/formats/oboInOwl#created_by> "PaulN" ;
                                       <http://www.geneontology.org/formats/oboInOwl#creation_date> "2022-01-26T14:42:10.342379Z" ;
                                       rdfs:label "Hockey" .


###  https://purl.org/turbbo/RBBO_0000022
<https://purl.org/turbbo/RBBO_0000022> rdf:type owl:Class ;
                                       rdfs:subClassOf RBBO:R9p5Yej3AOqhbZTK2kCgSWX ;
                                       <http://www.geneontology.org/formats/oboInOwl#created_by> "PaulN" ;
                                       <http://www.geneontology.org/formats/oboInOwl#creation_date> "2022-01-26T14:42:26.657392Z" ;
                                       rdfs:label "Netball" .


###  https://purl.org/turbbo/RBBO_0000023
<https://purl.org/turbbo/RBBO_0000023> rdf:type owl:Class ;
                                       rdfs:subClassOf RBBO:R9p5Yej3AOqhbZTK2kCgSWX ;
                                       <http://www.geneontology.org/formats/oboInOwl#created_by> "PaulN" ;
                                       <http://www.geneontology.org/formats/oboInOwl#creation_date> "2022-01-26T14:43:10.402244Z" ;
                                       rdfs:label "Rugby" .


###  https://purl.org/turbbo/RBBO_0000024
<https://purl.org/turbbo/RBBO_0000024> rdf:type owl:Class ;
                                       rdfs:subClassOf RBBO:R7MWXGKIGLx4ykI6IfNRWHF ;
                                       <http://www.geneontology.org/formats/oboInOwl#created_by> "PaulN" ;
                                       <http://www.geneontology.org/formats/oboInOwl#creation_date> "2022-01-26T14:45:20.464089Z" ;
                                       rdfs:label "Plagiarism" .


###  https://purl.org/turbbo/RBBO_0000025
<https://purl.org/turbbo/RBBO_0000025> rdf:type owl:Class ;
                                       rdfs:subClassOf RBBO:R7MWXGKIGLx4ykI6IfNRWHF ;
                                       <http://www.geneontology.org/formats/oboInOwl#created_by> "PaulN" ;
                                       <http://www.geneontology.org/formats/oboInOwl#creation_date> "2022-01-26T14:46:21.295611Z" ;
                                       rdfs:label "Homework" .


###  https://purl.org/turbbo/RBBO_0000026
<https://purl.org/turbbo/RBBO_0000026> rdf:type owl:Class ;
                                       rdfs:subClassOf RBBO:R7MWXGKIGLx4ykI6IfNRWHF ;
                                       <http://www.geneontology.org/formats/oboInOwl#created_by> "PaulN" ;
                                       <http://www.geneontology.org/formats/oboInOwl#creation_date> "2022-01-26T14:46:40.961658Z" ;
                                       rdfs:label "Revision" .


###  https://purl.org/turbbo/RBBO_0000027
<https://purl.org/turbbo/RBBO_0000027> rdf:type owl:Class ;
                                       rdfs:subClassOf RBBO:RChrJYRTZRmBDhl2HTuXV4S ;
                                       <http://www.geneontology.org/formats/oboInOwl#created_by> "VyvH" ;
                                       <http://www.geneontology.org/formats/oboInOwl#creation_date> "2022-02-03T20:05:23.359606Z" ;
                                       rdfs:label "Participating in Psychological Intervention" .


###  https://purl.org/turbbo/RBBO_0000028
<https://purl.org/turbbo/RBBO_0000028> rdf:type owl:Class ;
                                       rdfs:subClassOf RBBO:RChrJYRTZRmBDhl2HTuXV4S ;
                                       <http://www.geneontology.org/formats/oboInOwl#created_by> "VyvH" ;
                                       <http://www.geneontology.org/formats/oboInOwl#creation_date> "2022-02-03T20:06:01.004184Z" ;
                                       rdfs:label "Participating in Physical Therapy or Physiotherapy" .


###  https://purl.org/turbbo/RBBO_0000029
<https://purl.org/turbbo/RBBO_0000029> rdf:type owl:Class ;
                                       rdfs:subClassOf RBBO:RDLYuvHGi7xCMFHwL7WJ8pF ;
                                       <http://www.geneontology.org/formats/oboInOwl#created_by> "VyvH" ;
                                       <http://www.geneontology.org/formats/oboInOwl#creation_date> "2022-02-03T20:16:35.132277Z" ;
                                       rdfs:label "Providing practical support" .


###  https://purl.org/turbbo/RBBO_0000030
<https://purl.org/turbbo/RBBO_0000030> rdf:type owl:Class ;
                                       rdfs:subClassOf RBBO:RfZmso8v8XZptVF2vKaUQ3 ;
                                       <http://www.geneontology.org/formats/oboInOwl#created_by> "VyvH" ;
                                       <http://www.geneontology.org/formats/oboInOwl#creation_date> "2022-02-03T20:18:24.244493Z" ;
                                       rdfs:label "Recycling" .


###  https://purl.org/turbbo/RBBO_0000031
<https://purl.org/turbbo/RBBO_0000031> rdf:type owl:Class ;
                                       rdfs:subClassOf RBBO:RfZmso8v8XZptVF2vKaUQ3 ;
                                       <http://www.geneontology.org/formats/oboInOwl#created_by> "VyvH" ;
                                       <http://www.geneontology.org/formats/oboInOwl#creation_date> "2022-02-03T20:19:05.725123Z" ;
                                       rdfs:label "Choosing public transport or active travel" .


###  https://purl.org/turbbo/RBBO_0000032
<https://purl.org/turbbo/RBBO_0000032> rdf:type owl:Class ;
                                       rdfs:subClassOf RBBO:R9JyzynAe7H3xtK0rPOT841 ;
                                       <http://www.geneontology.org/formats/oboInOwl#created_by> "VyvH" ;
                                       <http://www.geneontology.org/formats/oboInOwl#creation_date> "2022-02-03T20:22:08.410702Z" ;
                                       rdfs:label "Participating in neighbourhood watch" .


###  https://purl.org/turbbo/RBBO_0000033
<https://purl.org/turbbo/RBBO_0000033> rdf:type owl:Class ;
                                       rdfs:subClassOf RBBO:RCLGCfCEICjWDiyU2xYotQk ;
                                       <http://www.geneontology.org/formats/oboInOwl#created_by> "VyvH" ;
                                       <http://www.geneontology.org/formats/oboInOwl#creation_date> "2022-02-03T20:23:08.719743Z" ;
                                       rdfs:label "Engaging in business enterprise" .


###  https://purl.org/turbbo/RBBO_0000034
<https://purl.org/turbbo/RBBO_0000034> rdf:type owl:Class ;
                                       rdfs:subClassOf RBBO:RCLGCfCEICjWDiyU2xYotQk ;
                                       <http://www.geneontology.org/formats/oboInOwl#created_by> "VyvH" ;
                                       <http://www.geneontology.org/formats/oboInOwl#creation_date> "2022-02-03T20:23:30.609298Z" ;
                                       rdfs:label "Engaging in volunteering" .


###  https://purl.org/turbbo/RBBO_0000035
<https://purl.org/turbbo/RBBO_0000035> rdf:type owl:Class ;
                                       rdfs:subClassOf RBBO:R7ksLdc5AtNZogZjcdwMAz ;
                                       <http://www.geneontology.org/formats/oboInOwl#created_by> "Harriet Baird" ;
                                       <http://www.geneontology.org/formats/oboInOwl#creation_date> "2022-02-08T09:59:51.664609Z" ;
                                       rdfs:label "Compulsive buying" .


###  https://purl.org/turbbo/RBBO_0000036
<https://purl.org/turbbo/RBBO_0000036> rdf:type owl:Class ;
                                       rdfs:subClassOf RBBO:RDdB56hI5WEz1kELL2HbIdh ;
                                       <http://www.geneontology.org/formats/oboInOwl#created_by> "Harriet Baird" ;
                                       <http://www.geneontology.org/formats/oboInOwl#creation_date> "2022-02-08T10:02:18.524339Z" ;
                                       rdfs:label "Smoking vape" .


###  https://purl.org/turbbo/RBBO_0000037
<https://purl.org/turbbo/RBBO_0000037> rdf:type owl:Class ;
                                       rdfs:subClassOf RBBO:RfZmso8v8XZptVF2vKaUQ3 ;
                                       <http://www.geneontology.org/formats/oboInOwl#created_by> "Harriet Baird" ;
                                       <http://www.geneontology.org/formats/oboInOwl#creation_date> "2022-02-08T10:38:02.831047Z" ;
                                       rdfs:label "Pro-environmental citizenship behaviour" .


###  https://purl.org/turbbo/RBBO_0000038
<https://purl.org/turbbo/RBBO_0000038> rdf:type owl:Class ;
                                       rdfs:subClassOf <https://purl.org/turbbo/RBBO_0000037> ;
                                       <http://www.geneontology.org/formats/oboInOwl#created_by> "Harriet Baird" ;
                                       <http://www.geneontology.org/formats/oboInOwl#creation_date> "2022-02-08T10:39:00.953646Z" ;
                                       rdfs:label "Contributed money towards the protection of the environment" .


###  https://purl.org/turbbo/RBBO_0000039
<https://purl.org/turbbo/RBBO_0000039> rdf:type owl:Class ;
                                       rdfs:subClassOf <https://purl.org/turbbo/RBBO_0000037> ;
                                       <http://www.geneontology.org/formats/oboInOwl#created_by> "Harriet Baird" ;
                                       <http://www.geneontology.org/formats/oboInOwl#creation_date> "2022-02-08T10:39:31.764712Z" ;
                                       rdfs:label "Member of an environmental or conservation protection group" .


###  https://purl.org/turbbo/RBBO_0000040
<https://purl.org/turbbo/RBBO_0000040> rdf:type owl:Class ;
                                       rdfs:subClassOf <https://purl.org/turbbo/RBBO_0000037> ;
                                       <http://www.geneontology.org/formats/oboInOwl#created_by> "Harriet Baird" ;
                                       <http://www.geneontology.org/formats/oboInOwl#creation_date> "2022-02-08T10:40:27.065581Z" ;
                                       rdfs:label "Vote for a political party that supports the environment" .


###  https://purl.org/turbbo/RBBO_0000041
<https://purl.org/turbbo/RBBO_0000041> rdf:type owl:Class ;
                                       rdfs:subClassOf <https://purl.org/turbbo/RBBO_0000037> ;
                                       <http://www.geneontology.org/formats/oboInOwl#created_by> "Harriet Baird" ;
                                       <http://www.geneontology.org/formats/oboInOwl#creation_date> "2022-02-08T10:41:02.477275Z" ;
                                       rdfs:label "Watch programmes about environmental issues" .


###  https://purl.org/turbbo/RBBO_0000042
<https://purl.org/turbbo/RBBO_0000042> rdf:type owl:Class ;
                                       rdfs:subClassOf RBBO:RfZmso8v8XZptVF2vKaUQ3 ;
                                       <http://www.geneontology.org/formats/oboInOwl#created_by> "Harriet Baird" ;
                                       <http://www.geneontology.org/formats/oboInOwl#creation_date> "2022-02-08T10:43:25.686929Z" ;
                                       rdfs:label "Resource conservation behaviour" .


###  https://purl.org/turbbo/RBBO_0000043
<https://purl.org/turbbo/RBBO_0000043> rdf:type owl:Class ;
                                       rdfs:subClassOf <https://purl.org/turbbo/RBBO_0000042> ;
                                       <http://www.geneontology.org/formats/oboInOwl#created_by> "Harriet Baird" ;
                                       <http://www.geneontology.org/formats/oboInOwl#creation_date> "2022-02-08T10:43:42.994468Z" ;
                                       rdfs:label "Conserving electricty" .


###  https://purl.org/turbbo/RBBO_0000044
<https://purl.org/turbbo/RBBO_0000044> rdf:type owl:Class ;
                                       rdfs:subClassOf <https://purl.org/turbbo/RBBO_0000042> ;
                                       <http://www.geneontology.org/formats/oboInOwl#created_by> "Harriet Baird" ;
                                       <http://www.geneontology.org/formats/oboInOwl#creation_date> "2022-02-08T10:44:03.334104Z" ;
                                       rdfs:label "Conserving water" .


###  https://purl.org/turbbo/RBBO_0000045
<https://purl.org/turbbo/RBBO_0000045> rdf:type owl:Class ;
                                       rdfs:subClassOf <https://purl.org/turbbo/RBBO_0000042> ;
                                       <http://www.geneontology.org/formats/oboInOwl#created_by> "Harriet Baird" ;
                                       <http://www.geneontology.org/formats/oboInOwl#creation_date> "2022-02-08T10:44:21.689618Z" ;
                                       rdfs:label "Waste reduction behaviour" .


###  https://purl.org/turbbo/RBBO_0000046
<https://purl.org/turbbo/RBBO_0000046> rdf:type owl:Class ;
                                       rdfs:subClassOf <https://purl.org/turbbo/RBBO_0000043> ;
                                       <http://www.geneontology.org/formats/oboInOwl#created_by> "Harriet Baird" ;
                                       <http://www.geneontology.org/formats/oboInOwl#creation_date> "2022-02-08T10:45:13.32274Z" ;
                                       rdfs:label "Turn the lights off in unoccupied rooms" .


###  https://purl.org/turbbo/RBBO_0000047
<https://purl.org/turbbo/RBBO_0000047> rdf:type owl:Class ;
                                       rdfs:subClassOf <https://purl.org/turbbo/RBBO_0000043> ;
                                       <http://www.geneontology.org/formats/oboInOwl#created_by> "Harriet Baird" ;
                                       <http://www.geneontology.org/formats/oboInOwl#creation_date> "2022-02-08T10:50:37.953177Z" ;
                                       rdfs:label "Unplug appliances that are not being used" .


###  https://purl.org/turbbo/RBBO_0000048
<https://purl.org/turbbo/RBBO_0000048> rdf:type owl:Class ;
                                       rdfs:subClassOf <https://purl.org/turbbo/RBBO_0000043> ;
                                       <http://www.geneontology.org/formats/oboInOwl#created_by> "Harriet Baird" ;
                                       <http://www.geneontology.org/formats/oboInOwl#creation_date> "2022-02-08T10:51:01.998458Z" ;
                                       rdfs:label "Shut your computer down when you are done with it" .


###  https://purl.org/turbbo/RBBO_0000049
<https://purl.org/turbbo/RBBO_0000049> rdf:type owl:Class ;
                                       rdfs:subClassOf <https://purl.org/turbbo/RBBO_0000044> ;
                                       <http://www.geneontology.org/formats/oboInOwl#created_by> "Harriet Baird" ;
                                       <http://www.geneontology.org/formats/oboInOwl#creation_date> "2022-02-08T10:51:37.526514Z" ;
                                       rdfs:label "Turn off the water while brushing your teeth" .


###  https://purl.org/turbbo/RBBO_0000050
<https://purl.org/turbbo/RBBO_0000050> rdf:type owl:Class ;
                                       rdfs:subClassOf <https://purl.org/turbbo/RBBO_0000044> ;
                                       <http://www.geneontology.org/formats/oboInOwl#created_by> "Harriet Baird" ;
                                       <http://www.geneontology.org/formats/oboInOwl#creation_date> "2022-02-08T10:52:16.488951Z" ;
                                       rdfs:label "Turn off the water while shaving" .


###  https://purl.org/turbbo/RBBO_0000051
<https://purl.org/turbbo/RBBO_0000051> rdf:type owl:Class ;
                                       rdfs:subClassOf <https://purl.org/turbbo/RBBO_0000044> ;
                                       <http://www.geneontology.org/formats/oboInOwl#created_by> "Harriet Baird" ;
                                       <http://www.geneontology.org/formats/oboInOwl#creation_date> "2022-02-08T10:52:36.91227Z" ;
                                       rdfs:label "Install water-saving shower heads or flow restrictors." .


###  https://purl.org/turbbo/RBBO_0000052
<https://purl.org/turbbo/RBBO_0000052> rdf:type owl:Class ;
                                       rdfs:subClassOf <https://purl.org/turbbo/RBBO_0000044> ;
                                       <http://www.geneontology.org/formats/oboInOwl#created_by> "Harriet Baird" ;
                                       <http://www.geneontology.org/formats/oboInOwl#creation_date> "2022-02-08T10:54:44.485866Z" ;
                                       rdfs:label "Take shorter showers" .


###  https://purl.org/turbbo/RBBO_0000053
<https://purl.org/turbbo/RBBO_0000053> rdf:type owl:Class ;
                                       rdfs:subClassOf <https://purl.org/turbbo/RBBO_0000045> ;
                                       <http://www.geneontology.org/formats/oboInOwl#created_by> "Harriet Baird" ;
                                       <http://www.geneontology.org/formats/oboInOwl#creation_date> "2022-02-08T10:55:46.187703Z" ;
                                       rdfs:label "Buy packaging-free products and produce" .


###  https://purl.org/turbbo/RBBO_0000054
<https://purl.org/turbbo/RBBO_0000054> rdf:type owl:Class ;
                                       rdfs:subClassOf <https://purl.org/turbbo/RBBO_0000045> ;
                                       <http://www.geneontology.org/formats/oboInOwl#created_by> "Harriet Baird" ;
                                       <http://www.geneontology.org/formats/oboInOwl#creation_date> "2022-02-08T10:56:23.90163Z" ;
                                       rdfs:label "Recycling of object or material" .


###  https://purl.org/turbbo/RBBO_0000055
<https://purl.org/turbbo/RBBO_0000055> rdf:type owl:Class ;
                                       rdfs:subClassOf <https://purl.org/turbbo/RBBO_0000045> ;
                                       <http://www.geneontology.org/formats/oboInOwl#created_by> "Harriet Baird" ;
                                       <http://www.geneontology.org/formats/oboInOwl#creation_date> "2022-02-08T10:56:51.09235Z" ;
                                       rdfs:label "Reuse object of material" .


###  https://purl.org/turbbo/RBBO_0000056
<https://purl.org/turbbo/RBBO_0000056> rdf:type owl:Class ;
                                       rdfs:subClassOf <https://purl.org/turbbo/RBBO_0000055> ;
                                       <http://www.geneontology.org/formats/oboInOwl#created_by> "Harriet Baird" ;
                                       <http://www.geneontology.org/formats/oboInOwl#creation_date> "2022-02-08T10:58:32.00747Z" ;
                                       rdfs:label "Refill" .


###  https://purl.org/turbbo/RBBO_0000057
<https://purl.org/turbbo/RBBO_0000057> rdf:type owl:Class ;
                                       rdfs:subClassOf <https://purl.org/turbbo/RBBO_0000055> ;
                                       <http://www.geneontology.org/formats/oboInOwl#created_by> "Harriet Baird" ;
                                       <http://www.geneontology.org/formats/oboInOwl#creation_date> "2022-02-08T10:58:38.659298Z" ;
                                       rdfs:label "Return" .


###  https://purl.org/turbbo/RBBO_0000058
<https://purl.org/turbbo/RBBO_0000058> rdf:type owl:Class ;
                                       rdfs:subClassOf RBBO:RfZmso8v8XZptVF2vKaUQ3 ;
                                       <http://www.geneontology.org/formats/oboInOwl#created_by> "Harriet Baird" ;
                                       <http://www.geneontology.org/formats/oboInOwl#creation_date> "2022-02-08T10:59:48.748553Z" ;
                                       rdfs:label "Sustainable eating behaviour" .


###  https://purl.org/turbbo/RBBO_0000059
<https://purl.org/turbbo/RBBO_0000059> rdf:type owl:Class ;
                                       rdfs:subClassOf <https://purl.org/turbbo/RBBO_0000058> ;
                                       <http://www.geneontology.org/formats/oboInOwl#created_by> "Harriet Baird" ;
                                       <http://www.geneontology.org/formats/oboInOwl#creation_date> "2022-02-08T11:00:39.748047Z" ;
                                       rdfs:label "Buying/ consuming seasonal produce" .


###  https://purl.org/turbbo/RBBO_0000060
<https://purl.org/turbbo/RBBO_0000060> rdf:type owl:Class ;
                                       rdfs:subClassOf <https://purl.org/turbbo/RBBO_0000058> ;
                                       <http://www.geneontology.org/formats/oboInOwl#created_by> "Harriet Baird" ;
                                       <http://www.geneontology.org/formats/oboInOwl#creation_date> "2022-02-08T11:00:57.654103Z" ;
                                       rdfs:label "Buying/ eating less meat" .


###  https://purl.org/turbbo/RBBO_0000061
<https://purl.org/turbbo/RBBO_0000061> rdf:type owl:Class ;
                                       rdfs:subClassOf <https://purl.org/turbbo/RBBO_0000058> ;
                                       <http://www.geneontology.org/formats/oboInOwl#created_by> "Harriet Baird" ;
                                       <http://www.geneontology.org/formats/oboInOwl#creation_date> "2022-02-08T11:02:32.451414Z" ;
                                       rdfs:label "Increasing consumption of plant-based foods" .


###  https://purl.org/turbbo/RBBO_0000062
<https://purl.org/turbbo/RBBO_0000062> rdf:type owl:Class ;
                                       rdfs:subClassOf RBBO:R9cWGdaP36P9kM5hHEPRMHg ;
                                       <http://www.geneontology.org/formats/oboInOwl#created_by> "Harriet Baird" ;
                                       <http://www.geneontology.org/formats/oboInOwl#creation_date> "2022-02-08T11:11:58.930086Z" ;
                                       rdfs:label "Washing body parts" .


###  https://purl.org/turbbo/RBBO_0000063
<https://purl.org/turbbo/RBBO_0000063> rdf:type owl:Class ;
                                       rdfs:subClassOf RBBO:R9cWGdaP36P9kM5hHEPRMHg ;
                                       <http://www.geneontology.org/formats/oboInOwl#created_by> "Harriet Baird" ;
                                       <http://www.geneontology.org/formats/oboInOwl#creation_date> "2022-02-08T11:12:25.753689Z" ;
                                       rdfs:label "Washing whole body" .


###  https://purl.org/turbbo/RBBO_0000064
<https://purl.org/turbbo/RBBO_0000064> rdf:type owl:Class ;
                                       rdfs:subClassOf RBBO:R9cWGdaP36P9kM5hHEPRMHg ;
                                       <http://www.geneontology.org/formats/oboInOwl#created_by> "Harriet Baird" ;
                                       <http://www.geneontology.org/formats/oboInOwl#creation_date> "2022-02-08T11:12:47.009781Z" ;
                                       rdfs:label "Drying oneself" .


###  https://purl.org/turbbo/RBBO_0000065
<https://purl.org/turbbo/RBBO_0000065> rdf:type owl:Class ;
                                       rdfs:subClassOf RBBO:R3NO3LpXB5rQZlwHyBqraH ;
                                       <http://www.geneontology.org/formats/oboInOwl#created_by> "Harriet Baird" ;
                                       <http://www.geneontology.org/formats/oboInOwl#creation_date> "2022-02-08T11:20:54.183513Z" ;
                                       rdfs:label "Washing and drying clothes and garments" .


###  https://purl.org/turbbo/RBBO_0000066
<https://purl.org/turbbo/RBBO_0000066> rdf:type owl:Class ;
                                       rdfs:subClassOf RBBO:R3NO3LpXB5rQZlwHyBqraH ;
                                       <http://www.geneontology.org/formats/oboInOwl#created_by> "Harriet Baird" ;
                                       <http://www.geneontology.org/formats/oboInOwl#creation_date> "2022-02-08T11:21:25.441626Z" ;
                                       rdfs:label "Disposing of rubbish/ garbage" .


###  https://purl.org/turbbo/RBBO_0000067
<https://purl.org/turbbo/RBBO_0000067> rdf:type owl:Class ;
                                       rdfs:subClassOf RBBO:RCV0qw9GIXO9nA6mEsE72Nr ;
                                       <http://www.geneontology.org/formats/oboInOwl#created_by> "Harriet Baird" ;
                                       <http://www.geneontology.org/formats/oboInOwl#creation_date> "2022-02-08T11:24:58.576958Z" ;
                                       rdfs:label "Acquisition of necessities" .


###  https://purl.org/turbbo/RBBO_0000068
<https://purl.org/turbbo/RBBO_0000068> rdf:type owl:Class ;
                                       rdfs:subClassOf <https://purl.org/turbbo/RBBO_0000067> ;
                                       <http://www.geneontology.org/formats/oboInOwl#created_by> "Harriet Baird" ;
                                       <http://www.geneontology.org/formats/oboInOwl#creation_date> "2022-02-08T11:26:00.362232Z" ;
                                       rdfs:label "Acquiring a place to live" .


###  https://purl.org/turbbo/RBBO_0000069
<https://purl.org/turbbo/RBBO_0000069> rdf:type owl:Class ;
                                       rdfs:subClassOf <https://purl.org/turbbo/RBBO_0000068> ;
                                       <http://www.geneontology.org/formats/oboInOwl#created_by> "Harriet Baird" ;
                                       <http://www.geneontology.org/formats/oboInOwl#creation_date> "2022-02-08T11:26:25.404973Z" ;
                                       rdfs:label "Buying a place to live" .


###  https://purl.org/turbbo/RBBO_0000070
<https://purl.org/turbbo/RBBO_0000070> rdf:type owl:Class ;
                                       rdfs:subClassOf <https://purl.org/turbbo/RBBO_0000068> ;
                                       <http://www.geneontology.org/formats/oboInOwl#created_by> "Harriet Baird" ;
                                       <http://www.geneontology.org/formats/oboInOwl#creation_date> "2022-02-08T11:26:36.992686Z" ;
                                       rdfs:label "Renting a place to live" .


###  https://purl.org/turbbo/RBBO_0000071
<https://purl.org/turbbo/RBBO_0000071> rdf:type owl:Class ;
                                       rdfs:subClassOf <https://purl.org/turbbo/RBBO_0000068> ;
                                       <http://www.geneontology.org/formats/oboInOwl#created_by> "Harriet Baird" ;
                                       <http://www.geneontology.org/formats/oboInOwl#creation_date> "2022-02-08T11:27:01.399847Z" ;
                                       rdfs:label "Furnishing a place to live" .


###  https://purl.org/turbbo/RBBO_0000072
<https://purl.org/turbbo/RBBO_0000072> rdf:type owl:Class ;
                                       rdfs:subClassOf <https://purl.org/turbbo/RBBO_0000076> ;
                                       <http://www.geneontology.org/formats/oboInOwl#created_by> "Harriet Baird" ;
                                       <http://www.geneontology.org/formats/oboInOwl#creation_date> "2022-02-08T11:27:52.364594Z" ;
                                       rdfs:label "Shopping" .


###  https://purl.org/turbbo/RBBO_0000073
<https://purl.org/turbbo/RBBO_0000073> rdf:type owl:Class ;
                                       rdfs:subClassOf <https://purl.org/turbbo/RBBO_0000072> ;
                                       <http://www.geneontology.org/formats/oboInOwl#created_by> "Harriet Baird" ;
                                       <http://www.geneontology.org/formats/oboInOwl#creation_date> "2022-02-08T11:29:03.73736Z" ;
                                       rdfs:label "Shopping for groceries" .


###  https://purl.org/turbbo/RBBO_0000074
<https://purl.org/turbbo/RBBO_0000074> rdf:type owl:Class ;
                                       rdfs:subClassOf RBBO:R3NO3LpXB5rQZlwHyBqraH ;
                                       <http://www.geneontology.org/formats/oboInOwl#created_by> "Harriet Baird" ;
                                       <http://www.geneontology.org/formats/oboInOwl#creation_date> "2022-02-08T11:29:42.499573Z" ;
                                       rdfs:label "Using household appliances" .


###  https://purl.org/turbbo/RBBO_0000075
<https://purl.org/turbbo/RBBO_0000075> rdf:type owl:Class ;
                                       rdfs:subClassOf RBBO:R3NO3LpXB5rQZlwHyBqraH ;
                                       <http://www.geneontology.org/formats/oboInOwl#created_by> "Harriet Baird" ;
                                       <http://www.geneontology.org/formats/oboInOwl#creation_date> "2022-02-08T11:30:14.793475Z" ;
                                       rdfs:label "Storing daily necessities" .


###  https://purl.org/turbbo/RBBO_0000076
<https://purl.org/turbbo/RBBO_0000076> rdf:type owl:Class ;
                                       rdfs:subClassOf <https://purl.org/turbbo/RBBO_0000067> ;
                                       <http://www.geneontology.org/formats/oboInOwl#created_by> "Harriet Baird" ;
                                       <http://www.geneontology.org/formats/oboInOwl#creation_date> "2022-02-08T11:35:39.114809Z" ;
                                       rdfs:label "Acquisition of goods and services" .


###  https://purl.org/turbbo/RBBO_0000077
<https://purl.org/turbbo/RBBO_0000077> rdf:type owl:Class ;
                                       rdfs:subClassOf <https://purl.org/turbbo/RBBO_0000076> ;
                                       <http://www.geneontology.org/formats/oboInOwl#created_by> "Harriet Baird" ;
                                       <http://www.geneontology.org/formats/oboInOwl#creation_date> "2022-02-08T11:36:36.263811Z" ;
                                       rdfs:label "Gathering daily necessities" .


###  https://purl.org/turbbo/RBBO_0000078
<https://purl.org/turbbo/RBBO_0000078> rdf:type owl:Class ;
                                       rdfs:subClassOf RBBO:RCgGDn1vqlfJSIRaFveJ3LD ;
                                       <http://www.geneontology.org/formats/oboInOwl#created_by> "Harriet Baird" ;
                                       <http://www.geneontology.org/formats/oboInOwl#creation_date> "2022-02-08T11:41:09.878041Z" ;
                                       rdfs:label "Use of contraceptive coil (IUD)" .


###  https://purl.org/turbbo/RBBO_0000079
<https://purl.org/turbbo/RBBO_0000079> rdf:type owl:Class ;
                                       rdfs:subClassOf RBBO:RCE7VvM7rpyKfsBJxKqHVvk ;
                                       <http://www.geneontology.org/formats/oboInOwl#created_by> "Harriet Baird" ;
                                       <http://www.geneontology.org/formats/oboInOwl#creation_date> "2022-02-08T11:42:14.65479Z" ;
                                       rdfs:label "Speaking to adult" .


###  https://purl.org/turbbo/RBBO_0000080
<https://purl.org/turbbo/RBBO_0000080> rdf:type owl:Class ;
                                       rdfs:subClassOf RBBO:R8qMM1AUIWkGs9uIR3zf0Oe ;
                                       <http://www.geneontology.org/formats/oboInOwl#created_by> "Harriet Baird" ;
                                       <http://www.geneontology.org/formats/oboInOwl#creation_date> "2022-02-08T11:45:03.091158Z" ;
                                       rdfs:label "Meditation" .


###  https://purl.org/turbbo/RBBO_0000081
<https://purl.org/turbbo/RBBO_0000081> rdf:type owl:Class ;
                                       rdfs:subClassOf RBBO:RC49XywX1UPXtJYddxnrb0h ;
                                       <http://www.geneontology.org/formats/oboInOwl#created_by> "Harriet Baird" ;
                                       <http://www.geneontology.org/formats/oboInOwl#creation_date> "2022-02-08T12:15:42.483576Z" ;
                                       rdfs:label "Problematic internet use" .


###  https://purl.org/turbbo/RBBO_0000082
<https://purl.org/turbbo/RBBO_0000082> rdf:type owl:Class ;
                                       rdfs:subClassOf RBBO:RDzsFgl9xnDJkw9zXLWULAv ;
                                       <http://www.geneontology.org/formats/oboInOwl#created_by> "Harriet Baird" ;
                                       <http://www.geneontology.org/formats/oboInOwl#creation_date> "2022-02-08T12:18:34.004071Z" ;
                                       rdfs:label "Using smartphones" .


###  https://purl.org/turbbo/RBBO_0000083
<https://purl.org/turbbo/RBBO_0000083> rdf:type owl:Class ;
                                       rdfs:subClassOf RBBO:R9BeiQh4oa8EbuNm1bjryZB ;
                                       <http://www.geneontology.org/formats/oboInOwl#created_by> "Harriet Baird" ;
                                       <http://www.geneontology.org/formats/oboInOwl#creation_date> "2022-02-08T12:19:45.6605Z" ;
                                       rdfs:label "Attending a job interview" .


###  https://purl.org/turbbo/RBBO_0000084
<https://purl.org/turbbo/RBBO_0000084> rdf:type owl:Class ;
                                       rdfs:subClassOf RBBO:R9SZhlXBAdyrsI5ItrSRZDG ;
                                       <http://www.geneontology.org/formats/oboInOwl#created_by> "Harriet Baird" ;
                                       <http://www.geneontology.org/formats/oboInOwl#creation_date> "2022-02-08T12:36:42.676528Z" ;
                                       rdfs:label "Using head protection (e.g., helmet)" .


###  https://purl.org/turbbo/RBBO_0000085
<https://purl.org/turbbo/RBBO_0000085> rdf:type owl:Class ;
                                       rdfs:subClassOf RBBO:RCrDL1h6RMXEqgnkTmAzyNh ;
                                       <http://www.geneontology.org/formats/oboInOwl#created_by> "Harriet Baird" ;
                                       <http://www.geneontology.org/formats/oboInOwl#creation_date> "2022-02-08T12:37:23.529202Z" ;
                                       rdfs:label "Wearing a seatbelt" .


###  https://purl.org/turbbo/RBBO_0000086
<https://purl.org/turbbo/RBBO_0000086> rdf:type owl:Class ;
                                       rdfs:subClassOf RBBO:R7SqDxfmXPDIUSZShgwaIyO ;
                                       <http://www.geneontology.org/formats/oboInOwl#created_by> "Harriet Baird" ;
                                       <http://www.geneontology.org/formats/oboInOwl#creation_date> "2022-02-08T12:41:02.147857Z" ;
                                       rdfs:label "Participation in clinical screening" .


###  https://purl.org/turbbo/RBBO_0000087
<https://purl.org/turbbo/RBBO_0000087> rdf:type owl:Class ;
                                       rdfs:subClassOf <https://purl.org/turbbo/RBBO_0000090> ;
                                       <http://www.geneontology.org/formats/oboInOwl#created_by> "Harriet Baird" ;
                                       <http://www.geneontology.org/formats/oboInOwl#creation_date> "2022-02-08T12:41:40.409636Z" ;
                                       rdfs:label "Participation in mammography screening" .


###  https://purl.org/turbbo/RBBO_0000088
<https://purl.org/turbbo/RBBO_0000088> rdf:type owl:Class ;
                                       rdfs:subClassOf <https://purl.org/turbbo/RBBO_0000090> ;
                                       <http://www.geneontology.org/formats/oboInOwl#created_by> "Harriet Baird" ;
                                       <http://www.geneontology.org/formats/oboInOwl#creation_date> "2022-02-08T12:42:34.21415Z" ;
                                       rdfs:label "Participation in cervical screening (a smear test)" .


###  https://purl.org/turbbo/RBBO_0000089
<https://purl.org/turbbo/RBBO_0000089> rdf:type owl:Class ;
                                       rdfs:subClassOf <https://purl.org/turbbo/RBBO_0000090> ;
                                       <http://www.geneontology.org/formats/oboInOwl#created_by> "Harriet Baird" ;
                                       <http://www.geneontology.org/formats/oboInOwl#creation_date> "2022-02-08T12:43:48.834471Z" ;
                                       rdfs:label "Participation in colorectal (bowel) cancer screening" .


###  https://purl.org/turbbo/RBBO_0000090
<https://purl.org/turbbo/RBBO_0000090> rdf:type owl:Class ;
                                       rdfs:subClassOf <https://purl.org/turbbo/RBBO_0000086> ;
                                       <http://www.geneontology.org/formats/oboInOwl#created_by> "Harriet Baird" ;
                                       <http://www.geneontology.org/formats/oboInOwl#creation_date> "2022-02-08T12:44:11.824668Z" ;
                                       rdfs:label "Participation in cancer screening" .


###  https://purl.org/turbbo/RBBO_0000091
<https://purl.org/turbbo/RBBO_0000091> rdf:type owl:Class ;
                                       rdfs:subClassOf <https://purl.org/turbbo/RBBO_0000086> ;
                                       <http://www.geneontology.org/formats/oboInOwl#created_by> "Harriet Baird" ;
                                       <http://www.geneontology.org/formats/oboInOwl#creation_date> "2022-02-08T12:45:07.775383Z" ;
                                       rdfs:label "Participation in diabetes screening" .


###  https://purl.org/turbbo/RBBO_0000092
<https://purl.org/turbbo/RBBO_0000092> rdf:type owl:Class ;
                                       rdfs:subClassOf <https://purl.org/turbbo/RBBO_0000086> ;
                                       <http://www.geneontology.org/formats/oboInOwl#created_by> "Harriet Baird" ;
                                       <http://www.geneontology.org/formats/oboInOwl#creation_date> "2022-02-08T12:45:43.719426Z" ;
                                       rdfs:label "Participation in hypertension screening" .


###  https://purl.org/turbbo/RBBO_0000123
<https://purl.org/turbbo/RBBO_0000123> rdf:type owl:Class ;
                                       rdfs:label "Behaviour" ;
                                       rdfs:seeAlso "Engaging in activities/ participating from IC-Behavior taxonomy" ;
                                       <http://www.w3.org/2004/02/skos/core#definition> "The condition in which things are happening or being done and/or the action of taking part in something." .


###  https://purl.org/turbbo/RBBO_R2u7u2nNFoKuQMcA3z3YG7
RBBO:R2u7u2nNFoKuQMcA3z3YG7 rdf:type owl:Class ;
                            rdfs:subClassOf RBBO:RDarCRBoiqojsnZ9V6Oj1EU ;
                            rdfs:label "Resting" ;
                            <http://www.w3.org/2004/02/skos/core#definition> "The act of ceasing work or movement in order to relax, refresh oneself, or recover strength." .


###  https://purl.org/turbbo/RBBO_R3GTM1WIfB3LofIOVpVVKU
RBBO:R3GTM1WIfB3LofIOVpVVKU rdf:type owl:Class ;
                            rdfs:subClassOf RBBO:RBuoEsSFBhOGJtFyQKJv3yx ;
                            rdfs:label "Sustenance ingesting" ;
                            <http://www.w3.org/2004/02/skos/core#definition> "Nourishment" .


###  https://purl.org/turbbo/RBBO_R3HIEV4Q60XlmRBVPFyaEZ
RBBO:R3HIEV4Q60XlmRBVPFyaEZ rdf:type owl:Class ;
                            rdfs:subClassOf RBBO:RCMQ2Xe8y2ROsQ2JODi10Pt ;
                            rdfs:label "Gardening" ;
                            <http://www.w3.org/2004/02/skos/core#definition> "The activity of tending and cultivating a garden." .


###  https://purl.org/turbbo/RBBO_R3NO3LpXB5rQZlwHyBqraH
RBBO:R3NO3LpXB5rQZlwHyBqraH rdf:type owl:Class ;
                            rdfs:subClassOf RBBO:RCV0qw9GIXO9nA6mEsE72Nr ;
                            rdfs:label "Doing housework" ;
                            <http://www.w3.org/2004/02/skos/core#definition> "The act of engaging in housekeeping" .


###  https://purl.org/turbbo/RBBO_R43WF6rp1q7dXrSPS9Ds7q
RBBO:R43WF6rp1q7dXrSPS9Ds7q rdf:type owl:Class ;
                            rdfs:subClassOf RBBO:Rb1xX794wVt3QQownZtSbO ;
                            rdfs:label "Attending Sports event" ;
                            <http://www.w3.org/2004/02/skos/core#definition> "Attending a planned occasion or activity focused on a sport." .


###  https://purl.org/turbbo/RBBO_R539h7zNDyqiNOlv41H9Pu
RBBO:R539h7zNDyqiNOlv41H9Pu rdf:type owl:Class ;
                            rdfs:subClassOf RBBO:RCKDQM6dfhit3RC352IGkgN ;
                            rdfs:label "Using Anabolic steroids" ;
                            <http://www.w3.org/2004/02/skos/core#definition> "The use of synthetic steroid hormones that resemble testosterone in promoting the growth of muscle" .


###  https://purl.org/turbbo/RBBO_R6I0RnK1viksUAXzK4gU5G
RBBO:R6I0RnK1viksUAXzK4gU5G rdf:type owl:Class ;
                            rdfs:subClassOf RBBO:R74Nph6Q96RGCllk8UMt94p ;
                            rdfs:label "Toothbrushing" ;
                            <http://www.w3.org/2004/02/skos/core#definition> "The action of using a toothbrush to clean the teeth." .


###  https://purl.org/turbbo/RBBO_R6hKctZFZcjKJBLZwC7y9T
RBBO:R6hKctZFZcjKJBLZwC7y9T rdf:type owl:Class ;
                            rdfs:subClassOf <https://purl.org/turbbo/RBBO_0000123> ;
                            rdfs:label "Communicating" ;
                            <http://www.w3.org/2004/02/skos/core#definition> "The act or process of using words, sounds, signs, or behaviors to express or exchange information or to express your ideas, thoughts, feelings, etc., to someone else." .


###  https://purl.org/turbbo/RBBO_R71V3Og38WQ7O96qyXLbX1m
RBBO:R71V3Og38WQ7O96qyXLbX1m rdf:type owl:Class ;
                             rdfs:subClassOf RBBO:RBZBFZG9PRFJpm31aToI1nl ;
                             rdfs:label "Having anal intercourse" ;
                             <http://www.w3.org/2004/02/skos/core#definition> "Sexual activity in which a person puts a natural or artificial penis into the anus of another." .


###  https://purl.org/turbbo/RBBO_R72ZXu52sC4SgJQPCbndepq
RBBO:R72ZXu52sC4SgJQPCbndepq rdf:type owl:Class ;
                             rdfs:subClassOf RBBO:RDqjiSX08Nc9xxSBrR5KMOM ;
                             rdfs:label "Writing" ;
                             <http://www.w3.org/2004/02/skos/core#definition> "The activity of composing text" .


###  https://purl.org/turbbo/RBBO_R73ScJd5f9k7m9Hd2ZERZPu
RBBO:R73ScJd5f9k7m9Hd2ZERZPu rdf:type owl:Class ;
                             rdfs:subClassOf RBBO:RCgGDn1vqlfJSIRaFveJ3LD ;
                             rdfs:label "Using condom" ;
                             <http://www.w3.org/2004/02/skos/core#definition> """Use of a sheath commonly of rubber worn over the penis (as to prevent conception or venereal infection during coitus) or a
device that is designed to be inserted into the vagina before coitus and that resembles in form and function the condom used by males.""" .


###  https://purl.org/turbbo/RBBO_R74Nph6Q96RGCllk8UMt94p
RBBO:R74Nph6Q96RGCllk8UMt94p rdf:type owl:Class ;
                             rdfs:subClassOf RBBO:RBuoEsSFBhOGJtFyQKJv3yx ;
                             rdfs:label "Caring for body parts/Personal hygiene" ;
                             <http://www.w3.org/2004/02/skos/core#definition> "The act of caring for body parts in order to ensure what is needed for their health or protection." .


###  https://purl.org/turbbo/RBBO_R7AM7ERYzGdFt5E71E8cIsG
RBBO:R7AM7ERYzGdFt5E71E8cIsG rdf:type owl:Class ;
                             rdfs:subClassOf RBBO:R8qMM1AUIWkGs9uIR3zf0Oe ;
                             rdfs:label "Praying" ;
                             <http://www.w3.org/2004/02/skos/core#definition> "The act of speaking to God especially in order to give thanks or to ask for something." .


###  https://purl.org/turbbo/RBBO_R7KumE46mwzHlQIlcwwADBI
RBBO:R7KumE46mwzHlQIlcwwADBI rdf:type owl:Class ;
                             rdfs:subClassOf RBBO:R3GTM1WIfB3LofIOVpVVKU ;
                             rdfs:label "Ingesting Vitamins" ;
                             <http://www.w3.org/2004/02/skos/core#definition> "Ingesting a group of organic food substances found in animals and plants in small quantities. They must be supplied in diet or dietary supplement and are essential for normal metabolism." .


###  https://purl.org/turbbo/RBBO_R7LFMgbt35Cfkx42ektsTEV
RBBO:R7LFMgbt35Cfkx42ektsTEV rdf:type owl:Class ;
                             rdfs:subClassOf RBBO:RC5cLYrHZhVyinK9OLpz4Ax ;
                             rdfs:label "Engaging in antisocial behavior" ;
                             <http://www.w3.org/2004/02/skos/core#definition> "Behaviors that harm or lack consideration for the well-being of others and/or break laws." .


###  https://purl.org/turbbo/RBBO_R7LgTiHQ8HpEgALLRG0j5ai
RBBO:R7LgTiHQ8HpEgALLRG0j5ai rdf:type owl:Class ;
                             rdfs:subClassOf RBBO:R7MWXGKIGLx4ykI6IfNRWHF ;
                             rdfs:label "Quitting school" ;
                             <http://www.w3.org/2004/02/skos/core#definition> "Leave school, usually permanently" .


###  https://purl.org/turbbo/RBBO_R7MWXGKIGLx4ykI6IfNRWHF
RBBO:R7MWXGKIGLx4ykI6IfNRWHF rdf:type owl:Class ;
                             rdfs:subClassOf RBBO:RCLGCfCEICjWDiyU2xYotQk ;
                             rdfs:label "Engaging in formal education" ;
                             <http://www.w3.org/2004/02/skos/core#definition> "Giving systematic instruction, at a school or university." .


###  https://purl.org/turbbo/RBBO_R7MZNxsxrHJFsQZe0BlH2P4
RBBO:R7MZNxsxrHJFsQZe0BlH2P4 rdf:type owl:Class ;
                             rdfs:subClassOf RBBO:RC5cLYrHZhVyinK9OLpz4Ax ;
                             rdfs:label "Engaging in behavior related to political life and citizenship" ;
                             <http://www.w3.org/2004/02/skos/core#definition> "Engaging in activities related to be a responsible member of a community and/ or to politcal parties (Public Service Employment Act, adapted)" .


###  https://purl.org/turbbo/RBBO_R7S8d4JYYCiTv7gJUzvecVp
RBBO:R7S8d4JYYCiTv7gJUzvecVp rdf:type owl:Class ;
                             rdfs:subClassOf RBBO:RDw1Q66ue2imTNF7lazEvKw ;
                             rdfs:label "Using a weapon on a person" ;
                             <http://www.w3.org/2004/02/skos/core#definition> "The act of using something to injure, defeat, or destroy on another." .


###  https://purl.org/turbbo/RBBO_R7SqDxfmXPDIUSZShgwaIyO
RBBO:R7SqDxfmXPDIUSZShgwaIyO rdf:type owl:Class ;
                             rdfs:subClassOf RBBO:R7x8NHLRGEcEymTXMx3THX7 ;
                             rdfs:label "Doing a clinical screening or test" ;
                             <http://www.w3.org/2004/02/skos/core#definition> "The act of participating in a systematic clinical examination or assessment." .


###  https://purl.org/turbbo/RBBO_R7Tk1H3NwuI0LdQOy7iFLUD
RBBO:R7Tk1H3NwuI0LdQOy7iFLUD rdf:type owl:Class ;
                             rdfs:subClassOf RBBO:R7uK2tMCWgORKYlpKazgtMt ;
                             rdfs:label "Eating Fast food" ;
                             <http://www.w3.org/2004/02/skos/core#definition> "The consumption of easily prepared food served in restaurants and snack bars as a quick meal or to be taken out." .


###  https://purl.org/turbbo/RBBO_R7XCC5zU34bLOestUwQWuuR
RBBO:R7XCC5zU34bLOestUwQWuuR rdf:type owl:Class ;
                             rdfs:subClassOf RBBO:R7qzqygnfKwMVxUR9f0qbNZ ;
                             rdfs:label "Drinking Milk" ;
                             <http://www.w3.org/2004/02/skos/core#definition> "Consumption of an opaque white fluid rich in fat and protein, secreted by female mammals for the nourishment of their young." .


###  https://purl.org/turbbo/RBBO_R7Yf7M0MxZ4q5ZlV3ns67lq
RBBO:R7Yf7M0MxZ4q5ZlV3ns67lq rdf:type owl:Class ;
                             rdfs:subClassOf RBBO:RBZBFZG9PRFJpm31aToI1nl ;
                             rdfs:label "Having vaginal intercourse" ;
                             <http://www.w3.org/2004/02/skos/core#definition> "Sexual activity in which a person puts a natural or artificial penis into the vagina of a woman." .


###  https://purl.org/turbbo/RBBO_R7cCPkS4EJPnAqfRaMu79xf
RBBO:R7cCPkS4EJPnAqfRaMu79xf rdf:type owl:Class ;
                             rdfs:subClassOf RBBO:R7MZNxsxrHJFsQZe0BlH2P4 ;
                             rdfs:label "Engaging in political activism" ;
                             <http://www.w3.org/2004/02/skos/core#definition> "The use of vigorous campaigning to bring about political change." .


###  https://purl.org/turbbo/RBBO_R7kHdkMUTa5gaJcK3oko65F
RBBO:R7kHdkMUTa5gaJcK3oko65F rdf:type owl:Class ;
                             rdfs:subClassOf RBBO:RCV0qw9GIXO9nA6mEsE72Nr ;
                             rdfs:label "Preparing meals" ;
                             <http://www.w3.org/2004/02/skos/core#definition> "The practice or skill of preparing food by combining, mixing, and heating ingredients." .


###  https://purl.org/turbbo/RBBO_R7ksLdc5AtNZogZjcdwMAz
RBBO:R7ksLdc5AtNZogZjcdwMAz rdf:type owl:Class ;
                            rdfs:subClassOf RBBO:RhlslZKl21SGb8L452uSU8 ;
                            rdfs:label "Spending" ;
                            <http://www.w3.org/2004/02/skos/core#definition> "The act of using an accepted method of payment to pay for something else." .


###  https://purl.org/turbbo/RBBO_R7ou7HEwYODwmkHhLtEqW2B
RBBO:R7ou7HEwYODwmkHhLtEqW2B rdf:type owl:Class ;
                             rdfs:subClassOf <https://purl.org/turbbo/RBBO_0000123> ;
                             rdfs:label "Moving/ Exercising" ;
                             <http://www.w3.org/2004/02/skos/core#definition> "To change position or make one´s body change position in a way that can be seen, heard or felt; physical activity that someone does to stay healthy or become stronger." .


###  https://purl.org/turbbo/RBBO_R7pSWXD6d3tkoGLH56hjASm
RBBO:R7pSWXD6d3tkoGLH56hjASm rdf:type owl:Class ;
                             rdfs:subClassOf RBBO:R7cCPkS4EJPnAqfRaMu79xf ;
                             rdfs:label "Engaging in protest" ;
                             <http://www.w3.org/2004/02/skos/core#definition> "Engaging in \"a compaint, objection, or display of unwillingess usually to an idea or a course of action." .


###  https://purl.org/turbbo/RBBO_R7qzqygnfKwMVxUR9f0qbNZ
RBBO:R7qzqygnfKwMVxUR9f0qbNZ rdf:type owl:Class ;
                             rdfs:subClassOf RBBO:R3GTM1WIfB3LofIOVpVVKU ;
                             rdfs:label "Drinking" ;
                             <http://www.w3.org/2004/02/skos/core#definition> "To take a liquid into your mouth and swallow it." .


###  https://purl.org/turbbo/RBBO_R7u1DYQZbK5g35P4fpskShU
RBBO:R7u1DYQZbK5g35P4fpskShU rdf:type owl:Class ;
                             rdfs:subClassOf RBBO:RayAVAeF9vXpz9v3jwSLzs ;
                             rdfs:label "Sabotaging" ;
                             <http://www.w3.org/2004/02/skos/core#definition> "Engaging in an act of deliberate subversion." .


###  https://purl.org/turbbo/RBBO_R7uK2tMCWgORKYlpKazgtMt
RBBO:R7uK2tMCWgORKYlpKazgtMt rdf:type owl:Class ;
                             rdfs:subClassOf RBBO:R3GTM1WIfB3LofIOVpVVKU ;
                             rdfs:label "Eating" ;
                             <http://www.w3.org/2004/02/skos/core#definition> "Put (food) into the mouth and chew and swallow it." .


###  https://purl.org/turbbo/RBBO_R7v3PZTiUBVbqoDi5fN07Xy
RBBO:R7v3PZTiUBVbqoDi5fN07Xy rdf:type owl:Class ;
                             rdfs:subClassOf RBBO:R3GTM1WIfB3LofIOVpVVKU ;
                             rdfs:label "Ingesting Fiber" ;
                             <http://www.w3.org/2004/02/skos/core#definition> "Ingesting mostly indigestible material in food that stimulates the intestine to peristalsis — called also bulk, roughage." .


###  https://purl.org/turbbo/RBBO_R7vxYwxQyKBDRKzRKRAgsTc
RBBO:R7vxYwxQyKBDRKzRKRAgsTc rdf:type owl:Class ;
                             rdfs:subClassOf RBBO:RCKDQM6dfhit3RC352IGkgN ;
                             rdfs:label "Abstaining" ;
                             <http://www.w3.org/2004/02/skos/core#definition> "Restraining oneself completely from mood or state changing substance or activity. (NOTE: lapse / relapse should be coded here)" .


###  https://purl.org/turbbo/RBBO_R7woWtbNCi0dJrw4OZCukC6
RBBO:R7woWtbNCi0dJrw4OZCukC6 rdf:type owl:Class ;
                             rdfs:subClassOf RBBO:RDzsFgl9xnDJkw9zXLWULAv ;
                             rdfs:label "Using computer devices" ;
                             <http://www.w3.org/2004/02/skos/core#definition> "The act of using a computer device (electronic machines such as laptop, smartphone, tablet, etc.)." .


###  https://purl.org/turbbo/RBBO_R7x8NHLRGEcEymTXMx3THX7
RBBO:R7x8NHLRGEcEymTXMx3THX7 rdf:type owl:Class ;
                             rdfs:subClassOf RBBO:RBuoEsSFBhOGJtFyQKJv3yx ;
                             rdfs:label "Engaging in behavior related to maintaining one's health" ;
                             <http://www.w3.org/2004/02/skos/core#definition> "Activities undertaken for the purpose of preventing or detecting disease or for improving health and well being." .


###  https://purl.org/turbbo/RBBO_R7yShojeNYC1aYv0rEc3xjO
RBBO:R7yShojeNYC1aYv0rEc3xjO rdf:type owl:Class ;
                             rdfs:subClassOf RBBO:Rb1xX794wVt3QQownZtSbO ;
                             rdfs:label "Attending Performing arts" ;
                             <http://www.w3.org/2004/02/skos/core#definition> "Attending a creative activity that is performed in front of an audience, such as drama, music, and dance." .


###  https://purl.org/turbbo/RBBO_R81UtNoTnqDkn9qWK7IrTU8
RBBO:R81UtNoTnqDkn9qWK7IrTU8 rdf:type owl:Class ;
                             rdfs:subClassOf RBBO:R8IYw8QdSmDOKfhF0LcZSGR ;
                             rdfs:label "Looking at erotic material" ;
                             <http://www.w3.org/2004/02/skos/core#definition> "Direct one’s gaze at erotic material." .


###  https://purl.org/turbbo/RBBO_R84iVOhssiIeFAzqm1Mi9zj
RBBO:R84iVOhssiIeFAzqm1Mi9zj rdf:type owl:Class ;
                             rdfs:subClassOf RBBO:R7uK2tMCWgORKYlpKazgtMt ;
                             rdfs:label "Eating Vegetables" ;
                             <http://www.w3.org/2004/02/skos/core#definition> "The consumption of the edible part of a usually herbaceous plant (such as the cabbage, bean, or potato)." .


###  https://purl.org/turbbo/RBBO_R85ghQJrvubARtcN51qsWvE
RBBO:R85ghQJrvubARtcN51qsWvE rdf:type owl:Class ;
                             rdfs:subClassOf RBBO:R9SZhlXBAdyrsI5ItrSRZDG ;
                             rdfs:label "Taking vaccinations" ;
                             <http://www.w3.org/2004/02/skos/core#definition> "Receiving administration of vaccines to stimulate the host's immune response. This includes any preparation intended for active immunological prophylaxis or treatment." .


###  https://purl.org/turbbo/RBBO_R8728B2O8Nh1286K7Qks2I5
RBBO:R8728B2O8Nh1286K7Qks2I5 rdf:type owl:Class ;
                             rdfs:subClassOf RBBO:R7ksLdc5AtNZogZjcdwMAz ;
                             rdfs:label "Renting movies" ;
                             <http://www.w3.org/2004/02/skos/core#definition> "To pay money in return for being able to view movies (that belong to someone else)." .


###  https://purl.org/turbbo/RBBO_R88jWHnsn3PZlovY39SFqII
RBBO:R88jWHnsn3PZlovY39SFqII rdf:type owl:Class ;
                             rdfs:subClassOf RBBO:R7ou7HEwYODwmkHhLtEqW2B ;
                             rdfs:label "Aerobics" ;
                             <http://www.w3.org/2004/02/skos/core#definition> "A system of exercises often done by a group of people while music is playing" .


###  https://purl.org/turbbo/RBBO_R88lPKWIB1fAon9hpD61R9
RBBO:R88lPKWIB1fAon9hpD61R9 rdf:type owl:Class ;
                            rdfs:subClassOf RBBO:RCKDQM6dfhit3RC352IGkgN ;
                            rdfs:label "Using Ecstasy" ;
                            <http://www.w3.org/2004/02/skos/core#definition> "The use of a synthetic amphetamine analog C11H15NO2 used illicitly for its mood-enhancing and hallucinogenic properties — called also MDMA" .


###  https://purl.org/turbbo/RBBO_R8969KVnC9qwhEOlMBFOl0K
RBBO:R8969KVnC9qwhEOlMBFOl0K rdf:type owl:Class ;
                             rdfs:subClassOf RBBO:RELjqe9K96RTVusFCzO665 ;
                             rdfs:label "Attending Parent Teacher Organization meeting" ;
                             <http://www.w3.org/2004/02/skos/core#definition> "To go and be present at a Parent Teacher Organization meeting." .


###  https://purl.org/turbbo/RBBO_R8DhTyMU53x20DpGqwMj0uW
RBBO:R8DhTyMU53x20DpGqwMj0uW rdf:type owl:Class ;
                             rdfs:subClassOf RBBO:RChrJYRTZRmBDhl2HTuXV4S ;
                             rdfs:label "Participating in Dental Care" ;
                             <http://www.w3.org/2004/02/skos/core#definition> "The act of seeking care for the functional and aesthetic aspects of the hard and soft tissues of the oral and maxillofacial regions." .


###  https://purl.org/turbbo/RBBO_R8FZDhDYustxTQzsvyutx8Q
RBBO:R8FZDhDYustxTQzsvyutx8Q rdf:type owl:Class ;
                             rdfs:subClassOf RBBO:RCj2g7DNklxWdnq0FhKcaUK ;
                             rdfs:label "Hiring a prostitute" ;
                             <http://www.w3.org/2004/02/skos/core#definition> "The act of employing a person to engage in sexual activity for payment." .


###  https://purl.org/turbbo/RBBO_R8GcYRzBiq0zUKaVzCrDbDh
RBBO:R8GcYRzBiq0zUKaVzCrDbDh rdf:type owl:Class ;
                             rdfs:subClassOf RBBO:RDw1Q66ue2imTNF7lazEvKw ;
                             rdfs:label "Engaging in domestic violence" ;
                             <http://www.w3.org/2004/02/skos/core#definition> "The act of an escalating set of violent behaviors in the context of a marital or other intimate relationship." .


###  https://purl.org/turbbo/RBBO_R8GzSPHABwljcmb4WOEdA6D
RBBO:R8GzSPHABwljcmb4WOEdA6D rdf:type owl:Class ;
                             rdfs:subClassOf RBBO:RDw1Q66ue2imTNF7lazEvKw ;
                             rdfs:label "Threatening" ;
                             <http://www.w3.org/2004/02/skos/core#definition> "The act of saying that you will harm someone or do something unpleasant or unwanted especially in order to make someone do what you want." .


###  https://purl.org/turbbo/RBBO_R8IYw8QdSmDOKfhF0LcZSGR
RBBO:R8IYw8QdSmDOKfhF0LcZSGR rdf:type owl:Class ;
                             rdfs:subClassOf RBBO:RD0GMkoktmQ73gfqCl0qW1R ;
                             rdfs:label "Looking" ;
                             <http://www.w3.org/2004/02/skos/core#definition> "Direct one’s gaze in a specified direction." .


###  https://purl.org/turbbo/RBBO_R8K4w41cfj2BD24EvxDQPM9
RBBO:R8K4w41cfj2BD24EvxDQPM9 rdf:type owl:Class ;
                             rdfs:subClassOf RBBO:RFGrqCSRvAPz3uiW6oXcW7 ;
                             rdfs:label "Participating in performing arts" .


###  https://purl.org/turbbo/RBBO_R8KGFREdhoCRkCDNcTG8rZL
RBBO:R8KGFREdhoCRkCDNcTG8rZL rdf:type owl:Class ;
                             rdfs:subClassOf RBBO:RDdB56hI5WEz1kELL2HbIdh ;
                             rdfs:label "Smoking Cigar(ette)" ;
                             <http://www.w3.org/2004/02/skos/core#definition> "The use of a small roll of paper filled with cut tobacco in order to smoke." .


###  https://purl.org/turbbo/RBBO_R8KvqWb8C67t2NkL6mgWYY8
RBBO:R8KvqWb8C67t2NkL6mgWYY8 rdf:type owl:Class ;
                             rdfs:subClassOf RBBO:RCKDQM6dfhit3RC352IGkgN ;
                             rdfs:label "Using Methamphetamines and amphetamines" ;
                             <http://www.w3.org/2004/02/skos/core#definition> "The use of a synthetic drug of the phenethylamine family that causes the nervous system to become more active resulting in increased energy and excitement." .


###  https://purl.org/turbbo/RBBO_R8L0j33ISylhnbDKERZPpfI
RBBO:R8L0j33ISylhnbDKERZPpfI rdf:type owl:Class ;
                             rdfs:subClassOf RBBO:R8qMM1AUIWkGs9uIR3zf0Oe ;
                             rdfs:label "Attending services" ;
                             <http://www.w3.org/2004/02/skos/core#definition> "To go and be present at a meeting for worship." .


###  https://purl.org/turbbo/RBBO_R8PZrDPglU5HUGsnWkFpBh8
RBBO:R8PZrDPglU5HUGsnWkFpBh8 rdf:type owl:Class ;
                             rdfs:subClassOf RBBO:R7ou7HEwYODwmkHhLtEqW2B ;
                             rdfs:label "Swimming" ;
                             <http://www.w3.org/2004/02/skos/core#definition> "The sport or activity of moving through water by moving your arms and legs." .


###  https://purl.org/turbbo/RBBO_R8QKq0DUYbu1hFlkFQbcDqz
RBBO:R8QKq0DUYbu1hFlkFQbcDqz rdf:type owl:Class ;
                             rdfs:subClassOf RBBO:RCLGCfCEICjWDiyU2xYotQk ;
                             rdfs:label "Engaging in behaviors related to acquiring, keeping and terminating a job" ;
                             <http://www.w3.org/2004/02/skos/core#definition> "Engage in activities to search for, secure, maintain, or terminate work that a person does regularly in order to earn money." .


###  https://purl.org/turbbo/RBBO_R8ReuBYJRPqCMN23dxvaHoB
RBBO:R8ReuBYJRPqCMN23dxvaHoB rdf:type owl:Class ;
                             rdfs:subClassOf RBBO:RFGrqCSRvAPz3uiW6oXcW7 ;
                             rdfs:label "Engaging in unstructured play" ;
                             <http://www.w3.org/2004/02/skos/core#definition> "Engaging in a game that is not happening according to a plan." .


###  https://purl.org/turbbo/RBBO_R8SK0qidAhGaUAt6EOlmvfo
RBBO:R8SK0qidAhGaUAt6EOlmvfo rdf:type owl:Class ;
                             rdfs:subClassOf RBBO:R7ou7HEwYODwmkHhLtEqW2B ;
                             rdfs:label "Biking" ;
                             <http://www.w3.org/2004/02/skos/core#definition> "The act of riding a bicycle." .


###  https://purl.org/turbbo/RBBO_R8TZfuwPIav5afH2Q5m2JhO
RBBO:R8TZfuwPIav5afH2Q5m2JhO rdf:type owl:Class ;
                             rdfs:subClassOf RBBO:RDd9PVm2VkoGBq6nc5q376d ;
                             rdfs:label "Volunteering" .


###  https://purl.org/turbbo/RBBO_R8Vq82H2GwQMknyntl4zDIL
RBBO:R8Vq82H2GwQMknyntl4zDIL rdf:type owl:Class ;
                             rdfs:subClassOf RBBO:R3GTM1WIfB3LofIOVpVVKU ;
                             rdfs:label "Ingesting Sweetener" ;
                             <http://www.w3.org/2004/02/skos/core#definition> "Ingesting a food additive which duplicates the effect of sugar on the taste, but with fewer calories. They are also called sugar substitutes." .


###  https://purl.org/turbbo/RBBO_R8YCY2i5DojBDHL0jf200QA
RBBO:R8YCY2i5DojBDHL0jf200QA rdf:type owl:Class ;
                             rdfs:subClassOf RBBO:R9SZhlXBAdyrsI5ItrSRZDG ;
                             rdfs:label "Using sun protection" ;
                             <http://www.w3.org/2004/02/skos/core#definition> "To cover or shield from sun exposure, injury, or damage, for purposes of maintaining one's health." .


###  https://purl.org/turbbo/RBBO_R8YXJ6zVKsyJLtpqdLeBgGe
RBBO:R8YXJ6zVKsyJLtpqdLeBgGe rdf:type owl:Class ;
                             rdfs:subClassOf RBBO:R3GTM1WIfB3LofIOVpVVKU ;
                             rdfs:label "Ingesting Sodium" ;
                             <http://www.w3.org/2004/02/skos/core#definition> "Ingesting a soft silver-white element that is found in salt, baking soda, and other compounds." .


###  https://purl.org/turbbo/RBBO_R8ajn0bTfdCHx3nX7JiNJM2
RBBO:R8ajn0bTfdCHx3nX7JiNJM2 rdf:type owl:Class ;
                             rdfs:subClassOf RBBO:RC9p1nKgQCD9ZNR5vvX2qiZ ;
                             rdfs:label "Writing messages" ;
                             <http://www.w3.org/2004/02/skos/core#definition> "The action of communication through a sequence of letters, words, or symbols marked on a surface" .


###  https://purl.org/turbbo/RBBO_R8cCVugnbr4KoPFPOy98Qt2
RBBO:R8cCVugnbr4KoPFPOy98Qt2 rdf:type owl:Class ;
                             rdfs:subClassOf RBBO:R8QKq0DUYbu1hFlkFQbcDqz ;
                             rdfs:label "Maintaining a job" ;
                             <http://www.w3.org/2004/02/skos/core#definition> "Retaining a paid position of regular employment." .


###  https://purl.org/turbbo/RBBO_R8gB9OYdqQSqTsDpbt2xwPk
RBBO:R8gB9OYdqQSqTsDpbt2xwPk rdf:type owl:Class ;
                             rdfs:subClassOf RBBO:R7ou7HEwYODwmkHhLtEqW2B ;
                             rdfs:label "Running" ;
                             <http://www.w3.org/2004/02/skos/core#definition> "To move using the legs, going faster than when walking." .


###  https://purl.org/turbbo/RBBO_R8gZTtFMXyiMRwUm5WLrhXS
RBBO:R8gZTtFMXyiMRwUm5WLrhXS rdf:type owl:Class ;
                             rdfs:subClassOf RBBO:R6hKctZFZcjKJBLZwC7y9T ;
                             rdfs:label "Engaging in interactive communication (both receiving and producing)" ;
                             <http://www.w3.org/2004/02/skos/core#definition> "Exchange of information by the use of words, sounds or signs between two or more people." .


###  https://purl.org/turbbo/RBBO_R8j2bn1hgnMSEJiolCCWbJ8
RBBO:R8j2bn1hgnMSEJiolCCWbJ8 rdf:type owl:Class ;
                             rdfs:subClassOf RBBO:R7uK2tMCWgORKYlpKazgtMt ;
                             rdfs:label "Eating Cereal" ;
                             <http://www.w3.org/2004/02/skos/core#definition> "The consumption of a plant (as a grass) yielding starchy grain suitable for food." .


###  https://purl.org/turbbo/RBBO_R8jttvmuprS05qQGlFDRZJE
RBBO:R8jttvmuprS05qQGlFDRZJE rdf:type owl:Class ;
                             rdfs:subClassOf RBBO:Rj9feeEPPMDelLiPVmOGiu ;
                             rdfs:label "Engaging in play education" ;
                             <http://www.w3.org/2004/02/skos/core#definition> "The act of educating someone (especially children) on activities for enjoyment and recreation rather than a serious or practical purpose." .


###  https://purl.org/turbbo/RBBO_R8kPkEyryCnXa6dbEra5Vai
RBBO:R8kPkEyryCnXa6dbEra5Vai rdf:type owl:Class ;
                             rdfs:subClassOf RBBO:R7MWXGKIGLx4ykI6IfNRWHF ,
                                             RBBO:Rj9feeEPPMDelLiPVmOGiu ;
                             rdfs:label "Studying" ;
                             <http://www.w3.org/2004/02/skos/core#definition> "Application of the mental faculties to the acquisition of knowledge." .


###  https://purl.org/turbbo/RBBO_R8nh8nvCVDLaYKhxeVb3IW8
RBBO:R8nh8nvCVDLaYKhxeVb3IW8 rdf:type owl:Class ;
                             rdfs:subClassOf RBBO:RDck4eDShRuThnEF6Ql5OxH ;
                             rdfs:label "Laughing" ;
                             <http://www.w3.org/2004/02/skos/core#definition> "Make the spontaneous sounds and movements of the face and body that are the instinctive expressions of lively amusement and sometimes also of derision." .


###  https://purl.org/turbbo/RBBO_R8npJYdDua4rtmotUR8gkXA
RBBO:R8npJYdDua4rtmotUR8gkXA rdf:type owl:Class ;
                             rdfs:subClassOf RBBO:RayAVAeF9vXpz9v3jwSLzs ;
                             rdfs:label "Illegal downloading of media" ;
                             <http://www.w3.org/2004/02/skos/core#definition> "The act of downloading media (e.g., books, music, or movies) without the sanction of the copyright holder." .


###  https://purl.org/turbbo/RBBO_R8qMM1AUIWkGs9uIR3zf0Oe
RBBO:R8qMM1AUIWkGs9uIR3zf0Oe rdf:type owl:Class ;
                             rdfs:subClassOf RBBO:R9JyzynAe7H3xtK0rPOT841 ;
                             rdfs:label "Engaging in behavior related to spirituality" ;
                             <http://www.w3.org/2004/02/skos/core#definition> "Engaging in behaviors concerned with spirituality, religion or religious matters" .


###  https://purl.org/turbbo/RBBO_R8qZTwXVecGIlp2WSH9wCuV
RBBO:R8qZTwXVecGIlp2WSH9wCuV rdf:type owl:Class ;
                             rdfs:subClassOf RBBO:RBOTVkkObNNllFP9EFEOIR2 ;
                             rdfs:label "Eating Potato chips" ;
                             <http://www.w3.org/2004/02/skos/core#definition> "The consumption of a wafer-thin slice of potato fried or baked until crisp." .


###  https://purl.org/turbbo/RBBO_R8ukhPJPMhF45gwrCl4Jm0F
RBBO:R8ukhPJPMhF45gwrCl4Jm0F rdf:type owl:Class ;
                             rdfs:subClassOf RBBO:RayAVAeF9vXpz9v3jwSLzs ;
                             rdfs:label "Disturbing the peace" ;
                             <http://www.w3.org/2004/02/skos/core#definition> "The act of being loud or roudy in public places." .


###  https://purl.org/turbbo/RBBO_R8xQJz3jvt4sTKFSkqiASfr
RBBO:R8xQJz3jvt4sTKFSkqiASfr rdf:type owl:Class ;
                             rdfs:subClassOf RBBO:RDw1Q66ue2imTNF7lazEvKw ;
                             rdfs:label "Encouraging others to fight" ;
                             <http://www.w3.org/2004/02/skos/core#definition> "Prompting others to take part in a violent struggle involving the exchange of physical blows or the use of weapons." .


###  https://purl.org/turbbo/RBBO_R91lBSpjaJ12eZqZOf0YYtE
RBBO:R91lBSpjaJ12eZqZOf0YYtE rdf:type owl:Class ;
                             rdfs:subClassOf RBBO:R3GTM1WIfB3LofIOVpVVKU ;
                             rdfs:label "Ingesting Energy" ;
                             <http://www.w3.org/2004/02/skos/core#definition> "The Strength and vitality provided by food or drink consumed for sustaining physical or mental activity" .


###  https://purl.org/turbbo/RBBO_R932mpM1CTdcqEBiTOXDNPM
RBBO:R932mpM1CTdcqEBiTOXDNPM rdf:type owl:Class ;
                             rdfs:subClassOf RBBO:RCj2g7DNklxWdnq0FhKcaUK ;
                             rdfs:label "Working as a prostitute" ;
                             <http://www.w3.org/2004/02/skos/core#definition> "The practice or occupation of engaging in sexual activity with someone for payment." .


###  https://purl.org/turbbo/RBBO_R93z8pYrtnWwimDtpP76jOC
RBBO:R93z8pYrtnWwimDtpP76jOC rdf:type owl:Class ;
                             rdfs:subClassOf RBBO:RhlslZKl21SGb8L452uSU8 ;
                             rdfs:label "Structuring" ;
                             <http://www.w3.org/2004/02/skos/core#definition> "The act of arranging transactions according to a plan." .


###  https://purl.org/turbbo/RBBO_R957y0lozcqJOI5opHzoPhe
RBBO:R957y0lozcqJOI5opHzoPhe rdf:type owl:Class ;
                             rdfs:subClassOf RBBO:RayAVAeF9vXpz9v3jwSLzs ;
                             rdfs:label "Exaggerating" ;
                             <http://www.w3.org/2004/02/skos/core#definition> "To enlarge beyond bounds or the truth." .


###  https://purl.org/turbbo/RBBO_R95U5YkbbSN3USUNqiS9yh5
RBBO:R95U5YkbbSN3USUNqiS9yh5 rdf:type owl:Class ;
                             rdfs:subClassOf RBBO:RayAVAeF9vXpz9v3jwSLzs ;
                             rdfs:label "Lying" ;
                             <http://www.w3.org/2004/02/skos/core#definition> "Making an untrue statement with intent to deceive or to create a false or misleading impression" .


###  https://purl.org/turbbo/RBBO_R98L21up1SSyEgiLNxwvbKM
RBBO:R98L21up1SSyEgiLNxwvbKM rdf:type owl:Class ;
                             rdfs:subClassOf RBBO:RDqjiSX08Nc9xxSBrR5KMOM ;
                             rdfs:label "Watching" ;
                             <http://www.w3.org/2004/02/skos/core#definition> "The action of observing attentively, typically for a period of time." .


###  https://purl.org/turbbo/RBBO_R9A9B5YB25QH3TR4iHuH9wq
RBBO:R9A9B5YB25QH3TR4iHuH9wq rdf:type owl:Class ;
                             rdfs:subClassOf RBBO:RCKDQM6dfhit3RC352IGkgN ;
                             rdfs:label "Using Sedatives" ;
                             <http://www.w3.org/2004/02/skos/core#definition> "The use of an agent that depresses the central nervous system (CNS) and is used to induce calm and sleep." .


###  https://purl.org/turbbo/RBBO_R9BeiQh4oa8EbuNm1bjryZB
RBBO:R9BeiQh4oa8EbuNm1bjryZB rdf:type owl:Class ;
                             rdfs:subClassOf RBBO:R8QKq0DUYbu1hFlkFQbcDqz ;
                             rdfs:label "Seeking a job" ;
                             <http://www.w3.org/2004/02/skos/core#definition> "To search for work that a person does regularly in order to earn money." .


###  https://purl.org/turbbo/RBBO_R9D52BADRQOlw7YY7xDYL0P
RBBO:R9D52BADRQOlw7YY7xDYL0P rdf:type owl:Class ;
                             rdfs:subClassOf RBBO:RDGyOtjqZKCX0tefKkHlCB4 ;
                             rdfs:label "Reading aloud" ;
                             <http://www.w3.org/2004/02/skos/core#definition> "The action of looking at and comprehending the meaning of (written or printed matter) by mentally interpreting the characters or symbols of which it is composed and simultaneously verbalizing the read content" .


###  https://purl.org/turbbo/RBBO_R9DODpTBGtD47Gkr98ZKGT4
RBBO:R9DODpTBGtD47Gkr98ZKGT4 rdf:type owl:Class ;
                             rdfs:subClassOf RBBO:RDck4eDShRuThnEF6Ql5OxH ;
                             rdfs:label "Producing body gestures/postures" ;
                             <http://www.w3.org/2004/02/skos/core#definition> "Producing a movement of your body that shows or emphasizes an idea or a feeling." .


###  https://purl.org/turbbo/RBBO_R9H2ctyCGAYoASJRT1kN0ln
RBBO:R9H2ctyCGAYoASJRT1kN0ln rdf:type owl:Class ;
                             rdfs:subClassOf RBBO:RDqrSoVPQjxqqJkRCeAY7Fh ;
                             rdfs:label "Discussing class selection" ;
                             <http://www.w3.org/2004/02/skos/core#definition> "To talk about academic class selection with another person or group." .


###  https://purl.org/turbbo/RBBO_R9JyzynAe7H3xtK0rPOT841
RBBO:R9JyzynAe7H3xtK0rPOT841 rdf:type owl:Class ;
                             rdfs:subClassOf RBBO:RC5cLYrHZhVyinK9OLpz4Ax ;
                             rdfs:label "Engaging in community life" ;
                             <http://www.w3.org/2004/02/skos/core#definition> "Engaging in activities with or related to a group of people who live in the same area (such as a city, town, or neighbourhood)." .


###  https://purl.org/turbbo/RBBO_R9Ohv3YKoJsxuaDDeL4eQXx
RBBO:R9Ohv3YKoJsxuaDDeL4eQXx rdf:type owl:Class ;
                             rdfs:subClassOf RBBO:RD0GMkoktmQ73gfqCl0qW1R ;
                             rdfs:label "Listening to spoken messages" ;
                             <http://www.w3.org/2004/02/skos/core#definition> "The action of receiving information or another one´s feelings in speech." .


###  https://purl.org/turbbo/RBBO_R9QvUdQnrx7qXQS2hP9uzrA
RBBO:R9QvUdQnrx7qXQS2hP9uzrA rdf:type owl:Class ;
                             rdfs:subClassOf RBBO:RDd9PVm2VkoGBq6nc5q376d ;
                             rdfs:label "Donating blood" ;
                             <http://www.w3.org/2004/02/skos/core#definition> "Volunteering to have blood removed for transplantation or other purpose." .


###  https://purl.org/turbbo/RBBO_R9SZhlXBAdyrsI5ItrSRZDG
RBBO:R9SZhlXBAdyrsI5ItrSRZDG rdf:type owl:Class ;
                             rdfs:subClassOf RBBO:R7x8NHLRGEcEymTXMx3THX7 ;
                             rdfs:label "Taking protective actions" ;
                             <http://www.w3.org/2004/02/skos/core#definition> "To cover or shield from exposure, injury, damage, or destruction for purposes of maintaining one's health." .


###  https://purl.org/turbbo/RBBO_R9UnNO27OcDXMFjeAejMhJr
RBBO:R9UnNO27OcDXMFjeAejMhJr rdf:type owl:Class ;
                             rdfs:subClassOf RBBO:RayAVAeF9vXpz9v3jwSLzs ;
                             rdfs:label "Speeding" ;
                             <http://www.w3.org/2004/02/skos/core#definition> "Operating a motorized vehicle at speeds in excess of the posted limit." .


###  https://purl.org/turbbo/RBBO_R9XzdtCeE4Ytjbjkmi81yJu
RBBO:R9XzdtCeE4Ytjbjkmi81yJu rdf:type owl:Class ;
                             rdfs:subClassOf <https://purl.org/turbbo/RBBO_0000123> ;
                             rdfs:label "Engaging in interpersonal interactions and relationships" ;
                             <http://www.w3.org/2004/02/skos/core#definition> "The act of engaging in short or long-term association between two or more people, including kinship relations, romantic, business, and social interactions." .


###  https://purl.org/turbbo/RBBO_R9YKewO63jKFuCf6CxcRw42
RBBO:R9YKewO63jKFuCf6CxcRw42 rdf:type owl:Class ;
                             rdfs:subClassOf RBBO:R7MWXGKIGLx4ykI6IfNRWHF ,
                                             RBBO:RayAVAeF9vXpz9v3jwSLzs ;
                             rdfs:label "Cheating" ;
                             <http://www.w3.org/2004/02/skos/core#definition> "To practice fraud or trickery." .


###  https://purl.org/turbbo/RBBO_R9Z7Ya4l3pO5GTyuD4lXXMj
RBBO:R9Z7Ya4l3pO5GTyuD4lXXMj rdf:type owl:Class ;
                             rdfs:subClassOf RBBO:RDck4eDShRuThnEF6Ql5OxH ;
                             rdfs:label "Touching" ;
                             <http://www.w3.org/2004/02/skos/core#definition> "Bring one’s hand or another part of one’s body into contact with another person or object" .


###  https://purl.org/turbbo/RBBO_R9cWGdaP36P9kM5hHEPRMHg
RBBO:R9cWGdaP36P9kM5hHEPRMHg rdf:type owl:Class ;
                             rdfs:subClassOf RBBO:RBuoEsSFBhOGJtFyQKJv3yx ;
                             rdfs:label "Washing oneself" ;
                             <http://www.w3.org/2004/02/skos/core#definition> "Clean oneself, commonly with soap and water." .


###  https://purl.org/turbbo/RBBO_R9emxBTFO7jzHWHEnRezJFm
RBBO:R9emxBTFO7jzHWHEnRezJFm rdf:type owl:Class ;
                             rdfs:subClassOf RBBO:Rj9feeEPPMDelLiPVmOGiu ;
                             rdfs:label "Engaging in cultural education" ;
                             <http://www.w3.org/2004/02/skos/core#definition> "The act of or relating to the ideas, customs, and social behavior of a society." .


###  https://purl.org/turbbo/RBBO_R9hKOlaTiUV2zNrdjrXHIoH
RBBO:R9hKOlaTiUV2zNrdjrXHIoH rdf:type owl:Class ;
                             rdfs:subClassOf RBBO:RFGrqCSRvAPz3uiW6oXcW7 ;
                             rdfs:label "Building models" ;
                             <http://www.w3.org/2004/02/skos/core#definition> "The act or process of making a usually small copy of something by putting together materials." .


###  https://purl.org/turbbo/RBBO_R9j8nrLtFzMmIVh4MlAP6EA
RBBO:R9j8nrLtFzMmIVh4MlAP6EA rdf:type owl:Class ;
                             rdfs:subClassOf RBBO:RhlslZKl21SGb8L452uSU8 ;
                             rdfs:label "Saving" ;
                             <http://www.w3.org/2004/02/skos/core#definition> "The process of setting aside a portion of current income for future use, or the flow of resources accumulated in this way over a given period of time." .


###  https://purl.org/turbbo/RBBO_R9p5Yej3AOqhbZTK2kCgSWX
RBBO:R9p5Yej3AOqhbZTK2kCgSWX rdf:type owl:Class ;
                             rdfs:subClassOf RBBO:RFGrqCSRvAPz3uiW6oXcW7 ;
                             rdfs:label "Playing sports" ;
                             <http://www.w3.org/2004/02/skos/core#definition> "The act of engaging in a contest or game in which people do certain physical activities according to a specific set of rules and compete against each other." .


###  https://purl.org/turbbo/RBBO_R9qiMGm7ZsvOF8PVopNjoce
RBBO:R9qiMGm7ZsvOF8PVopNjoce rdf:type owl:Class ;
                             rdfs:subClassOf RBBO:R7SqDxfmXPDIUSZShgwaIyO ;
                             rdfs:label "Participating in testing" ;
                             <http://www.w3.org/2004/02/skos/core#definition> "The act of participating in a diagnostic procedure for critical evaluation of the presence or absence of a condition, disease or change in function." .


###  https://purl.org/turbbo/RBBO_R9uUdCancI6Xhj93NGDpAa0
RBBO:R9uUdCancI6Xhj93NGDpAa0 rdf:type owl:Class ;
                             rdfs:subClassOf RBBO:RDd9PVm2VkoGBq6nc5q376d ;
                             rdfs:label "Donating organs" ;
                             <http://www.w3.org/2004/02/skos/core#definition> "The act of volunteering to give up and transfer an organ, organ part, or tissue from one body to another, for the purpose of replacing the recipient's damaged or failing organ with a working one from the donor." .


###  https://purl.org/turbbo/RBBO_R9vNeC1oitAazXgjCZLFreu
RBBO:R9vNeC1oitAazXgjCZLFreu rdf:type owl:Class ;
                             rdfs:subClassOf RBBO:RCKDQM6dfhit3RC352IGkgN ;
                             rdfs:label "Using Hallucinogens" ;
                             <http://www.w3.org/2004/02/skos/core#definition> "The use of drugs that cause profound distortions in a person's perceptions of reality, including delusions and false notions." .


###  https://purl.org/turbbo/RBBO_R9wnOxSo6VExTSy6o6aVaHH
RBBO:R9wnOxSo6VExTSy6o6aVaHH rdf:type owl:Class ;
                             rdfs:subClassOf RBBO:R7ou7HEwYODwmkHhLtEqW2B ;
                             rdfs:label "Driving motorized vehicles" ;
                             <http://www.w3.org/2004/02/skos/core#definition> "The act of control and operation of a motorized vehicle." .


###  https://purl.org/turbbo/RBBO_R9x7Hkf4ZOijPKfUQeDiqSM
RBBO:R9x7Hkf4ZOijPKfUQeDiqSM rdf:type owl:Class ;
                             rdfs:subClassOf RBBO:RDw1Q66ue2imTNF7lazEvKw ;
                             rdfs:label "Robbing" .


###  https://purl.org/turbbo/RBBO_RB0PylLvIZAtwndoosMLliQ
RBBO:RB0PylLvIZAtwndoosMLliQ rdf:type owl:Class ;
                             rdfs:subClassOf RBBO:RDck4eDShRuThnEF6Ql5OxH ;
                             rdfs:label "Producing drawings or photographs" ;
                             <http://www.w3.org/2004/02/skos/core#definition> "Making picture(s) or diagram(s) with a pencil, pen, or crayon rather than paint; taking photographs." .


###  https://purl.org/turbbo/RBBO_RB1r62EgpOwuwELaN1GN8WR
RBBO:RB1r62EgpOwuwELaN1GN8WR rdf:type owl:Class ;
                             rdfs:subClassOf RBBO:RCKDQM6dfhit3RC352IGkgN ;
                             rdfs:label "Engaging in suicidal behavior/ suicide" ;
                             <http://www.w3.org/2004/02/skos/core#definition> "Suicide is the act of taking one's own life on purpose. Suicidal behavior is any action that could cause a person to die, such as taking a drug overdose or crashing a car on purpose." .


###  https://purl.org/turbbo/RBBO_RB259d2EF9BQAEoE02NuAv3
RBBO:RB259d2EF9BQAEoE02NuAv3 rdf:type owl:Class ;
                             rdfs:subClassOf RBBO:RINOST75D6djkBWwq9c5bA ;
                             rdfs:label "Having non-intercourse sexual contact" ;
                             <http://www.w3.org/2004/02/skos/core#definition> "The act of physical sexual contact such as petting, engaging in amorous embracing, caressing, and kissing between individuals, but without intercourse." .


###  https://purl.org/turbbo/RBBO_RB3KW9HRLxfZaM9TK6L64Dy
RBBO:RB3KW9HRLxfZaM9TK6L64Dy rdf:type owl:Class ;
                             rdfs:subClassOf RBBO:R3GTM1WIfB3LofIOVpVVKU ;
                             rdfs:label "Ingesting Fat" ;
                             <http://www.w3.org/2004/02/skos/core#definition> "Ingesting a class of food constituents, also known as fats and oils, that serve as a source of energy and essential fatty acids in animals." .


###  https://purl.org/turbbo/RBBO_RB4NyZKyze11ZGYvquGrdrA
RBBO:RB4NyZKyze11ZGYvquGrdrA rdf:type owl:Class ;
                             rdfs:subClassOf RBBO:R9JyzynAe7H3xtK0rPOT841 ;
                             rdfs:label "Joining or maintaining association or group membership" ;
                             <http://www.w3.org/2004/02/skos/core#definition> "The act of joining or maintaining membership in an organized groups of people who have the same interest, job, etc." .


###  https://purl.org/turbbo/RBBO_RB65zbnDKVRSjQ3mKpcHp8t
RBBO:RB65zbnDKVRSjQ3mKpcHp8t rdf:type owl:Class ;
                             rdfs:subClassOf RBBO:R7qzqygnfKwMVxUR9f0qbNZ ;
                             rdfs:label "Drinking Smoothie" ;
                             <http://www.w3.org/2004/02/skos/core#definition> "Consumption of a thick, smooth drink of fresh fruit pureed with milk, yogurt, or ice cream." .


###  https://purl.org/turbbo/RBBO_RB8MzAOq8S3Jt4O0y71cZC3
RBBO:RB8MzAOq8S3Jt4O0y71cZC3 rdf:type owl:Class ;
                             rdfs:subClassOf RBBO:RayAVAeF9vXpz9v3jwSLzs ;
                             rdfs:label "Joining or maintaining membership in criminal enterprise" ;
                             <http://www.w3.org/2004/02/skos/core#definition> "The act of joining or maintaining membership in an organized enterprise carrying out illegal activity." .


###  https://purl.org/turbbo/RBBO_RBEmO5ddPGEUtlHSBkeLFO0
RBBO:RBEmO5ddPGEUtlHSBkeLFO0 rdf:type owl:Class ;
                             rdfs:subClassOf RBBO:RFGrqCSRvAPz3uiW6oXcW7 ;
                             rdfs:label "Doing crafts" .


###  https://purl.org/turbbo/RBBO_RBFL8qZUMKuFB1orHEuZVSt
RBBO:RBFL8qZUMKuFB1orHEuZVSt rdf:type owl:Class ;
                             rdfs:subClassOf RBBO:R9D52BADRQOlw7YY7xDYL0P ;
                             rdfs:label "Reading aloud to child" ;
                             <http://www.w3.org/2004/02/skos/core#definition> "The action of looking at and comprehending the meaning of (written or printed matter) by mentally interpreting the characters or symbols of which it is composed and simultaneously verbalizing the read content to a child." .


###  https://purl.org/turbbo/RBBO_RBFcrIvHBtTdBRW5pvvInk
RBBO:RBFcrIvHBtTdBRW5pvvInk rdf:type owl:Class ;
                            rdfs:subClassOf RBBO:RDB0WPFBq8eRpd2dUYyztb4 ;
                            rdfs:label "Voting" ;
                            <http://www.w3.org/2004/02/skos/core#definition> "The official choice that someone makes in an election, meeting, etc., by casting a ballot, rasing the hand, speaking their choice aloud, etc." .


###  https://purl.org/turbbo/RBBO_RBHbpWceDYn4BB2W7tomnNI
RBBO:RBHbpWceDYn4BB2W7tomnNI rdf:type owl:Class ;
                             rdfs:subClassOf RBBO:RDck4eDShRuThnEF6Ql5OxH ;
                             rdfs:label "Producing facial expressions" ;
                             <http://www.w3.org/2004/02/skos/core#definition> "The look on someone's face (such as smiling, frowning, etc)." .


###  https://purl.org/turbbo/RBBO_RBOTVkkObNNllFP9EFEOIR2
RBBO:RBOTVkkObNNllFP9EFEOIR2 rdf:type owl:Class ;
                             rdfs:subClassOf RBBO:R7uK2tMCWgORKYlpKazgtMt ;
                             rdfs:label "Eating Snack" ;
                             <http://www.w3.org/2004/02/skos/core#definition> "The consumption of a small amount of food between meals." .


###  https://purl.org/turbbo/RBBO_RBTRLIR5oUwjhLmK6oAIMb4
RBBO:RBTRLIR5oUwjhLmK6oAIMb4 rdf:type owl:Class ;
                             rdfs:subClassOf RBBO:RChrJYRTZRmBDhl2HTuXV4S ;
                             rdfs:label "Participating in Group support/ treatment" ;
                             <http://www.w3.org/2004/02/skos/core#definition> "The act of attending group support sessions led by a trained professional in order to attain healing or recovery." .


###  https://purl.org/turbbo/RBBO_RBTc7cx9eEMPQCOGL8vKPtV
RBBO:RBTc7cx9eEMPQCOGL8vKPtV rdf:type owl:Class ;
                             rdfs:subClassOf RBBO:R3GTM1WIfB3LofIOVpVVKU ;
                             rdfs:label "Ingesting Sugar" ;
                             <http://www.w3.org/2004/02/skos/core#definition> "Ingesting a white crystalline carbohydrate, typically sucrose, used as a sweetener and preservative." .


###  https://purl.org/turbbo/RBBO_RBYfKE4dQXzYNdQGWpLm4RK
RBBO:RBYfKE4dQXzYNdQGWpLm4RK rdf:type owl:Class ;
                             rdfs:subClassOf RBBO:RayAVAeF9vXpz9v3jwSLzs ;
                             rdfs:label "Stealing" ;
                             <http://www.w3.org/2004/02/skos/core#definition> "To take the property of another wrongfully and especially as a habitual or regular practice." .


###  https://purl.org/turbbo/RBBO_RBYkEcGOLDMPaivRiRxA2Zx
RBBO:RBYkEcGOLDMPaivRiRxA2Zx rdf:type owl:Class ;
                             rdfs:subClassOf RBBO:RFGrqCSRvAPz3uiW6oXcW7 ;
                             rdfs:label "Playing video game" ;
                             <http://www.w3.org/2004/02/skos/core#definition> "The act of playing an electronic game played by means of images on a video screen and often emphasizing fast action." .


###  https://purl.org/turbbo/RBBO_RBZBFZG9PRFJpm31aToI1nl
RBBO:RBZBFZG9PRFJpm31aToI1nl rdf:type owl:Class ;
                             rdfs:subClassOf RBBO:RINOST75D6djkBWwq9c5bA ;
                             rdfs:label "Having intercourse" ;
                             <http://www.w3.org/2004/02/skos/core#definition> "The act of physical sexual contact between individuals that involves the genitalia of at least one person." .


###  https://purl.org/turbbo/RBBO_RBdjzI2SqWrJ2prVOK0NHpT
RBBO:RBdjzI2SqWrJ2prVOK0NHpT rdf:type owl:Class ;
                             rdfs:subClassOf RBBO:RayAVAeF9vXpz9v3jwSLzs ;
                             rdfs:label "Breaking curfew" ;
                             <http://www.w3.org/2004/02/skos/core#definition> "The act of being on streets or public areas during hours designated as off-limit by an authority (state or parents)." .


###  https://purl.org/turbbo/RBBO_RBkPOivG8JaZijqer0ZkDjQ
RBBO:RBkPOivG8JaZijqer0ZkDjQ rdf:type owl:Class ;
                             rdfs:subClassOf RBBO:RDLYuvHGi7xCMFHwL7WJ8pF ;
                             rdfs:label "Providing tangible/pragmatic support" ;
                             <http://www.w3.org/2004/02/skos/core#definition> "To give help or assistance through providing something practical that can be touched or felt." .


###  https://purl.org/turbbo/RBBO_RBq7tZ4pj7jvFmyRWgzCAgH
RBBO:RBq7tZ4pj7jvFmyRWgzCAgH rdf:type owl:Class ;
                             rdfs:subClassOf RBBO:RDd9PVm2VkoGBq6nc5q376d ;
                             rdfs:label "Donating money" ;
                             <http://www.w3.org/2004/02/skos/core#definition> "To give money in order to help a cause." .


###  https://purl.org/turbbo/RBBO_RBqLqcQI5H4LBjGjeKL3Xyb
RBBO:RBqLqcQI5H4LBjGjeKL3Xyb rdf:type owl:Class ;
                             rdfs:subClassOf RBBO:R7SqDxfmXPDIUSZShgwaIyO ;
                             rdfs:label "Self-testing" ;
                             <http://www.w3.org/2004/02/skos/core#definition> "The act of checking own body for symptoms of illness." .


###  https://purl.org/turbbo/RBBO_RBtjpUP2Y67IuUsEulri7ce
RBBO:RBtjpUP2Y67IuUsEulri7ce rdf:type owl:Class ;
                             rdfs:subClassOf RBBO:RCKDQM6dfhit3RC352IGkgN ;
                             rdfs:label "Using Opiates" ;
                             <http://www.w3.org/2004/02/skos/core#definition> "The use of the coagulated juice of the opium poppy." .


###  https://purl.org/turbbo/RBBO_RBuoEsSFBhOGJtFyQKJv3yx
RBBO:RBuoEsSFBhOGJtFyQKJv3yx rdf:type owl:Class ;
                             rdfs:subClassOf <https://purl.org/turbbo/RBBO_0000123> ;
                             rdfs:label "Engaging in self-care behavior" ;
                             <http://www.w3.org/2004/02/skos/core#definition> "The provision of what is necessary for one´s health, welfare, maintenance, and protection." .


###  https://purl.org/turbbo/RBBO_RBwChPeGumIcWiAkyjALSbR
RBBO:RBwChPeGumIcWiAkyjALSbR rdf:type owl:Class ;
                             rdfs:subClassOf RBBO:R7x8NHLRGEcEymTXMx3THX7 ;
                             rdfs:label "Managing diet and fitness" ;
                             <http://www.w3.org/2004/02/skos/core#definition> "To eat and drink sparingly or according to prescribed rules and to exercise for the purpose of improving or maintaining health." .


###  https://purl.org/turbbo/RBBO_RBzlXysycBR1G0UWI9dLzUg
RBBO:RBzlXysycBR1G0UWI9dLzUg rdf:type owl:Class ;
                             rdfs:subClassOf RBBO:RDw1Q66ue2imTNF7lazEvKw ;
                             rdfs:label "Damaging property" ;
                             <http://www.w3.org/2004/02/skos/core#definition> "The act of causing damage to or the destruction of public or private property, caused by a person who is not its owner." .


###  https://purl.org/turbbo/RBBO_RC0YClFPlVX751xC4ns9FVj
RBBO:RC0YClFPlVX751xC4ns9FVj rdf:type owl:Class ;
                             rdfs:subClassOf RBBO:RBkPOivG8JaZijqer0ZkDjQ ;
                             rdfs:label "Providing financial support" ;
                             <http://www.w3.org/2004/02/skos/core#definition> "To give help or assistance in the form of money." .


###  https://purl.org/turbbo/RBBO_RC2WMf41q0tzpzdY4Q3IlE4
RBBO:RC2WMf41q0tzpzdY4Q3IlE4 rdf:type owl:Class ;
                             rdfs:subClassOf RBBO:R9qiMGm7ZsvOF8PVopNjoce ;
                             rdfs:label "Participate in baseline exercise test" ;
                             <http://www.w3.org/2004/02/skos/core#definition> "The act of establishing an exercise function starting point to which change may be compared." .


###  https://purl.org/turbbo/RBBO_RC49XywX1UPXtJYddxnrb0h
RBBO:RC49XywX1UPXtJYddxnrb0h rdf:type owl:Class ;
                             rdfs:subClassOf RBBO:R7woWtbNCi0dJrw4OZCukC6 ;
                             rdfs:label "Using the internet" ;
                             <http://www.w3.org/2004/02/skos/core#definition> "Use of global computer network providing a variety of information and communication facilities." .


###  https://purl.org/turbbo/RBBO_RC5LiU2X5C1XaClchoLtN7h
RBBO:RC5LiU2X5C1XaClchoLtN7h rdf:type owl:Class ;
                             rdfs:subClassOf RBBO:RDarCRBoiqojsnZ9V6Oj1EU ;
                             rdfs:label "Doing relaxation exercises" ;
                             <http://www.w3.org/2004/02/skos/core#definition> "The act of performing exercises to reduce stress, muscle tension, and anxiety in the body." .


###  https://purl.org/turbbo/RBBO_RC5cLYrHZhVyinK9OLpz4Ax
RBBO:RC5cLYrHZhVyinK9OLpz4Ax rdf:type owl:Class ;
                             rdfs:subClassOf <https://purl.org/turbbo/RBBO_0000123> ;
                             rdfs:label "Engaging in behavior related to community, social, and civic life" ;
                             <http://www.w3.org/2004/02/skos/core#definition> "Engaging in activities related to a unified body of individuals, including recreation, community affairs, and pro/antisocial behavior." .


###  https://purl.org/turbbo/RBBO_RC5xmY90ofv5EQ1opHYU6rB
RBBO:RC5xmY90ofv5EQ1opHYU6rB rdf:type owl:Class ;
                             rdfs:subClassOf RBBO:RhlslZKl21SGb8L452uSU8 ;
                             rdfs:label "Investing" ;
                             <http://www.w3.org/2004/02/skos/core#definition> "The act of expending money with the expectation of achieving a profit or material result by putting it into financial schemes, shares, or property, or by using it to develop a commercial venture." .


###  https://purl.org/turbbo/RBBO_RC9LMCql8HpBhA11P4OoZgi
RBBO:RC9LMCql8HpBhA11P4OoZgi rdf:type owl:Class ;
                             rdfs:subClassOf RBBO:R93z8pYrtnWwimDtpP76jOC ;
                             rdfs:label "Closing account" ;
                             <http://www.w3.org/2004/02/skos/core#definition> "The occurance of any account that has been closed out or otherwise terminated." .


###  https://purl.org/turbbo/RBBO_RC9irdFOfWCUDChsoJh1FWw
RBBO:RC9irdFOfWCUDChsoJh1FWw rdf:type owl:Class ;
                             rdfs:subClassOf RBBO:RDw1Q66ue2imTNF7lazEvKw ;
                             rdfs:label "Stalking" ;
                             <http://www.w3.org/2004/02/skos/core#definition> "The act of criminal activity consisting of the repeated following and harassing of another person." .


###  https://purl.org/turbbo/RBBO_RC9p1nKgQCD9ZNR5vvX2qiZ
RBBO:RC9p1nKgQCD9ZNR5vvX2qiZ rdf:type owl:Class ;
                             rdfs:subClassOf RBBO:RCV5kFFQ8uWjqjPCrdjngHb ;
                             rdfs:label "Producing verbal communications" ;
                             <http://www.w3.org/2004/02/skos/core#definition> "The act or process of generating words to express information or to express your ideas, thoughts, feelings, etc., to someone else." .


###  https://purl.org/turbbo/RBBO_RCC63qDwHmigEz6huhl9dCG
RBBO:RCC63qDwHmigEz6huhl9dCG rdf:type owl:Class ;
                             rdfs:subClassOf RBBO:R74Nph6Q96RGCllk8UMt94p ;
                             rdfs:label "Flossing" ;
                             <http://www.w3.org/2004/02/skos/core#definition> "The use of waxed or unwaxed synthetic thread to dislodge plaque, foods and microbes from the lateral borders of teeth." .


###  https://purl.org/turbbo/RBBO_RCCIgPeUjgaKYDjePlHqzlm
RBBO:RCCIgPeUjgaKYDjePlHqzlm rdf:type owl:Class ;
                             rdfs:subClassOf RBBO:RDSprVXKVeqV4JtMjaGwwDX ;
                             rdfs:label "Artificial feeding" ;
                             <http://www.w3.org/2004/02/skos/core#definition> "The act of feeding a baby with food other than mother's milk." .


###  https://purl.org/turbbo/RBBO_RCD8LHOgE9WxbIcDhGHIuVW
RBBO:RCD8LHOgE9WxbIcDhGHIuVW rdf:type owl:Class ;
                             rdfs:subClassOf RBBO:RBOTVkkObNNllFP9EFEOIR2 ;
                             rdfs:label "Eating Candy" ;
                             <http://www.w3.org/2004/02/skos/core#definition> "The consumption of a sweet food made with sugar or syrup combined with fruit, chocolate, or nuts." .


###  https://purl.org/turbbo/RBBO_RCDJN2atxNwOBqbKSmxM1Fc
RBBO:RCDJN2atxNwOBqbKSmxM1Fc rdf:type owl:Class ;
                             rdfs:subClassOf RBBO:R7x8NHLRGEcEymTXMx3THX7 ;
                             rdfs:label "Adhering to medication/ treatment regime" ;
                             <http://www.w3.org/2004/02/skos/core#definition> "The act of abiding by a stated treatment plan or protocol." .


###  https://purl.org/turbbo/RBBO_RCDX7XRjZ177uHg6OoUyvv0
RBBO:RCDX7XRjZ177uHg6OoUyvv0 rdf:type owl:Class ;
                             rdfs:subClassOf RBBO:RayAVAeF9vXpz9v3jwSLzs ;
                             rdfs:label "Selling stolen property" ;
                             <http://www.w3.org/2004/02/skos/core#definition> "The act of giving or handing over property that does not belong to the possessor in exchange for money." .


###  https://purl.org/turbbo/RBBO_RCE7VvM7rpyKfsBJxKqHVvk
RBBO:RCE7VvM7rpyKfsBJxKqHVvk rdf:type owl:Class ;
                             rdfs:subClassOf RBBO:RC9p1nKgQCD9ZNR5vvX2qiZ ;
                             rdfs:label "Speaking" ;
                             <http://www.w3.org/2004/02/skos/core#definition> "The action of expressing one's thoughts and feelings in spoken language (includes for e.g. whining)" .


###  https://purl.org/turbbo/RBBO_RCKDQM6dfhit3RC352IGkgN
RBBO:RCKDQM6dfhit3RC352IGkgN rdf:type owl:Class ;
                             rdfs:subClassOf <https://purl.org/turbbo/RBBO_0000123> ;
                             rdfs:label "Engaging in mood / state changing activities and behavior" ;
                             <http://www.w3.org/2004/02/skos/core#definition> "Engaging in behaviors causing changes in the conscious state of mind or predominant emotion." .


###  https://purl.org/turbbo/RBBO_RCLGCfCEICjWDiyU2xYotQk
RBBO:RCLGCfCEICjWDiyU2xYotQk rdf:type owl:Class ;
                             rdfs:subClassOf <https://purl.org/turbbo/RBBO_0000123> ;
                             rdfs:label "Engaging in behavior related to major life areas" ;
                             <http://www.w3.org/2004/02/skos/core#definition> "Carrying out actions required to engage in education, work and employment and to conduct economic transactions, including the use of technologies." .


###  https://purl.org/turbbo/RBBO_RCLUrCDjw1iSB9E2K1K47IG
RBBO:RCLUrCDjw1iSB9E2K1K47IG rdf:type owl:Class ;
                             rdfs:subClassOf RBBO:RfZmso8v8XZptVF2vKaUQ3 ;
                             rdfs:label "Conserving energy" ;
                             <http://www.w3.org/2004/02/skos/core#definition> "To avoid wasteful use of power." .


###  https://purl.org/turbbo/RBBO_RCMQ2Xe8y2ROsQ2JODi10Pt
RBBO:RCMQ2Xe8y2ROsQ2JODi10Pt rdf:type owl:Class ;
                             rdfs:subClassOf RBBO:RCV0qw9GIXO9nA6mEsE72Nr ;
                             rdfs:label "Caring for household objects and non-human members" ;
                             <http://www.w3.org/2004/02/skos/core#definition> "To keep something in the household safe and provided for." .


###  https://purl.org/turbbo/RBBO_RCNXOEb6sjTOBSIrv5Z5Bfv
RBBO:RCNXOEb6sjTOBSIrv5Z5Bfv rdf:type owl:Class ;
                             rdfs:subClassOf RBBO:RDw1Q66ue2imTNF7lazEvKw ;
                             rdfs:label "Breaking and entering" ;
                             <http://www.w3.org/2004/02/skos/core#definition> "The act of entering a residence or other enclosed property through the slightest amount of force, without authorization." .


###  https://purl.org/turbbo/RBBO_RCQ0BGxWd0dw2Ax39GRhiqs
RBBO:RCQ0BGxWd0dw2Ax39GRhiqs rdf:type owl:Class ;
                             rdfs:subClassOf RBBO:RayAVAeF9vXpz9v3jwSLzs ;
                             rdfs:label "Not disclosing" ;
                             <http://www.w3.org/2004/02/skos/core#definition> "Not making requested information known." .


###  https://purl.org/turbbo/RBBO_RCTpYCPfulTB3fOxPqErQ2V
RBBO:RCTpYCPfulTB3fOxPqErQ2V rdf:type owl:Class ;
                             rdfs:subClassOf RBBO:RayAVAeF9vXpz9v3jwSLzs ;
                             rdfs:label "Drug dealing" ;
                             <http://www.w3.org/2004/02/skos/core#definition> "The act of giving or handing over drugs in exchange for money without a license from the state." .


###  https://purl.org/turbbo/RBBO_RCV0qw9GIXO9nA6mEsE72Nr
RBBO:RCV0qw9GIXO9nA6mEsE72Nr rdf:type owl:Class ;
                             rdfs:subClassOf <https://purl.org/turbbo/RBBO_0000123> ;
                             rdfs:label "Engaging in domestic life activities" ;
                             <http://www.w3.org/2004/02/skos/core#definition> "Carrying out domestic and everyday actions and tasks." .


###  https://purl.org/turbbo/RBBO_RCV5kFFQ8uWjqjPCrdjngHb
RBBO:RCV5kFFQ8uWjqjPCrdjngHb rdf:type owl:Class ;
                             rdfs:subClassOf RBBO:R6hKctZFZcjKJBLZwC7y9T ;
                             rdfs:label "Producing communications" ;
                             <http://www.w3.org/2004/02/skos/core#definition> "The act or process of generating words, sounds, signs, or behaviors to express information or to express your ideas, thoughts, feelings, etc., to someone else." .


###  https://purl.org/turbbo/RBBO_RCW6LwsmwRRJDHJ5Sw3NcqF
RBBO:RCW6LwsmwRRJDHJ5Sw3NcqF rdf:type owl:Class ;
                             rdfs:subClassOf RBBO:RCKDQM6dfhit3RC352IGkgN ;
                             rdfs:label "Using Marijuana" ;
                             <http://www.w3.org/2004/02/skos/core#definition> "The act of smoking the dried leaves and flowering tops of the pistillate hemp plant that yield THC." .


###  https://purl.org/turbbo/RBBO_RCX7sTnjz11ol0VKC4azwIC
RBBO:RCX7sTnjz11ol0VKC4azwIC rdf:type owl:Class ;
                             rdfs:subClassOf RBBO:R7ou7HEwYODwmkHhLtEqW2B ;
                             rdfs:label "Crawling" ;
                             <http://www.w3.org/2004/02/skos/core#definition> "Move forward on the hands and knees or by dragging the body close to the ground." .


###  https://purl.org/turbbo/RBBO_RCXasK8gbuKMgaU1ZrRXQZM
RBBO:RCXasK8gbuKMgaU1ZrRXQZM rdf:type owl:Class ;
                             rdfs:subClassOf RBBO:RCKDQM6dfhit3RC352IGkgN ;
                             rdfs:label "Using Cocaine" ;
                             <http://www.w3.org/2004/02/skos/core#definition> "The use of a tropane alkaloid that is obtained from the leaves of the coca plant." .


###  https://purl.org/turbbo/RBBO_RCcKEhZxYCpuN3rXXYRFoKa
RBBO:RCcKEhZxYCpuN3rXXYRFoKa rdf:type owl:Class ;
                             rdfs:subClassOf RBBO:RDqjiSX08Nc9xxSBrR5KMOM ;
                             rdfs:label "Listening" ;
                             <http://www.w3.org/2004/02/skos/core#definition> "To pay attention to someone or something in order to hear what is being said, sung, played, etc." .


###  https://purl.org/turbbo/RBBO_RCgGDn1vqlfJSIRaFveJ3LD
RBBO:RCgGDn1vqlfJSIRaFveJ3LD rdf:type owl:Class ;
                             rdfs:subClassOf RBBO:R9SZhlXBAdyrsI5ItrSRZDG ;
                             rdfs:label "Using contraceptive devices" ;
                             <http://www.w3.org/2004/02/skos/core#definition> "Use of a device or drug that serves to prevent a woman from becoming pregnant." .


###  https://purl.org/turbbo/RBBO_RCh5z0vk5UDzC46FZI7ew7i
RBBO:RCh5z0vk5UDzC46FZI7ew7i rdf:type owl:Class ;
                             rdfs:subClassOf RBBO:RCKDQM6dfhit3RC352IGkgN ;
                             rdfs:label "Using Alcohol" ;
                             <http://www.w3.org/2004/02/skos/core#definition> "The use of ethanol, a type of alcohol found in beverages, that acts as a central nervous system depressant." .


###  https://purl.org/turbbo/RBBO_RChrJYRTZRmBDhl2HTuXV4S
RBBO:RChrJYRTZRmBDhl2HTuXV4S rdf:type owl:Class ;
                             rdfs:subClassOf RBBO:R7x8NHLRGEcEymTXMx3THX7 ;
                             rdfs:label "Using health care/ participating in treatment" ;
                             <http://www.w3.org/2004/02/skos/core#definition> "The actions of prevention, treatment, and management of illness and the preservation of mental and physical wellbeing through the services offered by the medical and allied health professions." .


###  https://purl.org/turbbo/RBBO_RCij8AeR486wWQrvpxJI2KG
RBBO:RCij8AeR486wWQrvpxJI2KG rdf:type owl:Class ;
                             rdfs:subClassOf RBBO:RDarCRBoiqojsnZ9V6Oj1EU ;
                             rdfs:label "Sleeping" ;
                             <http://www.w3.org/2004/02/skos/core#definition> "Putting oneself into a condition of body and mind in which the nervous system is relatively inactive, the eyes closed, the postural muscles relaxed, and consciousness practically suspended." .


###  https://purl.org/turbbo/RBBO_RCj2g7DNklxWdnq0FhKcaUK
RBBO:RCj2g7DNklxWdnq0FhKcaUK rdf:type owl:Class ;
                             rdfs:subClassOf RBBO:RCkUmDEEBCZJdgoHyJUrlzm ;
                             rdfs:label "Engaging in behavior related to prostitution" ;
                             <http://www.w3.org/2004/02/skos/core#definition> "Engaging in sexual activity with someone in return for payment or as a customer." .


###  https://purl.org/turbbo/RBBO_RCkUmDEEBCZJdgoHyJUrlzm
RBBO:RCkUmDEEBCZJdgoHyJUrlzm rdf:type owl:Class ;
                             rdfs:subClassOf RBBO:R9XzdtCeE4Ytjbjkmi81yJu ;
                             rdfs:label "Engaging in behaviors related to intimate relationships" ;
                             <http://www.w3.org/2004/02/skos/core#definition> "Engaging in behaviors related to private and personal relationships; this may be in a sexual way." .


###  https://purl.org/turbbo/RBBO_RCoukmgJYw5wh7IXXRNL08T
RBBO:RCoukmgJYw5wh7IXXRNL08T rdf:type owl:Class ;
                             rdfs:subClassOf RBBO:R98L21up1SSyEgiLNxwvbKM ;
                             rdfs:label "Watching TV" ;
                             <http://www.w3.org/2004/02/skos/core#definition> "The act of watching television." .


###  https://purl.org/turbbo/RBBO_RCrDL1h6RMXEqgnkTmAzyNh
RBBO:RCrDL1h6RMXEqgnkTmAzyNh rdf:type owl:Class ;
                             rdfs:subClassOf RBBO:R9SZhlXBAdyrsI5ItrSRZDG ;
                             rdfs:label "Using safety restraints" ;
                             <http://www.w3.org/2004/02/skos/core#definition> "The use of devices (seat belt, car seat, booster seat, life belt, safety harness, etc.) in order to prevent getting hurt" .


###  https://purl.org/turbbo/RBBO_RCuyyZAZJSXGT3CbFA45RAJ
RBBO:RCuyyZAZJSXGT3CbFA45RAJ rdf:type owl:Class ;
                             rdfs:subClassOf RBBO:RFGrqCSRvAPz3uiW6oXcW7 ;
                             rdfs:label "Working with photography equipment" .


###  https://purl.org/turbbo/RBBO_RD0GMkoktmQ73gfqCl0qW1R
RBBO:RD0GMkoktmQ73gfqCl0qW1R rdf:type owl:Class ;
                             rdfs:subClassOf RBBO:R6hKctZFZcjKJBLZwC7y9T ;
                             rdfs:label "Receiving communications" ;
                             <http://www.w3.org/2004/02/skos/core#definition> "The act or process of receiving words, sounds, signs, or behaviors that express information." .


###  https://purl.org/turbbo/RBBO_RDB0WPFBq8eRpd2dUYyztb4
RBBO:RDB0WPFBq8eRpd2dUYyztb4 rdf:type owl:Class ;
                             rdfs:subClassOf RBBO:R7MZNxsxrHJFsQZe0BlH2P4 ;
                             rdfs:label "Engaging in civic involvement" ;
                             <http://www.w3.org/2004/02/skos/core#definition> "An action designed to identify and address issues of public concer." .


###  https://purl.org/turbbo/RBBO_RDCdADDJmSYz0KQPW8JeeEL
RBBO:RDCdADDJmSYz0KQPW8JeeEL rdf:type owl:Class ;
                             rdfs:subClassOf RBBO:RayAVAeF9vXpz9v3jwSLzs ;
                             rdfs:label "Carrying a weapon" ;
                             <http://www.w3.org/2004/02/skos/core#definition> "Holding a weapon, a device which primary purpose is to attack or defend against others." .


###  https://purl.org/turbbo/RBBO_RDD3rbWNSvbnzQEYVOzVTaf
RBBO:RDD3rbWNSvbnzQEYVOzVTaf rdf:type owl:Class ;
                             rdfs:subClassOf RBBO:Rb1xX794wVt3QQownZtSbO ;
                             rdfs:label "Go to and be present at a planned occasion or activity (such as a social gathering or sports program)." ;
                             <http://www.w3.org/2004/02/skos/core#definition> "Attending to a story or event recorded by a camera as a set of moving images and shown in a theater or on television." .


###  https://purl.org/turbbo/RBBO_RDGyOtjqZKCX0tefKkHlCB4
RBBO:RDGyOtjqZKCX0tefKkHlCB4 rdf:type owl:Class ;
                             rdfs:subClassOf RBBO:RDqjiSX08Nc9xxSBrR5KMOM ;
                             rdfs:label "Reading" ;
                             <http://www.w3.org/2004/02/skos/core#definition> "The action of looking at and comprehending the meaning of (written or printed matter) by mentally interpreting the characters or symbols of which it is composed." .


###  https://purl.org/turbbo/RBBO_RDHDhOpQRdVHIWshnX8texT
RBBO:RDHDhOpQRdVHIWshnX8texT rdf:type owl:Class ;
                             rdfs:subClassOf RBBO:RhlslZKl21SGb8L452uSU8 ;
                             rdfs:label "Accounting" ;
                             <http://www.w3.org/2004/02/skos/core#definition> "The act of keeping the financial records of a business or person." .


###  https://purl.org/turbbo/RBBO_RDIIAa0apBgWd6V8u5gqFdx
RBBO:RDIIAa0apBgWd6V8u5gqFdx rdf:type owl:Class ;
                             rdfs:subClassOf RBBO:RDck4eDShRuThnEF6Ql5OxH ;
                             rdfs:label "Crying" ;
                             <http://www.w3.org/2004/02/skos/core#definition> "Producing tears often while making loud sounds because of pain, sorrow, or other strong emotions." .


###  https://purl.org/turbbo/RBBO_RDJKU5nu0UQ99SqvzqDERuT
RBBO:RDJKU5nu0UQ99SqvzqDERuT rdf:type owl:Class ;
                             rdfs:subClassOf RBBO:R8cCVugnbr4KoPFPOy98Qt2 ;
                             rdfs:label "Being absent" ;
                             <http://www.w3.org/2004/02/skos/core#definition> "The practice of regularly staying away from work or school without valid reason" .


###  https://purl.org/turbbo/RBBO_RDL2jv9fzH1Qut883nyV9h2
RBBO:RDL2jv9fzH1Qut883nyV9h2 rdf:type owl:Class ;
                             rdfs:subClassOf RBBO:RDB0WPFBq8eRpd2dUYyztb4 ;
                             rdfs:label "Joining or maintaining membership in political organizations" ;
                             <http://www.w3.org/2004/02/skos/core#definition> "Participation in an organization that, on the basis of one or more shared concerns, attempts to influence public policy in its favour." .


###  https://purl.org/turbbo/RBBO_RDLYuvHGi7xCMFHwL7WJ8pF
RBBO:RDLYuvHGi7xCMFHwL7WJ8pF rdf:type owl:Class ;
                             rdfs:subClassOf RBBO:RC5cLYrHZhVyinK9OLpz4Ax ;
                             rdfs:label "Engaging in prosocial behavior" ;
                             <http://www.w3.org/2004/02/skos/core#definition> "Engaging in behavior which is positive, helpful, and intended to promote social acceptance and friendship." .


###  https://purl.org/turbbo/RBBO_RDNayceseHCIB2iSzFiUw1F
RBBO:RDNayceseHCIB2iSzFiUw1F rdf:type owl:Class ;
                             rdfs:subClassOf RBBO:R7pSWXD6d3tkoGLH56hjASm ;
                             rdfs:label "Engaging in strikes" ;
                             <http://www.w3.org/2004/02/skos/core#definition> "The act of stopping work in order to force an employer to comply with demands." .


###  https://purl.org/turbbo/RBBO_RDSprVXKVeqV4JtMjaGwwDX
RBBO:RDSprVXKVeqV4JtMjaGwwDX rdf:type owl:Class ;
                             rdfs:subClassOf RBBO:RBkPOivG8JaZijqer0ZkDjQ ;
                             rdfs:label "Feeding" ;
                             <http://www.w3.org/2004/02/skos/core#definition> "The act of giving food to someone else, often a child." .


###  https://purl.org/turbbo/RBBO_RDTyuOxxUCulUO8Mpp6qkok
RBBO:RDTyuOxxUCulUO8Mpp6qkok rdf:type owl:Class ;
                             rdfs:subClassOf RBBO:RDdB56hI5WEz1kELL2HbIdh ;
                             rdfs:label "Smoking Water pipe" ;
                             <http://www.w3.org/2004/02/skos/core#definition> "The use of a device for smoking in which the tobacco smoke passes through water before it is inhaled." .


###  https://purl.org/turbbo/RBBO_RDUJWELA0SPaErG3vHbdX4L
RBBO:RDUJWELA0SPaErG3vHbdX4L rdf:type owl:Class ;
                             rdfs:subClassOf RBBO:R7ou7HEwYODwmkHhLtEqW2B ;
                             rdfs:label "Stretching" ;
                             <http://www.w3.org/2004/02/skos/core#definition> "Straighten or extend one’s body or a part of one’s body to its full length, typically so as to tighten one’s muscles." .


###  https://purl.org/turbbo/RBBO_RDUbufE2Nf82qL40OOzDf0X
RBBO:RDUbufE2Nf82qL40OOzDf0X rdf:type owl:Class ;
                             rdfs:subClassOf RBBO:RFGrqCSRvAPz3uiW6oXcW7 ;
                             rdfs:label "Participating in lesson" .


###  https://purl.org/turbbo/RBBO_RDUvbq2izGgpt3kOUvTN7DN
RBBO:RDUvbq2izGgpt3kOUvTN7DN rdf:type owl:Class ;
                             rdfs:subClassOf RBBO:RChrJYRTZRmBDhl2HTuXV4S ;
                             rdfs:label "Participating in Physician treatment" ;
                             <http://www.w3.org/2004/02/skos/core#definition> "The actions of treatment of illness through the services offered by the medical professions." .


###  https://purl.org/turbbo/RBBO_RDWlGjHDqw1graeSapdOC8q
RBBO:RDWlGjHDqw1graeSapdOC8q rdf:type owl:Class ;
                             rdfs:subClassOf RBBO:R8QKq0DUYbu1hFlkFQbcDqz ;
                             rdfs:label "Terminating a job" ;
                             <http://www.w3.org/2004/02/skos/core#definition> "To cause a job to end." .


###  https://purl.org/turbbo/RBBO_RDZT0VWQEBqvPfHRPJBiyVO
RBBO:RDZT0VWQEBqvPfHRPJBiyVO rdf:type owl:Class ;
                             rdfs:subClassOf RBBO:RDLYuvHGi7xCMFHwL7WJ8pF ;
                             rdfs:label "Providing informational support" ;
                             <http://www.w3.org/2004/02/skos/core#definition> "To give help or assistance through providing information." .


###  https://purl.org/turbbo/RBBO_RDarCRBoiqojsnZ9V6Oj1EU
RBBO:RDarCRBoiqojsnZ9V6Oj1EU rdf:type owl:Class ;
                             rdfs:subClassOf RBBO:R7x8NHLRGEcEymTXMx3THX7 ;
                             rdfs:label "Recuperating" ;
                             <http://www.w3.org/2004/02/skos/core#definition> "Actions taken to recover from sickness or exhaustion and to regain health or strength." .


###  https://purl.org/turbbo/RBBO_RDazgYyfZxs7cSniOP0LqUl
RBBO:RDazgYyfZxs7cSniOP0LqUl rdf:type owl:Class ;
                             rdfs:subClassOf RBBO:RDdB56hI5WEz1kELL2HbIdh ;
                             rdfs:label "Using Oral tobacco" ;
                             <http://www.w3.org/2004/02/skos/core#definition> "The use of tobacco that is placed in the mouth between the cheek and the gum." .


###  https://purl.org/turbbo/RBBO_RDcFnYzsIyED62rWslUIgsQ
RBBO:RDcFnYzsIyED62rWslUIgsQ rdf:type owl:Class ;
                             rdfs:subClassOf RBBO:RCKDQM6dfhit3RC352IGkgN ,
                                             RBBO:RDWlGjHDqw1graeSapdOC8q ;
                             rdfs:label "Quitting or resigning from a job" ;
                             <http://www.w3.org/2004/02/skos/core#definition> "The act of giving up (a job or position) in a formal or official way." .


###  https://purl.org/turbbo/RBBO_RDck4eDShRuThnEF6Ql5OxH
RBBO:RDck4eDShRuThnEF6Ql5OxH rdf:type owl:Class ;
                             rdfs:subClassOf RBBO:RCV5kFFQ8uWjqjPCrdjngHb ;
                             rdfs:label "Producing non-verbal communications" ;
                             <http://www.w3.org/2004/02/skos/core#definition> "The act of communication not involving or using words." .


###  https://purl.org/turbbo/RBBO_RDd9PVm2VkoGBq6nc5q376d
RBBO:RDd9PVm2VkoGBq6nc5q376d rdf:type owl:Class ;
                             rdfs:subClassOf RBBO:RDB0WPFBq8eRpd2dUYyztb4 ;
                             rdfs:label "Donating" ;
                             <http://www.w3.org/2004/02/skos/core#definition> "The act of freely offering time, goods, money or expertise for a civic involvement." .


###  https://purl.org/turbbo/RBBO_RDdB56hI5WEz1kELL2HbIdh
RBBO:RDdB56hI5WEz1kELL2HbIdh rdf:type owl:Class ;
                             rdfs:subClassOf RBBO:RCKDQM6dfhit3RC352IGkgN ;
                             rdfs:label "Using Tobacco" ;
                             <http://www.w3.org/2004/02/skos/core#definition> "The use of the tobacco plant leaf and its product." .


###  https://purl.org/turbbo/RBBO_RDdnDizb7yQLTGidIQACx7C
RBBO:RDdnDizb7yQLTGidIQACx7C rdf:type owl:Class ;
                             rdfs:subClassOf RBBO:R7qzqygnfKwMVxUR9f0qbNZ ;
                             rdfs:label "Drinking Soda" ;
                             <http://www.w3.org/2004/02/skos/core#definition> "The consumption of a sweet, carbonate, nonalcoholic beverage." .


###  https://purl.org/turbbo/RBBO_RDeUwnwxfKUS5E5xlwbtwQP
RBBO:RDeUwnwxfKUS5E5xlwbtwQP rdf:type owl:Class ;
                             rdfs:subClassOf RBBO:RayAVAeF9vXpz9v3jwSLzs ;
                             rdfs:label "Using property of others without consent" ;
                             <http://www.w3.org/2004/02/skos/core#definition> "The act of using someone else´s property without owners permission." .


###  https://purl.org/turbbo/RBBO_RDmKjBpNIWwc0pUklW7MzjR
RBBO:RDmKjBpNIWwc0pUklW7MzjR rdf:type owl:Class ;
                             rdfs:subClassOf RBBO:R9SZhlXBAdyrsI5ItrSRZDG ;
                             rdfs:label "Using hearing protection" ;
                             <http://www.w3.org/2004/02/skos/core#definition> "The use of hearing protection devices when exposed to high noise." .


###  https://purl.org/turbbo/RBBO_RDn0ZVSM2vfmu81DdUnDKoA
RBBO:RDn0ZVSM2vfmu81DdUnDKoA rdf:type owl:Class ;
                             rdfs:subClassOf RBBO:R9BeiQh4oa8EbuNm1bjryZB ;
                             rdfs:label "Applying to a job" ;
                             <http://www.w3.org/2004/02/skos/core#definition> "To ask formally for work that a person does regularly in order to earn money." .


###  https://purl.org/turbbo/RBBO_RDnuf6OklKW1hXGCl6f1FQ
RBBO:RDnuf6OklKW1hXGCl6f1FQ rdf:type owl:Class ;
                            rdfs:subClassOf RBBO:RD0GMkoktmQ73gfqCl0qW1R ;
                            rdfs:label "Gathering information" ;
                            <http://www.w3.org/2004/02/skos/core#definition> "The act of collecting information." .


###  https://purl.org/turbbo/RBBO_RDqjiSX08Nc9xxSBrR5KMOM
RBBO:RDqjiSX08Nc9xxSBrR5KMOM rdf:type owl:Class ;
                             rdfs:subClassOf <https://purl.org/turbbo/RBBO_0000123> ;
                             rdfs:label "Engaging in learning and applying knowledge" ;
                             <http://www.w3.org/2004/02/skos/core#definition> "The acquisition or application of knowledge or skills through study, experience, or being taught." .


###  https://purl.org/turbbo/RBBO_RDqrSoVPQjxqqJkRCeAY7Fh
RBBO:RDqrSoVPQjxqqJkRCeAY7Fh rdf:type owl:Class ;
                             rdfs:subClassOf RBBO:R7MWXGKIGLx4ykI6IfNRWHF ;
                             rdfs:label "Engaging in educational parenting" ;
                             <http://www.w3.org/2004/02/skos/core#definition> "The process of taking care of children's educational well being until they are old enough to take care of this themselves." .


###  https://purl.org/turbbo/RBBO_RDvb6aFUJwVt0s07bERv9DR
RBBO:RDvb6aFUJwVt0s07bERv9DR rdf:type owl:Class ;
                             rdfs:subClassOf RBBO:R7pSWXD6d3tkoGLH56hjASm ;
                             rdfs:label "Engaging in Political contact" ;
                             <http://www.w3.org/2004/02/skos/core#definition> "Communication with a political actor." .


###  https://purl.org/turbbo/RBBO_RDw1Q66ue2imTNF7lazEvKw
RBBO:RDw1Q66ue2imTNF7lazEvKw rdf:type owl:Class ;
                             rdfs:subClassOf RBBO:R7LFMgbt35Cfkx42ektsTEV ;
                             rdfs:label "Engaging in aggressive behavior" ;
                             <http://www.w3.org/2004/02/skos/core#definition> "Behavior that causes or threatens harm to other people." .


###  https://purl.org/turbbo/RBBO_RDw3qFlleEQPLNjw6ZGTd8Z
RBBO:RDw3qFlleEQPLNjw6ZGTd8Z rdf:type owl:Class ;
                             rdfs:subClassOf RBBO:R7MWXGKIGLx4ykI6IfNRWHF ;
                             rdfs:label "Attending school" ;
                             <http://www.w3.org/2004/02/skos/core#definition> "The action or process of teaching a child." .


###  https://purl.org/turbbo/RBBO_RDxp8Bwy2X738H5qxan42Bw
RBBO:RDxp8Bwy2X738H5qxan42Bw rdf:type owl:Class ;
                             rdfs:subClassOf RBBO:RDWlGjHDqw1graeSapdOC8q ;
                             rdfs:label "Retiring from a job" ;
                             <http://www.w3.org/2004/02/skos/core#definition> "The withdrawal from one's position or occupation or from active working life." .


###  https://purl.org/turbbo/RBBO_RDyZolgzJg2qTtAOywxH2yy
RBBO:RDyZolgzJg2qTtAOywxH2yy rdf:type owl:Class ;
                             rdfs:subClassOf RBBO:RhlslZKl21SGb8L452uSU8 ;
                             rdfs:label "Acquiring goods and services" ;
                             <http://www.w3.org/2004/02/skos/core#definition> "The act of acquiring (something) permanently or temporarily." .


###  https://purl.org/turbbo/RBBO_RDylVUTN7gssLSu1xP0nJDa
RBBO:RDylVUTN7gssLSu1xP0nJDa rdf:type owl:Class ;
                             rdfs:subClassOf RBBO:R7pSWXD6d3tkoGLH56hjASm ;
                             rdfs:label "Blocking traffic" ;
                             <http://www.w3.org/2004/02/skos/core#definition> "The action or process of obstructing movement, progress, or activity within traffic." .


###  https://purl.org/turbbo/RBBO_RDyt3Gqf4k8WR1xaRJAj1Kx
RBBO:RDyt3Gqf4k8WR1xaRJAj1Kx rdf:type owl:Class ;
                             rdfs:subClassOf RBBO:R8cCVugnbr4KoPFPOy98Qt2 ;
                             rdfs:label "Departing early" ;
                             <http://www.w3.org/2004/02/skos/core#definition> "To go away from work before the usual or expected time." .


###  https://purl.org/turbbo/RBBO_RDzsFgl9xnDJkw9zXLWULAv
RBBO:RDzsFgl9xnDJkw9zXLWULAv rdf:type owl:Class ;
                             rdfs:subClassOf RBBO:RCLGCfCEICjWDiyU2xYotQk ;
                             rdfs:label "Using technology" ;
                             <http://www.w3.org/2004/02/skos/core#definition> "Engaging in a task using technical processes, methods, or knowledge." .


###  https://purl.org/turbbo/RBBO_RELGFPbeTmyA8dwf248hdf
RBBO:RELGFPbeTmyA8dwf248hdf rdf:type owl:Class ;
                            rdfs:subClassOf RBBO:RayAVAeF9vXpz9v3jwSLzs ;
                            rdfs:label "Accepting stolen property" ;
                            <http://www.w3.org/2004/02/skos/core#definition> "The act of receiving/taking possession of property that does not belong to the possesor." .


###  https://purl.org/turbbo/RBBO_RELjqe9K96RTVusFCzO665
RBBO:RELjqe9K96RTVusFCzO665 rdf:type owl:Class ;
                            rdfs:subClassOf RBBO:RDqrSoVPQjxqqJkRCeAY7Fh ;
                            rdfs:label "Attending school event" ;
                            <http://www.w3.org/2004/02/skos/core#definition> "To go and be present at a school event." .


###  https://purl.org/turbbo/RBBO_REmsFQNMuh3CGKcGBuBLfF
RBBO:REmsFQNMuh3CGKcGBuBLfF rdf:type owl:Class ;
                            rdfs:subClassOf RBBO:RFGrqCSRvAPz3uiW6oXcW7 ;
                            rdfs:label "Hunting" ;
                            <http://www.w3.org/2004/02/skos/core#definition> "To pursue and kill (a wild animal) for sport or food." .


###  https://purl.org/turbbo/RBBO_RFFvgJZOVt9s4BsxZOe4Ns
RBBO:RFFvgJZOVt9s4BsxZOe4Ns rdf:type owl:Class ;
                            rdfs:subClassOf RBBO:R3GTM1WIfB3LofIOVpVVKU ;
                            rdfs:label "Ingesting Protein" ;
                            <http://www.w3.org/2004/02/skos/core#definition> "Ingesting a group of complex organic macromolecules composed of one or more chains (linear polymers) of alpha-L-amino acids linked by peptide bonds and ranging in size from a few thousand to over 1 million Daltons. Proteins are fundamental genetically encoded components of living cells with specific structures and functions dictated by amino acid sequence." .


###  https://purl.org/turbbo/RBBO_RFGrqCSRvAPz3uiW6oXcW7
RBBO:RFGrqCSRvAPz3uiW6oXcW7 rdf:type owl:Class ;
                            rdfs:subClassOf RBBO:RWnX1GwU1D6dWspenC31cx ;
                            rdfs:label "Participating in hobbies/activities" ;
                            <http://www.w3.org/2004/02/skos/core#definition> "A pursuit outside one's regular occupation engaged in especially for relaxation" .


###  https://purl.org/turbbo/RBBO_RFrfRW4dhbwIoLOXGRCUib
RBBO:RFrfRW4dhbwIoLOXGRCUib rdf:type owl:Class ;
                            rdfs:subClassOf RBBO:R7qzqygnfKwMVxUR9f0qbNZ ;
                            rdfs:label "Drinking Coffee" ;
                            <http://www.w3.org/2004/02/skos/core#definition> "The consumption of a drink made from the roasted and ground beanlike seeds of a tropical shrub." .


###  https://purl.org/turbbo/RBBO_RG0IfHhxAote9X1WUd2rEY
RBBO:RG0IfHhxAote9X1WUd2rEY rdf:type owl:Class ;
                            rdfs:subClassOf RBBO:R7uK2tMCWgORKYlpKazgtMt ;
                            rdfs:label "Eating Baked goods" ;
                            <http://www.w3.org/2004/02/skos/core#definition> "Consumption of food products that have been baked in an oven." .


###  https://purl.org/turbbo/RBBO_RG968kLWRO6N5z8H6WWozU
RBBO:RG968kLWRO6N5z8H6WWozU rdf:type owl:Class ;
                            rdfs:subClassOf RBBO:RDqrSoVPQjxqqJkRCeAY7Fh ;
                            rdfs:label "Visiting class" ;
                            <http://www.w3.org/2004/02/skos/core#definition> "To go and be present at a class session." .


###  https://purl.org/turbbo/RBBO_RHPyU2gwOKLNfkBzKpbdcX
RBBO:RHPyU2gwOKLNfkBzKpbdcX rdf:type owl:Class ;
                            rdfs:subClassOf RBBO:R7MWXGKIGLx4ykI6IfNRWHF ,
                                            RBBO:Rj9feeEPPMDelLiPVmOGiu ;
                            rdfs:label "Teaching" ;
                            <http://www.w3.org/2004/02/skos/core#definition> "To cause or help (someone) to learn about a subject." .


###  https://purl.org/turbbo/RBBO_RINOST75D6djkBWwq9c5bA
RBBO:RINOST75D6djkBWwq9c5bA rdf:type owl:Class ;
                            rdfs:subClassOf RBBO:RCkUmDEEBCZJdgoHyJUrlzm ;
                            rdfs:label "Engaging in sexually intimate actions" ;
                            <http://www.w3.org/2004/02/skos/core#definition> "The act of private and personal sexual interactions." .


###  https://purl.org/turbbo/RBBO_RJO6iC2VRzba8WErTMzjVY
RBBO:RJO6iC2VRzba8WErTMzjVY rdf:type owl:Class ;
                            rdfs:subClassOf RBBO:R7MZNxsxrHJFsQZe0BlH2P4 ;
                            rdfs:label "Supporting a political campaign" ;
                            <http://www.w3.org/2004/02/skos/core#definition> "Offering support for an organized effort which seeks to influence the decision making process within a specific group. Often refers to electoral campaigns, wherein representatives are chosen or referendums are decided" .


###  https://purl.org/turbbo/RBBO_RKywIOxd28NpHngBGOrhmM
RBBO:RKywIOxd28NpHngBGOrhmM rdf:type owl:Class ;
                            rdfs:subClassOf RBBO:RCE7VvM7rpyKfsBJxKqHVvk ;
                            rdfs:label "Speaking to a child" ;
                            <http://www.w3.org/2004/02/skos/core#definition> "The [parent] talks to the child." .


###  https://purl.org/turbbo/RBBO_RM8IEbYCf0Lh0sCY12xysa
RBBO:RM8IEbYCf0Lh0sCY12xysa rdf:type owl:Class ;
                            rdfs:subClassOf RBBO:R7pSWXD6d3tkoGLH56hjASm ;
                            rdfs:label "Engaging in boycotts" ;
                            <http://www.w3.org/2004/02/skos/core#definition> "A punitive ban that forbids relations with certain groups, cooperation with a policy, or the handling of goods." .


###  https://purl.org/turbbo/RBBO_RNHPFDfx1RIGUC2DxGVclA
RBBO:RNHPFDfx1RIGUC2DxGVclA rdf:type owl:Class ;
                            rdfs:subClassOf RBBO:RCMQ2Xe8y2ROsQ2JODi10Pt ;
                            rdfs:label "Taking care of animals" ;
                            <http://www.w3.org/2004/02/skos/core#definition> "To keep an animal in the household safe and provided for." .


###  https://purl.org/turbbo/RBBO_RPOb1PeqNWQMEmR8PP3vzy
RBBO:RPOb1PeqNWQMEmR8PP3vzy rdf:type owl:Class ;
                            rdfs:subClassOf RBBO:RDw1Q66ue2imTNF7lazEvKw ;
                            rdfs:label "Engaging in sexual assault" ;
                            <http://www.w3.org/2004/02/skos/core#definition> "The act of illegal sexual contact that usually involves force upon a person without consent or is inflicted upon a person who is incapable of giving consent." .


###  https://purl.org/turbbo/RBBO_RPbzQu9FJJx3Wc4aXHN7J1
RBBO:RPbzQu9FJJx3Wc4aXHN7J1 rdf:type owl:Class ;
                            rdfs:subClassOf RBBO:RDw1Q66ue2imTNF7lazEvKw ;
                            rdfs:label "Fighting physically" ;
                            <http://www.w3.org/2004/02/skos/core#definition> "The act of using physical force to try to hurt someone, to defeat an enemy." .


###  https://purl.org/turbbo/RBBO_RR373pfhTV9IFDQ05dFELW
RBBO:RR373pfhTV9IFDQ05dFELW rdf:type owl:Class ;
                            rdfs:subClassOf RBBO:RCKDQM6dfhit3RC352IGkgN ;
                            rdfs:label "Using Inhalants" ;
                            <http://www.w3.org/2004/02/skos/core#definition> "The use of substances that produce chemical vapors that can be inhaled to induce a psychoactive, or mind-altering, effect." .


###  https://purl.org/turbbo/RBBO_RRaNdhCF3dVWlKQXqMvKaa
RBBO:RRaNdhCF3dVWlKQXqMvKaa rdf:type owl:Class ;
                            rdfs:subClassOf RBBO:RDd9PVm2VkoGBq6nc5q376d ;
                            rdfs:label "Research participation" ;
                            <http://www.w3.org/2004/02/skos/core#definition> "The act of participating as an individual that is observed, analyzed, examined, investigated, experimented upon, or/and treated in the course of a particular study." .


###  https://purl.org/turbbo/RBBO_RWXCHZrMMzfJByqIOBrpTw
RBBO:RWXCHZrMMzfJByqIOBrpTw rdf:type owl:Class ;
                            rdfs:subClassOf RBBO:RDSprVXKVeqV4JtMjaGwwDX ;
                            rdfs:label "Breastfeeding" ;
                            <http://www.w3.org/2004/02/skos/core#definition> "The act of nursing (a baby) at the breast; suckling" .


###  https://purl.org/turbbo/RBBO_RWnX1GwU1D6dWspenC31cx
RBBO:RWnX1GwU1D6dWspenC31cx rdf:type owl:Class ;
                            rdfs:subClassOf RBBO:RC5cLYrHZhVyinK9OLpz4Ax ;
                            rdfs:label "Engaging in recreation and leisure activities" ;
                            <http://www.w3.org/2004/02/skos/core#definition> "Engaging in activities that provide refreshment of one's mind or body after work, through amusement or play." .


###  https://purl.org/turbbo/RBBO_RY0zoHgTUlb8DRG5uu94K8
RBBO:RY0zoHgTUlb8DRG5uu94K8 rdf:type owl:Class ;
                            rdfs:subClassOf RBBO:RDLYuvHGi7xCMFHwL7WJ8pF ;
                            rdfs:label "Providing emotional support" ;
                            <http://www.w3.org/2004/02/skos/core#definition> "Engaging in behavior which provides sympathy and encouragement." .


###  https://purl.org/turbbo/RBBO_RayAVAeF9vXpz9v3jwSLzs
RBBO:RayAVAeF9vXpz9v3jwSLzs rdf:type owl:Class ;
                            rdfs:subClassOf RBBO:R7LFMgbt35Cfkx42ektsTEV ;
                            rdfs:label "Engaging in non-aggressive antisocial behavior" ;
                            <http://www.w3.org/2004/02/skos/core#definition> "Non-violent behaviors that harm or lack consideration for the well-being of others." .


###  https://purl.org/turbbo/RBBO_Rb1xX794wVt3QQownZtSbO
RBBO:Rb1xX794wVt3QQownZtSbO rdf:type owl:Class ;
                            rdfs:subClassOf RBBO:RWnX1GwU1D6dWspenC31cx ;
                            rdfs:label "Attending Events" ;
                            <http://www.w3.org/2004/02/skos/core#definition> "Go to and be present at a planned occasion or activity (such as a social gathering or sports program)." .


###  https://purl.org/turbbo/RBBO_RbNf7VEy1PxZ0dorTHM9JL
RBBO:RbNf7VEy1PxZ0dorTHM9JL rdf:type owl:Class ;
                            rdfs:subClassOf RBBO:RDw1Q66ue2imTNF7lazEvKw ;
                            rdfs:label "Intimidating with weapon" ;
                            <http://www.w3.org/2004/02/skos/core#definition> "The act of using an instrument of combat, designed to injure or kill, in an attempt to persuade anothers actions." .


###  https://purl.org/turbbo/RBBO_RbTyaBi2bOHP4ozQoWEII
RBBO:RbTyaBi2bOHP4ozQoWEII rdf:type owl:Class ;
                           rdfs:subClassOf RBBO:R8qMM1AUIWkGs9uIR3zf0Oe ;
                           rdfs:label "Reading spiritual text" ;
                           <http://www.w3.org/2004/02/skos/core#definition> "Engaging in activities that provide refreshment of one's mind or body after work, through amusement or play." .


###  https://purl.org/turbbo/RBBO_Rca0mn9wW01cj6QOf4AzGS
RBBO:Rca0mn9wW01cj6QOf4AzGS rdf:type owl:Class ;
                            rdfs:subClassOf RBBO:RhlslZKl21SGb8L452uSU8 ;
                            rdfs:label "Selling" ;
                            <http://www.w3.org/2004/02/skos/core#definition> "To exchange (something) for money." .


###  https://purl.org/turbbo/RBBO_ReGfCA6kmPSboQD5R1oatV
RBBO:ReGfCA6kmPSboQD5R1oatV rdf:type owl:Class ;
                            rdfs:subClassOf RBBO:R3GTM1WIfB3LofIOVpVVKU ;
                            rdfs:label "Ingesting Cholesterol" ;
                            <http://www.w3.org/2004/02/skos/core#definition> "Ingesting an animal sterol found in the body tissues (and blood plasma) of vertebrates." .


###  https://purl.org/turbbo/RBBO_RegBtmSAlhPnzgmfSUeTLH
RBBO:RegBtmSAlhPnzgmfSUeTLH rdf:type owl:Class ;
                            rdfs:subClassOf RBBO:RCcKEhZxYCpuN3rXXYRFoKa ;
                            rdfs:label "Listening to music" ;
                            <http://www.w3.org/2004/02/skos/core#definition> "To pay attention to in order to hear to music that is being sung / played." .


###  https://purl.org/turbbo/RBBO_Rf9oqhtZCda9LIk7oVS9DU
RBBO:Rf9oqhtZCda9LIk7oVS9DU rdf:type owl:Class ;
                            rdfs:subClassOf RBBO:RayAVAeF9vXpz9v3jwSLzs ;
                            rdfs:label "Engaging in truancy" ;
                            <http://www.w3.org/2004/02/skos/core#definition> "The action of staying away from school without good reason; absenteeism." .


###  https://purl.org/turbbo/RBBO_RfZmso8v8XZptVF2vKaUQ3
RBBO:RfZmso8v8XZptVF2vKaUQ3 rdf:type owl:Class ;
                            rdfs:subClassOf RBBO:R7MZNxsxrHJFsQZe0BlH2P4 ;
                            rdfs:label "Protecting the environment" ;
                            <http://www.w3.org/2004/02/skos/core#definition> "Keeping the environment from being harmed." .


###  https://purl.org/turbbo/RBBO_RfwrrDcashsZzpYX32Y8lP
RBBO:RfwrrDcashsZzpYX32Y8lP rdf:type owl:Class ;
                            rdfs:subClassOf RBBO:RDqjiSX08Nc9xxSBrR5KMOM ;
                            rdfs:label "Drawing" ;
                            <http://www.w3.org/2004/02/skos/core#definition> "The act or art of making a picture, image, etc., with a pencil, pen, marker, chalk, etc., but usually not with paint." .


###  https://purl.org/turbbo/RBBO_RhlslZKl21SGb8L452uSU8
RBBO:RhlslZKl21SGb8L452uSU8 rdf:type owl:Class ;
                            rdfs:subClassOf RBBO:RCLGCfCEICjWDiyU2xYotQk ;
                            rdfs:label "Engaging in basic economic transactions" ;
                            <http://www.w3.org/2004/02/skos/core#definition> "Engaging in actions where economic value is provided by exchange between parties." .


###  https://purl.org/turbbo/RBBO_RhzG71ht01mQ8JDhza2Wzi
RBBO:RhzG71ht01mQ8JDhza2Wzi rdf:type owl:Class ;
                            rdfs:subClassOf RBBO:R3GTM1WIfB3LofIOVpVVKU ;
                            rdfs:label "Ingesting Carbohydrate" ;
                            <http://www.w3.org/2004/02/skos/core#definition> "Ingesting any one of various substances found in certain foods (such as bread, rice, and potatoes) that provide your body with heat and energy and are made of carbon, hydrogen, and oxygen." .


###  https://purl.org/turbbo/RBBO_Rj9feeEPPMDelLiPVmOGiu
RBBO:Rj9feeEPPMDelLiPVmOGiu rdf:type owl:Class ;
                            rdfs:subClassOf RBBO:RCLGCfCEICjWDiyU2xYotQk ;
                            rdfs:label "Engaging in informal education" ;
                            <http://www.w3.org/2004/02/skos/core#definition> "Participating in learning activities outside the formal school setting that develop a person mentally, morally, or aesthetically." .


###  https://purl.org/turbbo/RBBO_RlI7OyT2VtC81reSeMdoLh
RBBO:RlI7OyT2VtC81reSeMdoLh rdf:type owl:Class ;
                            rdfs:subClassOf RBBO:R7uK2tMCWgORKYlpKazgtMt ;
                            rdfs:label "Eating Fruits" ;
                            <http://www.w3.org/2004/02/skos/core#definition> "The consumption of the usually edible reproductive body of a seed plant." .


###  https://purl.org/turbbo/RBBO_RlMYAo16e5oslcFDCdrGii
RBBO:RlMYAo16e5oslcFDCdrGii rdf:type owl:Class ;
                            rdfs:subClassOf RBBO:RBZBFZG9PRFJpm31aToI1nl ;
                            rdfs:label "Having oral intercourse" ;
                            <http://www.w3.org/2004/02/skos/core#definition> "The act of sexual activity in which the genitals of one partner are stimulated by the mouth of the other; fellatio or cunnilingus." .


###  https://purl.org/turbbo/RBBO_RlnJeTriFA2gqojpzOKehu
RBBO:RlnJeTriFA2gqojpzOKehu rdf:type owl:Class ;
                            rdfs:subClassOf RBBO:RFGrqCSRvAPz3uiW6oXcW7 ;
                            rdfs:label "Collecting" ;
                            <http://www.w3.org/2004/02/skos/core#definition> "Engaging in the process of bringing or gathering something together." .


###  https://purl.org/turbbo/RBBO_RmSYcVyGoF5Juc2czWvFKJ
RBBO:RmSYcVyGoF5Juc2czWvFKJ rdf:type owl:Class ;
                            rdfs:subClassOf RBBO:RJO6iC2VRzba8WErTMzjVY ;
                            rdfs:label "Hanging posters" ;
                            <http://www.w3.org/2004/02/skos/core#definition> "To suspend a large printed picture containing a political message." .


###  https://purl.org/turbbo/RBBO_RmsFbX68kZa0rYXa7PeIG7
RBBO:RmsFbX68kZa0rYXa7PeIG7 rdf:type owl:Class ;
                            rdfs:subClassOf RBBO:R3NO3LpXB5rQZlwHyBqraH ;
                            rdfs:label "Cleaning" ;
                            <http://www.w3.org/2004/02/skos/core#definition> "An act of making a place clean or tidy." .


###  https://purl.org/turbbo/RBBO_Rpw8QahfkN1ulHg1owtelv
RBBO:Rpw8QahfkN1ulHg1owtelv rdf:type owl:Class ;
                            rdfs:subClassOf RBBO:R7uK2tMCWgORKYlpKazgtMt ;
                            rdfs:label "Eating Ice-cream" ;
                            <http://www.w3.org/2004/02/skos/core#definition> "The consumption of a sweet flavored frozen food containing cream or butterfat and usually eggs" .


###  https://purl.org/turbbo/RBBO_Rr9R5cDg7RRsQSbJS1vKnM
RBBO:Rr9R5cDg7RRsQSbJS1vKnM rdf:type owl:Class ;
                            rdfs:subClassOf RBBO:R7ou7HEwYODwmkHhLtEqW2B ;
                            rdfs:label "Walking" ;
                            <http://www.w3.org/2004/02/skos/core#definition> "Move at a regular pace by lifting and setting down each foot in turn, never having both feet off the ground at once." .


###  https://purl.org/turbbo/RBBO_RrE6zfKvWJJOOuww3AlZlr
RBBO:RrE6zfKvWJJOOuww3AlZlr rdf:type owl:Class ;
                            rdfs:subClassOf RBBO:R7x8NHLRGEcEymTXMx3THX7 ;
                            rdfs:label "Taking medication" ;
                            <http://www.w3.org/2004/02/skos/core#definition> "The act of taking a dose of medication into one's body (e.g., by swallowing, drinking, or inhaling)." .


###  https://purl.org/turbbo/RBBO_RsTw4zzwI41RORImDRdsGM
RBBO:RsTw4zzwI41RORImDRdsGM rdf:type owl:Class ;
                            rdfs:subClassOf RBBO:RDw1Q66ue2imTNF7lazEvKw ;
                            rdfs:label "Verbally abusing" ;
                            <http://www.w3.org/2004/02/skos/core#definition> "The act of using words that attack or injure an individual or words that constitute psychological violence." .


###  https://purl.org/turbbo/RBBO_RsaqqjBS39mUXYl1xpaRIM
RBBO:RsaqqjBS39mUXYl1xpaRIM rdf:type owl:Class ;
                            rdfs:subClassOf RBBO:RDqrSoVPQjxqqJkRCeAY7Fh ;
                            rdfs:label "Speaking with school staff" ;
                            <http://www.w3.org/2004/02/skos/core#definition> "Expressing one's thoughts and feelings in spoken language to a school employee." .


###  https://purl.org/turbbo/RBBO_Ru3YYyTyH8kcXOiDkhHurf
RBBO:Ru3YYyTyH8kcXOiDkhHurf rdf:type owl:Class ;
                            rdfs:subClassOf RBBO:RayAVAeF9vXpz9v3jwSLzs ;
                            rdfs:label "Swearing" ;
                            <http://www.w3.org/2004/02/skos/core#definition> "The use offensive words when speaking" .


###  https://purl.org/turbbo/RBBO_Ruc1Jl3zFXAQnNutAfVIK4
RBBO:Ruc1Jl3zFXAQnNutAfVIK4 rdf:type owl:Class ;
                            rdfs:subClassOf RBBO:R93z8pYrtnWwimDtpP76jOC ;
                            rdfs:label "Opening account" ;
                            <http://www.w3.org/2004/02/skos/core#definition> "The act of making an account open (typically on anticipation of financial transactions)." .


###  https://purl.org/turbbo/RBBO_RwxCVUZQX5SqouSShk7A5I
RBBO:RwxCVUZQX5SqouSShk7A5I rdf:type owl:Class ;
                            rdfs:subClassOf RBBO:R7MWXGKIGLx4ykI6IfNRWHF ;
                            rdfs:label "Enrolling in school" ;
                            <http://www.w3.org/2004/02/skos/core#definition> "Officially register as a student on a course." .


###  https://purl.org/turbbo/RBBO_Rx25R848f1ANoSDNsmEr4q
RBBO:Rx25R848f1ANoSDNsmEr4q rdf:type owl:Class ;
                            rdfs:subClassOf RBBO:RCMQ2Xe8y2ROsQ2JODi10Pt ;
                            rdfs:label "Doing repairs" ;
                            <http://www.w3.org/2004/02/skos/core#definition> "To fix or mend something suffering from damage or a fault." .


###  https://purl.org/turbbo/RBBO_RxoQIYkqSzILenRDzAon83
RBBO:RxoQIYkqSzILenRDzAon83 rdf:type owl:Class ;
                            rdfs:subClassOf RBBO:RBuoEsSFBhOGJtFyQKJv3yx ;
                            rdfs:label "Help-seeking" ;
                            <http://www.w3.org/2004/02/skos/core#definition> "Request assistance to make it easier for someone to do a job, to deal with a problem, etc." .


###  https://purl.org/turbbo/RBBO_Ry90zmHK5VM4cDr1CuYXSp
RBBO:Ry90zmHK5VM4cDr1CuYXSp rdf:type owl:Class ;
                            rdfs:subClassOf RBBO:R7ksLdc5AtNZogZjcdwMAz ;
                            rdfs:label "Gambling" ;
                            <http://www.w3.org/2004/02/skos/core#definition> "The act of playing a game in which you can win or lose money or possessions." .


###  https://purl.org/turbbo/RBBO_RzLZVHATcpg9utyb6Wrz8n
RBBO:RzLZVHATcpg9utyb6Wrz8n rdf:type owl:Class ;
                            rdfs:subClassOf RBBO:R3GTM1WIfB3LofIOVpVVKU ;
                            rdfs:label "Ingesting Calcium" ;
                            <http://www.w3.org/2004/02/skos/core#definition> "Ingesting a silver-white divalent metallic element of the alkaline-earth group occurring only in combination." .


###  https://purl.org/turbbo/RBBO_RzlNZjf1nvIoW4m63l9QJP
RBBO:RzlNZjf1nvIoW4m63l9QJP rdf:type owl:Class ;
                            rdfs:subClassOf RBBO:RJO6iC2VRzba8WErTMzjVY ;
                            rdfs:label "Painting slogans" ;
                            <http://www.w3.org/2004/02/skos/core#definition> "The process or art of using paint to mark a brief attention-getting phrase used in advertising or promotion." .


###  Generated by the OWL API (version 4.5.24.2023-01-14T21:28:32Z) https://github.com/owlcs/owlapi
