@prefix : <https://purl.org/turbbo/RBBO_behaviour_properties.owl#> .
@prefix owl: <http://www.w3.org/2002/07/owl#> .
@prefix rdf: <http://www.w3.org/1999/02/22-rdf-syntax-ns#> .
@prefix xml: <http://www.w3.org/XML/1998/namespace> .
@prefix xsd: <http://www.w3.org/2001/XMLSchema#> .
@prefix rdfs: <http://www.w3.org/2000/01/rdf-schema#> .
@base <https://purl.org/turbbo/RBBO_behaviour_properties.owl> .

<https://purl.org/turbbo/RBBO_behaviour_properties.owl> rdf:type owl:Ontology ;
                                                         rdfs:comment """RBBO - Behaviour properties

This module of RBBO consists of classes and data properties which describe the characteristics of behaviours.""" ;
                                                         owl:versionInfo "2023-07-17" .

#################################################################
#    Annotation properties
#################################################################

###  http://purl.obolibrary.org/obo/IAO_0000115
<http://purl.obolibrary.org/obo/IAO_0000115> rdf:type owl:AnnotationProperty .


###  http://purl.obolibrary.org/obo/IAO_0000116
<http://purl.obolibrary.org/obo/IAO_0000116> rdf:type owl:AnnotationProperty .


###  http://purl.org/dc/elements/1.1/title
<http://purl.org/dc/elements/1.1/title> rdf:type owl:AnnotationProperty .


###  http://www.geneontology.org/formats/oboInOwl#created_by
<http://www.geneontology.org/formats/oboInOwl#created_by> rdf:type owl:AnnotationProperty .


###  http://www.geneontology.org/formats/oboInOwl#creation_date
<http://www.geneontology.org/formats/oboInOwl#creation_date> rdf:type owl:AnnotationProperty .


###  http://www.w3.org/2004/02/skos/core#definition
<http://www.w3.org/2004/02/skos/core#definition> rdf:type owl:AnnotationProperty .


###  https://purl.org/turbbo/RBBO_0000150
<https://purl.org/turbbo/RBBO_0000150> rdf:type owl:AnnotationProperty .


#################################################################
#    Object Properties
#################################################################

###  https://purl.org/turbbo/RBBO_0000085
<https://purl.org/turbbo/RBBO_0000085> rdf:type owl:ObjectProperty ;
                                       rdfs:label "occurs before" .


###  https://purl.org/turbbo/RBBO_0000086
<https://purl.org/turbbo/RBBO_0000086> rdf:type owl:ObjectProperty ;
                                       rdfs:label "occurs after" .


###  https://purl.org/turbbo/RBBO_0000089
<https://purl.org/turbbo/RBBO_0000089> rdf:type owl:ObjectProperty ;
                                       rdfs:label "composed of" .


###  https://purl.org/turbbo/RBBO_0000092
<https://purl.org/turbbo/RBBO_0000092> rdf:type owl:ObjectProperty ;
                                       rdfs:range <https://purl.org/turbbo/RBBO_0000107> ;
                                       rdfs:label "facilitated by" .


###  https://purl.org/turbbo/RBBO_0000094
<https://purl.org/turbbo/RBBO_0000094> rdf:type owl:ObjectProperty ;
                                       rdfs:range <https://purl.org/turbbo/RBBO_0000143> ;
                                       rdfs:label "has effectiveness" .


###  https://purl.org/turbbo/RBBO_0000096
<https://purl.org/turbbo/RBBO_0000096> rdf:type owl:ObjectProperty ;
                                       rdfs:range <https://purl.org/turbbo/RBBO_0000105> ;
                                       rdfs:label "has goal" .


###  https://purl.org/turbbo/RBBO_0000097
<https://purl.org/turbbo/RBBO_0000097> rdf:type owl:ObjectProperty ;
                                       rdfs:range <https://purl.org/turbbo/RBBO_0000112> ;
                                       rdfs:label "has impact" .


###  https://purl.org/turbbo/RBBO_0000098
<https://purl.org/turbbo/RBBO_0000098> rdf:type owl:ObjectProperty ;
                                       rdfs:range <https://purl.org/turbbo/RBBO_0000110> ;
                                       rdfs:label "has intention" .


###  https://purl.org/turbbo/RBBO_0000099
<https://purl.org/turbbo/RBBO_0000099> rdf:type owl:ObjectProperty ;
                                       rdfs:range <https://purl.org/turbbo/RBBO_0000121> ;
                                       rdfs:label "has legality" .


###  https://purl.org/turbbo/RBBO_0000103
<https://purl.org/turbbo/RBBO_0000103> rdf:type owl:ObjectProperty ;
                                       rdfs:domain <https://purl.org/turbbo/RBBO_0000124> ;
                                       rdfs:range <https://purl.org/turbbo/RBBO_0000144> ;
                                       rdfs:label "has type" .


###  https://purl.org/turbbo/RBBO_0000108
<https://purl.org/turbbo/RBBO_0000108> rdf:type owl:ObjectProperty ;
                                       rdfs:range <https://purl.org/turbbo/RBBO_0000126> ;
                                       rdfs:label "is reflective of" .


###  https://purl.org/turbbo/RBBO_0000111
<https://purl.org/turbbo/RBBO_0000111> rdf:type owl:ObjectProperty ;
                                       rdfs:domain <https://purl.org/turbbo/RBBO_0000112> ,
                                                   <https://purl.org/turbbo/RBBO_0000125> ,
                                                   <https://purl.org/turbbo/RBBO_0000143> ;
                                       rdfs:label "measured by" .


###  https://purl.org/turbbo/RBBO_0000117
<https://purl.org/turbbo/RBBO_0000117> rdf:type owl:ObjectProperty ;
                                       rdfs:range <https://purl.org/turbbo/RBBO_0000124> ;
                                       rdfs:label "motivated by" .


###  https://purl.org/turbbo/RBBO_0000118
<https://purl.org/turbbo/RBBO_0000118> rdf:type owl:ObjectProperty ;
                                       rdfs:label "occurs in" .


###  https://purl.org/turbbo/RBBO_0000119
<https://purl.org/turbbo/RBBO_0000119> rdf:type owl:ObjectProperty ;
                                       rdfs:range <https://purl.org/turbbo/RBBO_0000125> ;
                                       rdfs:label "occurs within" .


###  https://purl.org/turbbo/RBBO_0000128
<https://purl.org/turbbo/RBBO_0000128> rdf:type owl:ObjectProperty ;
                                       rdfs:range <https://purl.org/turbbo/RBBO_0000148> ;
                                       rdfs:label "requires skill" .


###  https://purl.org/turbbo/RBBO_0000129
<https://purl.org/turbbo/RBBO_0000129> rdf:type owl:ObjectProperty ;
                                       rdfs:range <https://purl.org/turbbo/RBBO_0000120> ;
                                       rdfs:label "restricted by" .


###  https://purl.org/turbbo/RBBO_0000130
<https://purl.org/turbbo/RBBO_0000130> rdf:type owl:ObjectProperty ;
                                       rdfs:domain <https://purl.org/turbbo/RBBO_0000110> ;
                                       rdfs:range <https://purl.org/turbbo/RBBO_0000105> ;
                                       rdfs:label "to achieve" .


#################################################################
#    Data properties
#################################################################

###  https://purl.org/turbbo/RBBO_0000001
<https://purl.org/turbbo/RBBO_0000001> rdf:type owl:DatatypeProperty ;
                                       rdfs:range xsd:boolean ;
                                       rdfs:comment """\"https://link.springer.com/chapter/10.1007/978-3-030-54994-7_32
Deliberate behaviour is driven by a goal, which not only depends on the knowledge domain but also on a representation of the goal achievement. This representation may be given by a combination of perceptions, actions and cognitive information.\" (Harriet Baird 4th April 2023)

This paper might be useful: https://bpspsychub.onlinelibrary.wiley.com/doi/full/10.1348/014466606X152261
\"It was theorised that deliberate behaviour is distinguished from spontaneous behaviour with respect to the amount of cognitive effort used in making the decision to carry out the particular behaviour\" ((Harriet Baird 4th April 2023)""" ,
                                                    "Is this the same as \"is intentional\"? I was tempted to define \"is deliberate\" as intentional behaviour." ;
                                       rdfs:label "is deliberate" ;
                                       <http://www.w3.org/2004/02/skos/core#definition> "Deliberate behaviour is driven by a goal, which not only depends on the knowledge domain but also on a representation of the goal achievement. (from https://link.springer.com/chapter/10.1007/978-3-030-54994-7_32)" .


###  https://purl.org/turbbo/RBBO_0000002
<https://purl.org/turbbo/RBBO_0000002> rdf:type owl:DatatypeProperty ;
                                       rdfs:range xsd:boolean ;
                                       rdfs:label "is changeable" ;
                                       <http://www.w3.org/2004/02/skos/core#definition> "Behaviour that is liable to variation" .


###  https://purl.org/turbbo/RBBO_0000004
<https://purl.org/turbbo/RBBO_0000004> rdf:type owl:DatatypeProperty ;
                                       rdfs:range xsd:boolean ;
                                       rdfs:comment "\"There are other ontologies that use differen definitions - e.g., A pattern of repeat behavior requiring little conscious thought - NCIT & GSSO An acquired pattern of behavior that often occurs automatically and is reliably triggered by some event or stimulus. - COGAT\" (Harriet Baird 4th April 2023)" ;
                                       rdfs:label "is habitual" ;
                                       <http://www.w3.org/2004/02/skos/core#definition> "A behaviour that results from a learnt stimulus-behaviour co-occurrence (Source: definition imported from the Behaviour Change Intervention Ontology (BCIO), via Qeios.)" .


###  https://purl.org/turbbo/RBBO_0000005
<https://purl.org/turbbo/RBBO_0000005> rdf:type owl:DatatypeProperty ;
                                       rdfs:range xsd:boolean ;
                                       rdfs:label "is heterogenous" ;
                                       <http://www.w3.org/2004/02/skos/core#definition> "The behaviour has a \"uniform consistency or composition\" (Source: National Cancer Institute Thesaurus via Bioportal)" .


###  https://purl.org/turbbo/RBBO_0000007
<https://purl.org/turbbo/RBBO_0000007> rdf:type owl:DatatypeProperty ;
                                       rdfs:range xsd:boolean ;
                                       rdfs:label "is legal" ;
                                       <http://www.w3.org/2004/02/skos/core#definition> "The behaviour meets the requirements under law; is not in violation of law or anything related to the law. (Source: National Cancer Institute. Legal. NCI Thesaurus. Code C54074, via Qeios)" .


###  https://purl.org/turbbo/RBBO_0000008
<https://purl.org/turbbo/RBBO_0000008> rdf:type owl:DatatypeProperty ;
                                       rdfs:range xsd:boolean ;
                                       rdfs:label "is moral" ;
                                       <http://www.w3.org/2004/02/skos/core#definition> "A moral behavior is one that is motivated by an explicit recognition of the prescriptive force of moral rules (Narvaez & Lapsley, 2005) or A moral behaviour is an acceptable way of life in a given society. This acceptable way of life or code of conduct is informed by religious beliefs, cultural beliefs, social beliefs, etc." .


###  https://purl.org/turbbo/RBBO_0000009
<https://purl.org/turbbo/RBBO_0000009> rdf:type owl:DatatypeProperty ;
                                       rdfs:range xsd:boolean ;
                                       rdfs:comment "May need to separate behaviour that is new to the individual from behaviour that is completely new (although perhaps the latter is so uncommon, that the property means new to the individual?)" ;
                                       rdfs:label "is new" ;
                                       <http://www.w3.org/2004/02/skos/core#definition> "Having no previous example or precedent or parallel; of a kind not seen before. (Source: National Cancer Institute. New. NCI Thesaurus. Code C25586.)" .


###  https://purl.org/turbbo/RBBO_0000010
<https://purl.org/turbbo/RBBO_0000010> rdf:type owl:DatatypeProperty ;
                                       rdfs:range xsd:boolean ;
                                       rdfs:comment """\"But there is a definition for behavioural opportunity \"An environmental disposition that enables or facilitates a behaviour.\" This definition was imported from the Behaviour Change Intervention Ontology (see https://bciovocab.org/). Comments and suggestions for improvements are welcome using the Qeios review system.\" (Harriet Baird on 4th April 2023)

\"Perhaps we could draw on the distinction between intentions and willingness here - e.g., opportuniistic behaviour \"is not intended, but rather results from a behavioural opportunity, defined as \"an environmental disposition that enables of facilitates a behaviour\"?\" (ThomasW 15th April 2023)""" ;
                                       rdfs:label "is opportunistic" ;
                                       <http://www.w3.org/2004/02/skos/core#definition> "Behaviour that is not intended, but rather results from a behavioural opportunity (\"an environmental disposition that enables of facilitates a behaviour\"). This definition was imported from the Behaviour Change Intervention Ontology (see https://bciovocab.org/)." .


###  https://purl.org/turbbo/RBBO_0000011
<https://purl.org/turbbo/RBBO_0000011> rdf:type owl:DatatypeProperty ;
                                       rdfs:range xsd:boolean ;
                                       rdfs:label "is optional" ;
                                       <http://www.w3.org/2004/02/skos/core#definition> "Possible but not necessary; left to personal choice. (Source: National Cancer Institute. Optional. NCI Thesaurus. Code C25603.)" .


###  https://purl.org/turbbo/RBBO_0000301
<https://purl.org/turbbo/RBBO_0000301> rdf:type owl:DatatypeProperty ;
                                       rdfs:comment "Maybe we need separate properties or \"Is abnormal for the individual\" and \"is abnormal for society\"? There is another definition of Qeios of abnormal which states \"Deviating in any way from the state, position, structure, condition, behavior, or rule which is considered a norm.\" (National Cancer Institute. Abnormal. NCI Thesaurus. Code C25401)" ;
                                       rdfs:label "is abnormal"^^xsd:string ;
                                       <http://www.w3.org/2004/02/skos/core#definition> "Conduct that is unusual for the individual. (Source: National Cancer Institute. Abnormal Behavior. NCI Thesaurus. Code C122430, via Qeios)" .


###  https://purl.org/turbbo/RBBO_0000303
<https://purl.org/turbbo/RBBO_0000303> rdf:type owl:DatatypeProperty ;
                                       rdfs:label "is adaptive"@en ;
                                       <http://www.w3.org/2004/02/skos/core#definition> "Adaptive behaviors are learned behaviors that reflect an individual's social and practical competence to meet the demands of everyday living (American Association on Intellectual and Developmental Disabilities)" .


###  https://purl.org/turbbo/RBBO_0000304
<https://purl.org/turbbo/RBBO_0000304> rdf:type owl:DatatypeProperty ;
                                       rdfs:label "is automatic"@en .


###  https://purl.org/turbbo/RBBO_0000305
<https://purl.org/turbbo/RBBO_0000305> rdf:type owl:DatatypeProperty ;
                                       rdfs:label "is consistent with self-identity"@en ;
                                       <http://www.w3.org/2004/02/skos/core#definition> "Behaviour that expresses the person's identity (where self-identity is defined as \"An identity that a person has about themselves\" from the Addiction Ontology, Qeios ID: FDB3BI.2)" .


###  https://purl.org/turbbo/RBBO_0000306
<https://purl.org/turbbo/RBBO_0000306> rdf:type owl:DatatypeProperty ;
                                       rdfs:comment "Challenge here is whose definition of desirable? And at the time of the behaviour or later?" ;
                                       rdfs:label "is desirable"@en ;
                                       <http://www.w3.org/2004/02/skos/core#definition> "An evaluative belief about the value of the consequences of behaviour (Source: This definition was imported from the Behaviour Change Intervention Ontology (see https://bciovocab.org/), via Qeois - edited slightly)." .


###  https://purl.org/turbbo/RBBO_0000307
<https://purl.org/turbbo/RBBO_0000307> rdf:type owl:DatatypeProperty ;
                                       rdfs:label "is impulsive"@en ;
                                       <http://www.w3.org/2004/02/skos/core#definition> "Initiation of actions without forethought as to the cost, results or consequences. (Source: National Cancer Institute. Impulsive Behavior. NCI Thesaurus. Code C93213.)" .


###  https://purl.org/turbbo/RBBO_0000308
<https://purl.org/turbbo/RBBO_0000308> rdf:type owl:DatatypeProperty ;
                                       rdfs:label "is intentional"@en ;
                                       <http://www.w3.org/2004/02/skos/core#definition> "Intentional behavior is a goal-directed activity whereby perceptions are sought and actions performed in service of the needs of the organism (Harter & Kozma, 2021)" .


###  https://purl.org/turbbo/RBBO_0000309
<https://purl.org/turbbo/RBBO_0000309> rdf:type owl:DatatypeProperty ;
                                       rdfs:label "is learned"@en ;
                                       <http://www.w3.org/2004/02/skos/core#definition> "A mental disposition to behave in a particular way in response to an internal or external event in the person's environment, which is acquired through habit learning. (Source:This definition was imported from the Behaviour Change Intervention Ontology (see https://bciovocab.org/). Comments and suggestions for improvements are welcome using the Qeios review system, via Qeios)" .


###  https://purl.org/turbbo/RBBO_0000310
<https://purl.org/turbbo/RBBO_0000310> rdf:type owl:DatatypeProperty ;
                                       rdfs:label "is normative"@en ;
                                       <http://www.w3.org/2004/02/skos/core#definition> "An individual human behaviour that is commonly enacted by people that are part of a social environmental system. This definition was imported from the Behaviour Change Intervention Ontology (see https://bciovocab.org/). Qeios ID: VYZF1Y" .


###  https://purl.org/turbbo/RBBO_0000311
<https://purl.org/turbbo/RBBO_0000311> rdf:type owl:DatatypeProperty ;
                                       rdfs:label "is physical"@en ;
                                       <http://www.w3.org/2004/02/skos/core#definition> "A behaviour that involves a musculoskeletal process in its realisation. (Source: This definition was imported from the Behaviour Change Intervention Ontology (see https://bciovocab.org/). Comments and suggestions for improvements are welcome using the Qeios review system - slightly edited to remove \"capability\")" .


###  https://purl.org/turbbo/RBBO_0000312
<https://purl.org/turbbo/RBBO_0000312> rdf:type owl:DatatypeProperty ;
                                       rdfs:label "is pleasurable"@en ;
                                       <http://www.w3.org/2004/02/skos/core#definition> "Pleasure (an emotion associated with feeling good) that is experienced as a result of engaging in a behaviour. Overall this definition was reused from the Behaviour Change Intervention Ontology (see https://bciovocab.org/) and augmented with a definition of pleasure from National Cancer Institute. Pleasure. NCI Thesaurus. Code C86580." .


###  https://purl.org/turbbo/RBBO_0000313
<https://purl.org/turbbo/RBBO_0000313> rdf:type owl:DatatypeProperty ;
                                       rdfs:label "is rational"@en ;
                                       <http://www.w3.org/2004/02/skos/core#definition> "Behaviour that is based on or in accordance with reason or logic." .


###  https://purl.org/turbbo/RBBO_0000314
<https://purl.org/turbbo/RBBO_0000314> rdf:type owl:DatatypeProperty ;
                                       rdfs:label "is repetitive"@en .


###  https://purl.org/turbbo/RBBO_0000315
<https://purl.org/turbbo/RBBO_0000315> rdf:type owl:DatatypeProperty ;
                                       rdfs:label "is spontaneous"@en ;
                                       <http://www.w3.org/2004/02/skos/core#definition> "Behaviour that happens or arised without apparent external cause. Adapted from definition of spontaneous from the National Cancer Institute. Spontaneous. NCI Thesaurus. Code C48307." .


#################################################################
#    Classes
#################################################################

###  https://purl.org/turbbo/RBBO_0000003
<https://purl.org/turbbo/RBBO_0000003> rdf:type owl:Class ;
                                       rdfs:subClassOf <https://purl.org/turbbo/RBBO_0000144> ;
                                       <http://www.geneontology.org/formats/oboInOwl#created_by> "ThomasW"^^xsd:string ;
                                       <http://www.geneontology.org/formats/oboInOwl#creation_date> "2023-10-30T13:46:29.117726Z"^^xsd:string ;
                                       rdfs:label "Habitual"@en ;
                                       <http://www.w3.org/2004/02/skos/core#definition> "A behaviour that results from a learnt stimulus-behaviour co-occurrence"^^xsd:string .


###  https://purl.org/turbbo/RBBO_0000006
<https://purl.org/turbbo/RBBO_0000006> rdf:type owl:Class ;
                                       <http://www.geneontology.org/formats/oboInOwl#created_by> "ThomasW"^^xsd:string ;
                                       <http://www.geneontology.org/formats/oboInOwl#creation_date> "2023-10-30T14:24:49.070593Z"^^xsd:string ;
                                       rdfs:label "Correlates with"@en .


###  https://purl.org/turbbo/RBBO_0000012
<https://purl.org/turbbo/RBBO_0000012> rdf:type owl:Class ;
                                       rdfs:subClassOf <https://purl.org/turbbo/RBBO_0000018> ;
                                       <http://www.geneontology.org/formats/oboInOwl#created_by> "ThomasW"^^xsd:string ;
                                       <http://www.geneontology.org/formats/oboInOwl#creation_date> "2023-10-30T13:53:58.369001Z"^^xsd:string ;
                                       rdfs:label "Effort"@en ;
                                       <http://www.w3.org/2004/02/skos/core#definition> "Requires physical or mental energy; hard work."^^xsd:string .


###  https://purl.org/turbbo/RBBO_0000013
<https://purl.org/turbbo/RBBO_0000013> rdf:type owl:Class ;
                                       rdfs:subClassOf <https://purl.org/turbbo/RBBO_0000144> ;
                                       <http://www.geneontology.org/formats/oboInOwl#created_by> "ThomasW"^^xsd:string ;
                                       <http://www.geneontology.org/formats/oboInOwl#creation_date> "2023-10-30T13:59:12.478398Z"^^xsd:string ;
                                       rdfs:label "Changeable"@en .


###  https://purl.org/turbbo/RBBO_0000014
<https://purl.org/turbbo/RBBO_0000014> rdf:type owl:Class ;
                                       rdfs:subClassOf <https://purl.org/turbbo/RBBO_0000124> ;
                                       <http://www.geneontology.org/formats/oboInOwl#created_by> "ThomasW"^^xsd:string ;
                                       <http://www.geneontology.org/formats/oboInOwl#creation_date> "2023-10-30T14:00:33.283443Z"^^xsd:string ;
                                       rdfs:label "Unintended"@en .


###  https://purl.org/turbbo/RBBO_0000015
<https://purl.org/turbbo/RBBO_0000015> rdf:type owl:Class ;
                                       rdfs:subClassOf <https://purl.org/turbbo/RBBO_0000144> ;
                                       <http://www.geneontology.org/formats/oboInOwl#created_by> "ThomasW"^^xsd:string ;
                                       <http://www.geneontology.org/formats/oboInOwl#creation_date> "2023-10-30T14:02:24.279538Z"^^xsd:string ;
                                       rdfs:label "Illegal"@en ;
                                       <http://www.w3.org/2004/02/skos/core#definition> "The behaviour is not allowed by the law (edited from: https://dictionary.cambridge.org/dictionary/english/legality)"^^xsd:string .


###  https://purl.org/turbbo/RBBO_0000016
<https://purl.org/turbbo/RBBO_0000016> rdf:type owl:Class ;
                                       rdfs:subClassOf <https://purl.org/turbbo/RBBO_0000125> ;
                                       <http://www.geneontology.org/formats/oboInOwl#created_by> "ThomasW"^^xsd:string ;
                                       <http://www.geneontology.org/formats/oboInOwl#creation_date> "2023-10-30T14:04:00.35628Z"^^xsd:string ;
                                       rdfs:label "Outside"@en .


###  https://purl.org/turbbo/RBBO_0000017
<https://purl.org/turbbo/RBBO_0000017> rdf:type owl:Class ;
                                       rdfs:subClassOf <https://purl.org/turbbo/RBBO_0000125> ;
                                       <http://www.geneontology.org/formats/oboInOwl#created_by> "ThomasW"^^xsd:string ;
                                       <http://www.geneontology.org/formats/oboInOwl#creation_date> "2023-10-30T14:04:06.998649Z"^^xsd:string ;
                                       rdfs:label "Inside"@en .


###  https://purl.org/turbbo/RBBO_0000018
<https://purl.org/turbbo/RBBO_0000018> rdf:type owl:Class ;
                                       <http://www.geneontology.org/formats/oboInOwl#created_by> "ThomasW"^^xsd:string ;
                                       <http://www.geneontology.org/formats/oboInOwl#creation_date> "2023-10-30T14:08:55.746298Z"^^xsd:string ;
                                       rdfs:label "Involves"@en ;
                                       <http://www.w3.org/2004/02/skos/core#definition> "Performance of the behaviour involves (i.e., is rarely possible without a minimum level of) one or more of the following"^^xsd:string .


###  https://purl.org/turbbo/RBBO_0000019
<https://purl.org/turbbo/RBBO_0000019> rdf:type owl:Class ;
                                       rdfs:subClassOf <https://purl.org/turbbo/RBBO_0000006> ;
                                       <http://www.geneontology.org/formats/oboInOwl#created_by> "ThomasW"^^xsd:string ;
                                       <http://www.geneontology.org/formats/oboInOwl#creation_date> "2023-10-30T14:25:21.698913Z"^^xsd:string ;
                                       rdfs:label "largeCorrelation"@en ;
                                       <http://www.w3.org/2004/02/skos/core#definition> "r = 0.50 (Cohen, 1992)"^^xsd:string .


###  https://purl.org/turbbo/RBBO_0000020
<https://purl.org/turbbo/RBBO_0000020> rdf:type owl:Class ;
                                       rdfs:subClassOf <https://purl.org/turbbo/RBBO_0000006> ;
                                       <http://www.geneontology.org/formats/oboInOwl#created_by> "ThomasW"^^xsd:string ;
                                       <http://www.geneontology.org/formats/oboInOwl#creation_date> "2023-10-30T14:25:31.013765Z"^^xsd:string ;
                                       rdfs:label "mediumCorrelation"@en ;
                                       <http://www.w3.org/2004/02/skos/core#definition> "r = 0.30 (Cohen, 1992)"^^xsd:string .


###  https://purl.org/turbbo/RBBO_0000021
<https://purl.org/turbbo/RBBO_0000021> rdf:type owl:Class ;
                                       rdfs:subClassOf <https://purl.org/turbbo/RBBO_0000006> ;
                                       <http://www.geneontology.org/formats/oboInOwl#created_by> "ThomasW"^^xsd:string ;
                                       <http://www.geneontology.org/formats/oboInOwl#creation_date> "2023-10-30T14:25:42.293692Z"^^xsd:string ;
                                       rdfs:label "smallCorrelation"@en ;
                                       <http://www.w3.org/2004/02/skos/core#definition> "r = 0.10 (Cohen, 1992)"^^xsd:string .


###  https://purl.org/turbbo/RBBO_0000105
<https://purl.org/turbbo/RBBO_0000105> rdf:type owl:Class ;
                                       rdfs:subClassOf <https://purl.org/turbbo/RBBO_0000124> ;
                                       rdfs:label "Goal-directed"^^xsd:string ;
                                       <http://www.w3.org/2004/02/skos/core#definition> "Goal = \"Internal representations of desired states, where states are broadly construed as outcomes, events, or processes.\" (Austin & Vancouver 1996, p. 338)"^^xsd:string ,
                                                                                        """Goal = A cognitive representation of an end state towards which one is striving.
(BCIO - https://www.bciovocab.org/BCIO:006049) Qeios (https://www.qeios.com/read/6M8C05)"""^^xsd:string ,
                                                                                        "Goal = The end state toward which a human is striving: the purpose of an activity or endeavor. (edited from: https://dictionary.apa.org/goal)"^^xsd:string .


###  https://purl.org/turbbo/RBBO_0000107
<https://purl.org/turbbo/RBBO_0000107> rdf:type owl:Class ;
                                       rdfs:label "Facilitated by"^^xsd:string ;
                                       <http://www.w3.org/2004/02/skos/core#definition> "A factor that facilitates or supports performance of a behaviour" ,
                                                                                        "Something that facilities or supports progress or the achievement of an ultimate objective or end." .


###  https://purl.org/turbbo/RBBO_0000110
<https://purl.org/turbbo/RBBO_0000110> rdf:type owl:Class ;
                                       rdfs:subClassOf <https://purl.org/turbbo/RBBO_0000124> ;
                                       rdfs:label "Intended"^^xsd:string ;
                                       <http://www.w3.org/2004/02/skos/core#definition> """A mental disposition to commit to enact or not enact a behaviour.
(BCIO - https://www.bciovocab.org/BCIO:006016) Qeios (https://www.qeios.com/read/5FTW17)""" ,
                                                                                        "A prior conscious decision to perform a behavior. (https://dictionary.apa.org/intention)" ,
                                                                                        "Behavioural intentions are assumed to capture the motivational factors that influence a behaviour” and to indicate “how hard people are willing to try, or how much effort they would exert to perform a behaviour” (Ajzen, 1991, p. 181)" .


###  https://purl.org/turbbo/RBBO_0000112
<https://purl.org/turbbo/RBBO_0000112> rdf:type owl:Class ;
                                       rdfs:label "Impact" ;
                                       <http://www.w3.org/2004/02/skos/core#definition> "The effect of the behaviour on someone or something." .


###  https://purl.org/turbbo/RBBO_0000120
<https://purl.org/turbbo/RBBO_0000120> rdf:type owl:Class ;
                                       rdfs:label "Barriers to"^^xsd:string ;
                                       <http://www.w3.org/2004/02/skos/core#definition> "A factor that hinders or obstructs performance of a behaviour" ,
                                                                                        "Barrier: Something that restricts, impedes, or blocks progress or the achievement of an ultimate objective or end. (https://dictionary.apa.org/barrier)"^^xsd:string .


###  https://purl.org/turbbo/RBBO_0000121
<https://purl.org/turbbo/RBBO_0000121> rdf:type owl:Class ;
                                       rdfs:subClassOf <https://purl.org/turbbo/RBBO_0000144> ;
                                       rdfs:label "Legal"^^xsd:string ;
                                       <http://www.w3.org/2004/02/skos/core#definition> "The behaviour is allowed by the law (edited from: https://dictionary.cambridge.org/dictionary/english/legality)"^^xsd:string .


###  https://purl.org/turbbo/RBBO_0000124
<https://purl.org/turbbo/RBBO_0000124> rdf:type owl:Class ;
                                       rdfs:label "Motivation" ;
                                       <http://www.w3.org/2004/02/skos/core#definition> """A mental process that energises and directs behaviour.
(BCIO - https://www.bciovocab.org/BCIO:006133) Qeios (https://www.qeios.com/read/U92HTU)""" ,
                                                                                        "The impetus that gives purpose or direction to behavior and operates in humans at a conscious or unconscious level. (https://dictionary.apa.org/motivation)" .


###  https://purl.org/turbbo/RBBO_0000125
<https://purl.org/turbbo/RBBO_0000125> rdf:type owl:Class ;
                                       rdfs:label "Context" ;
                                       <http://www.w3.org/2004/02/skos/core#definition> "The conditions or circumstances in which a particular behaviour occurs (edited from https://dictionary.apa.org/context)" ,
                                                                                        "The time, place or setting in which a behaviour takes place." .


###  https://purl.org/turbbo/RBBO_0000126
<https://purl.org/turbbo/RBBO_0000126> rdf:type owl:Class ;
                                       rdfs:subClassOf <https://purl.org/turbbo/RBBO_0000144> ;
                                       rdfs:label "Consistent with actors identity"^^xsd:string ;
                                       <http://www.w3.org/2004/02/skos/core#definition> """A cognitive representation of themselves by a person or group.
(BCIO - https://www.bciovocab.org/ADDICTO:0000381)""" ,
                                                                                        "An individual’s sense of self defined by (a) a set of physical, psychological, and interpersonal characteristics that is not wholly shared with any other person and (b) a range of affiliations (e.g., ethnicity) and social roles. Identity involves a sense of continuity, or the feeling that one is the same person today that one was yesterday or last year (despite physical or other changes). (https://dictionary.apa.org/identity)" .


###  https://purl.org/turbbo/RBBO_0000136
<https://purl.org/turbbo/RBBO_0000136> rdf:type owl:Class ;
                                       rdfs:subClassOf <https://purl.org/turbbo/RBBO_0000124> ;
                                       rdfs:label "Autonomous" ;
                                       <http://www.w3.org/2004/02/skos/core#definition> "Autonomous motivation is defined as engaging in a behaviour because it is perceived to be consistent with intrinsic goals or outcomes and emanates from the self (Hagger et al., 2014)" ,
                                                                                        """Motivation that is internally generated and based on a behaviour being interesting or valuable to an individual.
(BCIO - https://www.bciovocab.org/BCIO:006302) (Qeios - https://www.qeios.com/read/OOD0Z2)""" .


###  https://purl.org/turbbo/RBBO_0000137
<https://purl.org/turbbo/RBBO_0000137> rdf:type owl:Class ;
                                       rdfs:subClassOf <https://purl.org/turbbo/RBBO_0000136> ;
                                       rdfs:label "Intrinsic" ;
                                       <http://www.w3.org/2004/02/skos/core#definition> """Autonomous motivation due to a behaviour's inherent enjoyment, satisfaction or benefits to oneself.
(BCIO - https://www.bciovocab.org/BCIO:006136) (Qeios - https://www.qeios.com/read/DBZBQF)""" ,
                                                                                        "Intrinsic motivation is defined as the doing of an activity for its inherent satisfaction rather than for some separable consequence." .


###  https://purl.org/turbbo/RBBO_0000138
<https://purl.org/turbbo/RBBO_0000138> rdf:type owl:Class ;
                                       rdfs:subClassOf <https://purl.org/turbbo/RBBO_0000124> ;
                                       rdfs:label "Controlled" ;
                                       <http://www.w3.org/2004/02/skos/core#definition> "Engaging in behaviours for externally referenced reasons such as to gain rewards or perceived approval from others or to avoid punishment or feelings of guilt (Hagger et al., 2014)" ,
                                                                                        "Motivation from outside the phenomenal self, by forces experienced as alien or pressuring, be they inner impulses or demands, or external contingencies of reward and punishment (Deci & Ryan, 2006). Self-determination theory (Ryan & Deci, 2000) defines controlled motivation as the opposite of autonomous motivation and so controlled motivation is also referred to as heteronomous." ;
                                       <https://purl.org/turbbo/RBBO_0000150> "Extrinsic Motivation (BCIO)" .


###  https://purl.org/turbbo/RBBO_0000143
<https://purl.org/turbbo/RBBO_0000143> rdf:type owl:Class ;
                                       rdfs:subClassOf <https://purl.org/turbbo/RBBO_0000112> ;
                                       rdfs:label "Effectiveness" ;
                                       <http://www.w3.org/2004/02/skos/core#definition> "The degree of success of a behaviour in achieving its goals. (edited from:https://dictionary.apa.org/effectiveness-evaluation)" .


###  https://purl.org/turbbo/RBBO_0000144
<https://purl.org/turbbo/RBBO_0000144> rdf:type owl:Class ;
                                       <http://purl.obolibrary.org/obo/IAO_0000116> "Revise when Middle ontology is ready" ;
                                       rdfs:label "Nature" .


###  https://purl.org/turbbo/RBBO_0000145
<https://purl.org/turbbo/RBBO_0000145> rdf:type owl:Class ;
                                       rdfs:subClassOf <https://purl.org/turbbo/RBBO_0000144> ;
                                       rdfs:label "Physical" ;
                                       <http://www.w3.org/2004/02/skos/core#definition> """A behavioural capability that involves a musculoskeletal process in its realisation.
(BCIO - https://www.bciovocab.org/BCIO:006009) (Qeios - https://www.qeios.com/read/OAKHLF)""" .


###  https://purl.org/turbbo/RBBO_0000146
<https://purl.org/turbbo/RBBO_0000146> rdf:type owl:Class ;
                                       rdfs:subClassOf <https://purl.org/turbbo/RBBO_0000144> ;
                                       rdfs:label "Psychological" .


###  https://purl.org/turbbo/RBBO_0000148
<https://purl.org/turbbo/RBBO_0000148> rdf:type owl:Class ;
                                       rdfs:subClassOf <https://purl.org/turbbo/RBBO_0000018> ;
                                       rdfs:label "Skill"^^xsd:string ;
                                       <http://www.w3.org/2004/02/skos/core#definition> "An ability or proficiency acquired through training and practice. (https://dictionary.apa.org/skill)"^^xsd:string .


###  https://purl.org/turbbo/RBBO_0000302
<https://purl.org/turbbo/RBBO_0000302> rdf:type owl:Class ;
                                       rdfs:subClassOf <https://purl.org/turbbo/RBBO_0000138> ;
                                       rdfs:label "Extrinsic"@en ;
                                       <http://www.w3.org/2004/02/skos/core#definition> "Extrinsic motivation is defined as a motivation to participate in an activity based on meeting an external goal, garnering praise and approval, winning a competition, or receiving an award or payment." ,
                                                                                        """Motivation that is based on external rewards, punishments or pressure regarding a behaviour.
(BCIO - https://www.bciovocab.org/BCIO:006307) Synonyms: Controlled Motivation (Qeios - https://www.qeios.com/read/KHN5CN)""" .


###  Generated by the OWL API (version 4.5.13) https://github.com/owlcs/owlapi
